<?xml version="1.0" encoding="UTF-8"?>
<rdf:RDF xmlns:dc="http://purl.org/dc/elements/1.1/" xmlns:fedora="info:fedora/" xmlns:rdf="http://www.w3.org/1999/02/22-rdf-syntax-ns#" xmlns:rdfs="http://www.w3.org/2000/01/rdf-schema#" xmlns:skos="http://www.w3.org/2004/02/skos/core#" xmlns:void="http://rdfs.org/ns/void#" xmlns:dct="http://purl.org/dc/terms#">
<!-- expand add definition / check Eastaugh for
     
    browns: Bister 
    metals: definitions
    
    Binding agents; ?? Sulphates; Additives
    Blue green vitriol ??
    -->

    <void:Dataset rdf:about="http://gams.uni-graz.at/">
        <dc:title>Vocabulary for materials used in mediaeval manuscripts - SKOS</dc:title>
        <dc:identifier></dc:identifier>
        <fedora:isMemberOf rdf:resource="info:fedora/context:ontology"/>
        <dc:creator>Ivana Dobcheva (rdf encoding; description texts)</dc:creator>
        <dc:creator>Manfred Schreiner</dc:creator>
        <dc:creator>Wilfried Vetter</dc:creator>       
    </void:Dataset>
    
    <skos:ConceptScheme rdf:about="http://gams.uni-graz.at/thesaurus/mss-materials">
        <dc:title>Materials used for Medieval Manuscripts</dc:title>
        <skos:hasTopConcept rdf:resource="http://gams.uni-graz.at/thesaurus/materials"/>
        <skos:note xml:lang="en">Taxonomy of types of materials associated with medieval manuscripts.</skos:note>
    </skos:ConceptScheme>
    
    <skos:Concept rdf:about="http://gams.uni-graz.at/thesaurus/materials">
        <skos:inScheme rdf:resource="http://gams.uni-graz.at/thesaurus/mss-materials"/>
        <skos:prefLabel xml:lang="de">Materialien</skos:prefLabel>
        <skos:prefLabel xml:lang="en">Materials</skos:prefLabel>
    </skos:Concept>
<!--    ############### Materials by chemical element-->
    <skos:Concept rdf:about="http://gams.uni-graz.at/thesaurus/elements">
        <skos:inScheme rdf:resource="http://gams.uni-graz.at/thesaurus/mss-materials"/>
        <skos:prefLabel xml:lang="en">Chemical elements</skos:prefLabel>
        <skos:prefLabel xml:lang="de">Chemische Elemente</skos:prefLabel>
        <skos:definition xml:lang="en">Chemical elements detected in materials from manuscripts, either as constant ingredients of substances or as so-called impurities within main substances or mixtures.</skos:definition>
        <skos:broader rdf:resource="http://gams.uni-graz.at/thesaurus/materials"/>
    </skos:Concept>
    <skos:Concept rdf:about="http://gams.uni-graz.at/thesaurus/hydrogen">
        <skos:inScheme rdf:resource="http://gams.uni-graz.at/thesaurus/mss-materials"/>
        <skos:prefLabel xml:lang="en">hydrogen</skos:prefLabel>
        <skos:prefLabel xml:lang="de">Wasserstoff</skos:prefLabel>
        <skos:altLabel xml:lang="en">H</skos:altLabel>
        <skos:related rdf:resource="http://data.loterre.fr/ark:/67375/8HQ-DTLN6DML-5"/>
        <skos:broader rdf:resource="http://gams.uni-graz.at/thesaurus/elements"/>
    </skos:Concept>
    
    <skos:Concept rdf:about="http://gams.uni-graz.at/thesaurus/carbon">
        <skos:inScheme rdf:resource="http://gams.uni-graz.at/thesaurus/mss-materials"/>
        <skos:prefLabel xml:lang="en">carbon</skos:prefLabel>
        <skos:prefLabel xml:lang="de">Kohlenstoff</skos:prefLabel>
        <skos:altLabel xml:lang="en">C</skos:altLabel>
        <skos:related rdf:resource="http://data.loterre.fr/ark:/67375/8HQ-GPJ5KG69-K"/>
        <skos:broader rdf:resource="http://gams.uni-graz.at/thesaurus/elements"/>
    </skos:Concept>
    <skos:Concept rdf:about="http://gams.uni-graz.at/thesaurus/nitrogen">
        <skos:inScheme rdf:resource="http://gams.uni-graz.at/thesaurus/mss-materials"/>
        <skos:prefLabel xml:lang="en">nitrogen</skos:prefLabel>
        <skos:prefLabel xml:lang="de">Stickstoff</skos:prefLabel>
        <skos:altLabel xml:lang="en">N</skos:altLabel>
        <skos:related rdf:resource="http://data.loterre.fr/ark:/67375/8HQ-FMW7R7GT-H"/>
        <skos:broader rdf:resource="http://gams.uni-graz.at/thesaurus/elements"/>
    </skos:Concept>
    <skos:Concept rdf:about="http://gams.uni-graz.at/thesaurus/oxygen">
        <skos:inScheme rdf:resource="http://gams.uni-graz.at/thesaurus/mss-materials"/>
        <skos:prefLabel xml:lang="en">oxygen</skos:prefLabel>
        <skos:prefLabel xml:lang="de">Sauerstoff</skos:prefLabel>
        <skos:altLabel xml:lang="en">O</skos:altLabel>
        <skos:related rdf:resource="http://data.loterre.fr/ark:/67375/8HQ-RX5D8P7R-1"/>
        <skos:broader rdf:resource="http://gams.uni-graz.at/thesaurus/elements"/>
    </skos:Concept>
    <skos:Concept rdf:about="http://gams.uni-graz.at/thesaurus/fluorine">
        <skos:inScheme rdf:resource="http://gams.uni-graz.at/thesaurus/mss-materials"/>
        <skos:prefLabel xml:lang="en">fluorine</skos:prefLabel>
        <skos:prefLabel xml:lang="de">Fluor</skos:prefLabel>
        <skos:altLabel xml:lang="en">F</skos:altLabel>
        <skos:related rdf:resource="http://data.loterre.fr/ark:/67375/8HQ-XNB95WRM-4"/>
        <skos:broader rdf:resource="http://gams.uni-graz.at/thesaurus/elements"/>
    </skos:Concept>
    
    <skos:Concept rdf:about="http://gams.uni-graz.at/thesaurus/sodium">
        <skos:inScheme rdf:resource="http://gams.uni-graz.at/thesaurus/mss-materials"/>
        <skos:altLabel xml:lang="en">Na</skos:altLabel>
        <skos:prefLabel xml:lang="en">sodium</skos:prefLabel>
        <skos:prefLabel xml:lang="de">Natrium</skos:prefLabel>
        <skos:related rdf:resource="http://data.loterre.fr/ark:/67375/8HQ-D9J9ZG62-C"/>
        <skos:broader rdf:resource="http://gams.uni-graz.at/thesaurus/elements"/>
    </skos:Concept>
    <skos:Concept rdf:about="http://gams.uni-graz.at/thesaurus/magnesium">
        <skos:inScheme rdf:resource="http://gams.uni-graz.at/thesaurus/mss-materials"/>
        <skos:prefLabel xml:lang="en">magnesium</skos:prefLabel>
        <skos:altLabel xml:lang="en">Mg</skos:altLabel>
        <skos:prefLabel xml:lang="de">Magnesium</skos:prefLabel>
        <skos:related rdf:resource="http://data.loterre.fr/ark:/67375/8HQ-S4R6VJD9-W"/>
        <skos:broader rdf:resource="http://gams.uni-graz.at/thesaurus/elements"/>
    </skos:Concept>
    <skos:Concept rdf:about="http://gams.uni-graz.at/thesaurus/aluminium">
        <skos:inScheme rdf:resource="http://gams.uni-graz.at/thesaurus/mss-materials"/>
        <skos:prefLabel xml:lang="en">aluminium</skos:prefLabel>
        <skos:prefLabel xml:lang="de">Aluminium</skos:prefLabel>
        <skos:altLabel xml:lang="en">Al</skos:altLabel>
        <skos:related rdf:resource="http://data.loterre.fr/ark:/67375/8HQ-X55C5RJ1-N"/>
        <skos:broader rdf:resource="http://gams.uni-graz.at/thesaurus/elements"/>
    </skos:Concept>
    <skos:Concept rdf:about="http://gams.uni-graz.at/thesaurus/silicon">
        <skos:inScheme rdf:resource="http://gams.uni-graz.at/thesaurus/mss-materials"/>
        <skos:prefLabel xml:lang="en">silicon</skos:prefLabel>
        <skos:prefLabel xml:lang="de">Silicium</skos:prefLabel>
        <skos:altLabel xml:lang="en">Si</skos:altLabel>
        <skos:related rdf:resource="http://data.loterre.fr/ark:/67375/8HQ-Q69H14CX-1"/>
        <skos:broader rdf:resource="http://gams.uni-graz.at/thesaurus/elements"/>
    </skos:Concept>
    <skos:Concept rdf:about="http://gams.uni-graz.at/thesaurus/phosphorus">
        <skos:inScheme rdf:resource="http://gams.uni-graz.at/thesaurus/mss-materials"/>
        <skos:prefLabel xml:lang="en">phosphorus</skos:prefLabel>
        <skos:prefLabel xml:lang="de">Phosphor</skos:prefLabel>
        <skos:altLabel xml:lang="en">P</skos:altLabel>
        <skos:related rdf:resource="http://data.loterre.fr/ark:/67375/8HQ-VC1M1XR4-F"/>
        <skos:broader rdf:resource="http://gams.uni-graz.at/thesaurus/elements"/>
    </skos:Concept>
    <skos:Concept rdf:about="http://gams.uni-graz.at/thesaurus/sulfur">
        <skos:inScheme rdf:resource="http://gams.uni-graz.at/thesaurus/mss-materials"/>
        <skos:prefLabel xml:lang="en">sulfur</skos:prefLabel>
        <skos:prefLabel xml:lang="de">Schwefel</skos:prefLabel>
        <skos:altLabel xml:lang="en">S</skos:altLabel>
        <skos:related rdf:resource="http://data.loterre.fr/ark:/67375/8HQ-NK1JKPQC-4"/>
        <skos:broader rdf:resource="http://gams.uni-graz.at/thesaurus/elements"/>
    </skos:Concept>
    <skos:Concept rdf:about="http://gams.uni-graz.at/thesaurus/chlorine">
        <skos:inScheme rdf:resource="http://gams.uni-graz.at/thesaurus/mss-materials"/>
        <skos:prefLabel xml:lang="en">chlorine</skos:prefLabel>
        <skos:prefLabel xml:lang="de">Chlor</skos:prefLabel>
        <skos:altLabel xml:lang="en">Cl</skos:altLabel>
        <skos:related rdf:resource="http://data.loterre.fr/ark:/67375/8HQ-HKV44ZNF-C"/>
        <skos:broader rdf:resource="http://gams.uni-graz.at/thesaurus/elements"/>
    </skos:Concept>
    <skos:Concept rdf:about="http://gams.uni-graz.at/thesaurus/argon">
        <skos:inScheme rdf:resource="http://gams.uni-graz.at/thesaurus/mss-materials"/>
        <skos:prefLabel xml:lang="en">argon</skos:prefLabel>
        <skos:prefLabel xml:lang="de">Argon</skos:prefLabel>
        <skos:altLabel xml:lang="en">Ar</skos:altLabel>
        <skos:related rdf:resource="http://data.loterre.fr/ark:/67375/8HQ-XZG1JMS2-0"/>
        <skos:broader rdf:resource="http://gams.uni-graz.at/thesaurus/elements"/>
    </skos:Concept>
    <skos:Concept rdf:about="http://gams.uni-graz.at/thesaurus/kalium">
        <skos:inScheme rdf:resource="http://gams.uni-graz.at/thesaurus/mss-materials"/>
        <skos:altLabel xml:lang="en">K</skos:altLabel>
        <skos:prefLabel xml:lang="de">Kalium</skos:prefLabel>
        <skos:prefLabel xml:lang="en">potassium</skos:prefLabel>
        <skos:related rdf:resource="http://data.loterre.fr/ark:/67375/8HQ-LGJQJQQ9-N"/>
        <skos:broader rdf:resource="http://gams.uni-graz.at/thesaurus/elements"/>
    </skos:Concept>
    <skos:Concept rdf:about="http://gams.uni-graz.at/thesaurus/calcium">
        <skos:inScheme rdf:resource="http://gams.uni-graz.at/thesaurus/mss-materials"/>
        <skos:prefLabel xml:lang="en">calcium</skos:prefLabel>
        <skos:prefLabel xml:lang="de">Calcium</skos:prefLabel>
        <skos:altLabel xml:lang="en">Ca</skos:altLabel>
        <skos:related rdf:resource="http://data.loterre.fr/ark:/67375/8HQ-SX8VX34H-4"/>
        <skos:broader rdf:resource="http://gams.uni-graz.at/thesaurus/elements"/>
    </skos:Concept>
    
    <skos:Concept rdf:about="http://gams.uni-graz.at/thesaurus/titanium">
        <skos:inScheme rdf:resource="http://gams.uni-graz.at/thesaurus/mss-materials"/>
        <skos:prefLabel xml:lang="en">titanium</skos:prefLabel>
        <skos:prefLabel xml:lang="de">Titan</skos:prefLabel>
        <skos:altLabel xml:lang="en">Ti</skos:altLabel>
        <skos:related rdf:resource="http://data.loterre.fr/ark:/67375/8HQ-B46N74X6-Z"/>
        <skos:broader rdf:resource="http://gams.uni-graz.at/thesaurus/elements"/>
    </skos:Concept>
    
    <skos:Concept rdf:about="http://gams.uni-graz.at/thesaurus/chromium">
        <skos:inScheme rdf:resource="http://gams.uni-graz.at/thesaurus/mss-materials"/>
        <skos:prefLabel xml:lang="en">chromium</skos:prefLabel>
        <skos:prefLabel xml:lang="de">Chrom</skos:prefLabel>
        <skos:altLabel xml:lang="en">Cr</skos:altLabel>
        <skos:related rdf:resource="http://data.loterre.fr/ark:/67375/8HQ-W2MFT88M-C"/>
        <skos:broader rdf:resource="http://gams.uni-graz.at/thesaurus/elements"/>
    </skos:Concept>
    <skos:Concept rdf:about="http://gams.uni-graz.at/thesaurus/manganese">
        <skos:inScheme rdf:resource="http://gams.uni-graz.at/thesaurus/mss-materials"/>
        <skos:prefLabel xml:lang="en">manganese</skos:prefLabel>
        <skos:prefLabel xml:lang="de">Mangan</skos:prefLabel>
        <skos:altLabel xml:lang="en">Mn</skos:altLabel>
        <skos:related rdf:resource="http://data.loterre.fr/ark:/67375/8HQ-ZHXJ4D8T-H"/>
        <skos:broader rdf:resource="http://gams.uni-graz.at/thesaurus/elements"/>
    </skos:Concept>
    <skos:Concept rdf:about="http://gams.uni-graz.at/thesaurus/iron">
        <skos:inScheme rdf:resource="http://gams.uni-graz.at/thesaurus/mss-materials"/>
        <skos:prefLabel xml:lang="en">iron</skos:prefLabel>
        <skos:prefLabel xml:lang="de">Eisen</skos:prefLabel>
        <skos:altLabel xml:lang="en">Fe</skos:altLabel>
        <skos:related rdf:resource="http://data.loterre.fr/ark:/67375/8HQ-NQ0K580N-5"/>
        <skos:broader rdf:resource="http://gams.uni-graz.at/thesaurus/elements"/>
    </skos:Concept>
    <skos:Concept rdf:about="http://gams.uni-graz.at/thesaurus/cobalt">
        <skos:inScheme rdf:resource="http://gams.uni-graz.at/thesaurus/mss-materials"/>
        <skos:prefLabel xml:lang="en">cobalt</skos:prefLabel>
        <skos:prefLabel xml:lang="de">Cobalt</skos:prefLabel>
        <skos:altLabel xml:lang="en">Co</skos:altLabel>
        <skos:related rdf:resource="http://data.loterre.fr/ark:/67375/8HQ-BVR52VXN-F"/>
        <skos:broader rdf:resource="http://gams.uni-graz.at/thesaurus/elements"/>
    </skos:Concept>
    <skos:Concept rdf:about="http://gams.uni-graz.at/thesaurus/nickel">
        <skos:inScheme rdf:resource="http://gams.uni-graz.at/thesaurus/mss-materials"/>
        <skos:prefLabel xml:lang="en">nickel</skos:prefLabel>
        <skos:prefLabel xml:lang="de">Nickel</skos:prefLabel>
        <skos:altLabel xml:lang="en">Ni</skos:altLabel>
        <skos:related rdf:resource="http://data.loterre.fr/ark:/67375/8HQ-FDQVX1R1-D"/>
        <skos:broader rdf:resource="http://gams.uni-graz.at/thesaurus/elements"/>
    </skos:Concept>
    <skos:Concept rdf:about="http://gams.uni-graz.at/thesaurus/copper">
        <skos:inScheme rdf:resource="http://gams.uni-graz.at/thesaurus/mss-materials"/>
        <skos:prefLabel xml:lang="en">copper</skos:prefLabel>
        <skos:prefLabel xml:lang="de">Kupfer</skos:prefLabel>
        <skos:altLabel xml:lang="en">Cu</skos:altLabel>
        <skos:related rdf:resource="http://data.loterre.fr/ark:/67375/8HQ-G3VCNX8B-6"/>
        <skos:broader rdf:resource="http://gams.uni-graz.at/thesaurus/elements"/>
    </skos:Concept>
    <skos:Concept rdf:about="http://gams.uni-graz.at/thesaurus/zinc">
        <skos:inScheme rdf:resource="http://gams.uni-graz.at/thesaurus/mss-materials"/>
        <skos:prefLabel xml:lang="en">zinc</skos:prefLabel>
        <skos:prefLabel xml:lang="de">Zink</skos:prefLabel>
        <skos:altLabel xml:lang="en">Zn</skos:altLabel>
        <skos:related rdf:resource="http://data.loterre.fr/ark:/67375/8HQ-ZH5RPRR9-D"/>
        <skos:broader rdf:resource="http://gams.uni-graz.at/thesaurus/elements"/>
    </skos:Concept>
   
    <skos:Concept rdf:about="http://gams.uni-graz.at/thesaurus/arsenic">
        <skos:inScheme rdf:resource="http://gams.uni-graz.at/thesaurus/mss-materials"/>
        <skos:prefLabel xml:lang="en">arsenic</skos:prefLabel>
        <skos:prefLabel xml:lang="de">Arsen</skos:prefLabel>
        <skos:altLabel xml:lang="en">As</skos:altLabel>
        <skos:related rdf:resource="http://data.loterre.fr/ark:/67375/8HQ-B31MNC3P-0"/>
        <skos:broader rdf:resource="http://gams.uni-graz.at/thesaurus/elements"/>
    </skos:Concept>
    <skos:Concept rdf:about="http://gams.uni-graz.at/thesaurus/selenium">
        <skos:inScheme rdf:resource="http://gams.uni-graz.at/thesaurus/mss-materials"/>
        <skos:prefLabel xml:lang="en">selenium</skos:prefLabel>
        <skos:prefLabel xml:lang="de">Selen</skos:prefLabel>
        <skos:altLabel xml:lang="en">Se</skos:altLabel>
        <skos:related rdf:resource="http://data.loterre.fr/ark:/67375/8HQ-SSFNCHSK-B"/>
        <skos:broader rdf:resource="http://gams.uni-graz.at/thesaurus/elements"/>
    </skos:Concept>
    <skos:Concept rdf:about="http://gams.uni-graz.at/thesaurus/bromine">
        <skos:inScheme rdf:resource="http://gams.uni-graz.at/thesaurus/mss-materials"/>
        <skos:prefLabel xml:lang="en">bromine</skos:prefLabel>
        <skos:prefLabel xml:lang="de">Brom</skos:prefLabel>
        <skos:altLabel xml:lang="en">Br</skos:altLabel>
        <skos:related rdf:resource="http://data.loterre.fr/ark:/67375/8HQ-JKQD0SHX-7"/>
        <skos:broader rdf:resource="http://gams.uni-graz.at/thesaurus/elements"/>
    </skos:Concept>
        
    <skos:Concept rdf:about="http://gams.uni-graz.at/thesaurus/strontium">
        <skos:inScheme rdf:resource="http://gams.uni-graz.at/thesaurus/mss-materials"/>
        <skos:prefLabel xml:lang="en">strontium</skos:prefLabel>
        <skos:prefLabel xml:lang="de">Strontium</skos:prefLabel>
        <skos:altLabel xml:lang="en">Sr</skos:altLabel>
        <skos:related rdf:resource="http://data.loterre.fr/ark:/67375/8HQ-GL3J8X2V-F"/>
        <skos:broader rdf:resource="http://gams.uni-graz.at/thesaurus/elements"/>
    </skos:Concept>
    
    <skos:Concept rdf:about="http://gams.uni-graz.at/thesaurus/zirconium">
        <skos:inScheme rdf:resource="http://gams.uni-graz.at/thesaurus/mss-materials"/>
        <skos:prefLabel xml:lang="en">zirconium</skos:prefLabel>
        <skos:prefLabel xml:lang="de">Zirconium</skos:prefLabel>
        <skos:altLabel xml:lang="en">Zr</skos:altLabel>
        <skos:related rdf:resource="http://data.loterre.fr/ark:/67375/8HQ-NCV4MKFK-N"/>
        <skos:broader rdf:resource="http://gams.uni-graz.at/thesaurus/elements"/>
    </skos:Concept>
    
    <skos:Concept rdf:about="http://gams.uni-graz.at/thesaurus/molybdenum">
        <skos:inScheme rdf:resource="http://gams.uni-graz.at/thesaurus/mss-materials"/>
        <skos:prefLabel xml:lang="en">molybdenum</skos:prefLabel>
        <skos:prefLabel xml:lang="de">Molybdän</skos:prefLabel>
        <skos:altLabel xml:lang="en">Mo</skos:altLabel>
        <skos:related rdf:resource="http://data.loterre.fr/ark:/67375/8HQ-KZJDHQWD-3"/>
        <skos:broader rdf:resource="http://gams.uni-graz.at/thesaurus/elements"/>
    </skos:Concept>   
    
    <skos:Concept rdf:about="http://gams.uni-graz.at/thesaurus/rhodium">
        <skos:inScheme rdf:resource="http://gams.uni-graz.at/thesaurus/mss-materials"/>
        <skos:prefLabel xml:lang="en">rhodium</skos:prefLabel>
        <skos:prefLabel xml:lang="de">Rhodium</skos:prefLabel>
        <skos:altLabel xml:lang="en">Rh</skos:altLabel>
        <skos:related rdf:resource="http://data.loterre.fr/ark:/67375/8HQ-FKKNQWB0-B"/>
        <skos:broader rdf:resource="http://gams.uni-graz.at/thesaurus/elements"/>
    </skos:Concept>
    
    <skos:Concept rdf:about="http://gams.uni-graz.at/thesaurus/silver">
        <skos:inScheme rdf:resource="http://gams.uni-graz.at/thesaurus/mss-materials"/>
        <skos:prefLabel xml:lang="en">silver</skos:prefLabel>
        <skos:prefLabel xml:lang="de">Silber</skos:prefLabel>
        <skos:altLabel xml:lang="en">Ag</skos:altLabel>
        <skos:related rdf:resource="http://data.loterre.fr/ark:/67375/8HQ-MBPSKJ5K-B"/>
        <skos:broader rdf:resource="http://gams.uni-graz.at/thesaurus/elements"/>
    </skos:Concept>
    <skos:Concept rdf:about="http://gams.uni-graz.at/thesaurus/cadmium">
        <skos:inScheme rdf:resource="http://gams.uni-graz.at/thesaurus/mss-materials"/>
        <skos:prefLabel xml:lang="en">cadmium</skos:prefLabel>
        <skos:prefLabel xml:lang="de">Cadmium</skos:prefLabel>
        <skos:altLabel xml:lang="en">Cd</skos:altLabel>
        <skos:related rdf:resource="http://data.loterre.fr/ark:/67375/8HQ-R5TL4FBV-J"/>
        <skos:broader rdf:resource="http://gams.uni-graz.at/thesaurus/elements"/>
    </skos:Concept>
    
    <skos:Concept rdf:about="http://gams.uni-graz.at/thesaurus/tin">
        <skos:inScheme rdf:resource="http://gams.uni-graz.at/thesaurus/mss-materials"/>
        <skos:prefLabel xml:lang="en">tin</skos:prefLabel>
        <skos:prefLabel xml:lang="de">Zinn</skos:prefLabel>
        <skos:altLabel xml:lang="en">Sn</skos:altLabel>
        <skos:related rdf:resource="http://data.loterre.fr/ark:/67375/8HQ-ZK5FBL3T-Z"/>
        <skos:broader rdf:resource="http://gams.uni-graz.at/thesaurus/elements"/>
    </skos:Concept>
    <skos:Concept rdf:about="http://gams.uni-graz.at/thesaurus/antimony">
        <skos:inScheme rdf:resource="http://gams.uni-graz.at/thesaurus/mss-materials"/>
        <skos:prefLabel xml:lang="en">antimony</skos:prefLabel>
        <skos:prefLabel xml:lang="de">Antimon</skos:prefLabel>
        <skos:altLabel xml:lang="en">Sb</skos:altLabel>
        <skos:related rdf:resource="http://data.loterre.fr/ark:/67375/8HQ-LGWKM8TW-9"/>
        <skos:broader rdf:resource="http://gams.uni-graz.at/thesaurus/elements"/>
    </skos:Concept>
    
    <skos:Concept rdf:about="http://gams.uni-graz.at/thesaurus/iod">
        <skos:inScheme rdf:resource="http://gams.uni-graz.at/thesaurus/mss-materials"/>
        <skos:altLabel xml:lang="en">I</skos:altLabel>
        <skos:prefLabel xml:lang="de">Iod</skos:prefLabel>
        <skos:prefLabel xml:lang="en">iodine</skos:prefLabel>
        <skos:related rdf:resource="http://data.loterre.fr/ark:/67375/8HQ-W76CCWHW-C"/>
        <skos:broader rdf:resource="http://gams.uni-graz.at/thesaurus/elements"/>
    </skos:Concept>
        
    <skos:Concept rdf:about="http://gams.uni-graz.at/thesaurus/barium">
        <skos:inScheme rdf:resource="http://gams.uni-graz.at/thesaurus/mss-materials"/>
        <skos:prefLabel xml:lang="en">barium</skos:prefLabel>
        <skos:prefLabel xml:lang="de">Barium</skos:prefLabel>
        <skos:altLabel xml:lang="en">Ba</skos:altLabel>
        <skos:related rdf:resource="http://data.loterre.fr/ark:/67375/8HQ-P1S60994-X"/>
        <skos:broader rdf:resource="http://gams.uni-graz.at/thesaurus/elements"/>
    </skos:Concept>   
   
    <skos:Concept rdf:about="http://gams.uni-graz.at/thesaurus/tungsten">
        <skos:inScheme rdf:resource="http://gams.uni-graz.at/thesaurus/mss-materials"/>
        <skos:prefLabel xml:lang="en">tungsten</skos:prefLabel>
        <skos:prefLabel xml:lang="de">Wolfram</skos:prefLabel>
        <skos:altLabel xml:lang="en">W</skos:altLabel>
        <skos:related rdf:resource="http://data.loterre.fr/ark:/67375/8HQ-B030NV4K-M"/>
        <skos:broader rdf:resource="http://gams.uni-graz.at/thesaurus/elements"/>
    </skos:Concept>
    
    <skos:Concept rdf:about="http://gams.uni-graz.at/thesaurus/platinum">
        <skos:inScheme rdf:resource="http://gams.uni-graz.at/thesaurus/mss-materials"/>
        <skos:prefLabel xml:lang="en">platinum</skos:prefLabel>
        <skos:prefLabel xml:lang="de">Platin</skos:prefLabel>
        <skos:altLabel xml:lang="en">Pt</skos:altLabel>
        <skos:related rdf:resource="http://data.loterre.fr/ark:/67375/8HQ-HCSZZCGN-4"/>
        <skos:broader rdf:resource="http://gams.uni-graz.at/thesaurus/elements"/>
    </skos:Concept>
    <skos:Concept rdf:about="http://gams.uni-graz.at/thesaurus/gold">
        <skos:inScheme rdf:resource="http://gams.uni-graz.at/thesaurus/mss-materials"/>
        <skos:prefLabel xml:lang="en">gold</skos:prefLabel>
        <skos:prefLabel xml:lang="de">Gold</skos:prefLabel>
        <skos:altLabel xml:lang="en">Au</skos:altLabel>
        <skos:related rdf:resource="http://data.loterre.fr/ark:/67375/8HQ-HD8QM9KB-M"/>
        <skos:broader rdf:resource="http://gams.uni-graz.at/thesaurus/elements"/>
    </skos:Concept>
    <skos:Concept rdf:about="http://gams.uni-graz.at/thesaurus/mercury">
        <skos:inScheme rdf:resource="http://gams.uni-graz.at/thesaurus/mss-materials"/>
        <skos:prefLabel xml:lang="en">mercury</skos:prefLabel>
        <skos:prefLabel xml:lang="de">Quecksilber</skos:prefLabel>
        <skos:altLabel xml:lang="en">Hg</skos:altLabel>
        <skos:related rdf:resource="http://data.loterre.fr/ark:/67375/8HQ-H9J0KWB5-L"/>
        <skos:broader rdf:resource="http://gams.uni-graz.at/thesaurus/elements"/>
    </skos:Concept>
   
    <skos:Concept rdf:about="http://gams.uni-graz.at/thesaurus/lead">
        <skos:inScheme rdf:resource="http://gams.uni-graz.at/thesaurus/mss-materials"/>
        <skos:prefLabel xml:lang="en">lead</skos:prefLabel>
        <skos:prefLabel xml:lang="de">Blei</skos:prefLabel>
        <skos:altLabel xml:lang="en">Pb</skos:altLabel>
        <skos:related rdf:resource="http://data.loterre.fr/ark:/67375/8HQ-NRPKN8GG-H"/>
        <skos:broader rdf:resource="http://gams.uni-graz.at/thesaurus/elements"/>
    </skos:Concept>
    <skos:Concept rdf:about="http://gams.uni-graz.at/thesaurus/bismuth">
        <skos:inScheme rdf:resource="http://gams.uni-graz.at/thesaurus/mss-materials"/>
        <skos:prefLabel xml:lang="en">bismuth</skos:prefLabel>
        <skos:prefLabel xml:lang="de">Bismut</skos:prefLabel>
        <skos:altLabel xml:lang="en">Bi</skos:altLabel>
        <skos:related rdf:resource="http://data.loterre.fr/ark:/67375/8HQ-SLTRM919-5"/>
        <skos:broader rdf:resource="http://gams.uni-graz.at/thesaurus/elements"/>
    </skos:Concept>   
   
    
<!--    ######### Materials by role -->
    <skos:Concept rdf:about="http://gams.uni-graz.at/thesaurus/materials_role">
        <skos:prefLabel xml:lang="en">Materials by their role</skos:prefLabel>
        <skos:prefLabel xml:lang="de">Materialien nach Funktionen</skos:prefLabel>
        <skos:definition xml:lang="en">Materials used in medieval manuscripts grouped according to their role as colorants, binding agents etc. </skos:definition>
        <skos:broader rdf:resource="http://gams.uni-graz.at/thesaurus/materials"/>
    </skos:Concept>
    
    <skos:Concept rdf:about="http://gams.uni-graz.at/thesaurus/other_materials">
        <skos:inScheme rdf:resource="http://gams.uni-graz.at/thesaurus/mss-materials"/>
        <skos:prefLabel xml:lang="de">Andere Materialien</skos:prefLabel>
        <skos:prefLabel xml:lang="en">Other materials</skos:prefLabel>
        <skos:definition xml:lang="en">A class for substances detected during material analysis, which either cannot be identified (with the methods applied), or do not fall under the existing classifications (i.e. colorants, binding agents etc.).</skos:definition>
        <skos:broader rdf:resource="http://gams.uni-graz.at/thesaurus/materials_role"/>
    </skos:Concept>
<!--    ######## WRITING SUPPORT ###########-->
    <skos:Concept rdf:about="http://gams.uni-graz.at/thesaurus/support">
        <skos:inScheme rdf:resource="http://gams.uni-graz.at/thesaurus/mss-materials"/>
        <skos:prefLabel xml:lang="de">Beschreibstoffe</skos:prefLabel>
        <skos:prefLabel xml:lang="en">Writing supports</skos:prefLabel>
        <skos:broader rdf:resource="http://gams.uni-graz.at/thesaurus/materials_role"/>
    </skos:Concept>
    
    <skos:Concept rdf:about="http://gams.uni-graz.at/thesaurus/parchment">
        <skos:inScheme rdf:resource="http://gams.uni-graz.at/thesaurus/mss-materials"/>
        <skos:prefLabel xml:lang="de">Pergament</skos:prefLabel>
        <skos:prefLabel xml:lang="en">Parchment</skos:prefLabel>
        <skos:broader rdf:resource="http://gams.uni-graz.at/thesaurus/support"/>
    </skos:Concept>  
    <skos:Concept rdf:about="http://gams.uni-graz.at/thesaurus/parchment_sheep">
        <skos:inScheme rdf:resource="http://gams.uni-graz.at/thesaurus/mss-materials"/>
        <skos:prefLabel xml:lang="de">Schafspergament</skos:prefLabel>
        <skos:prefLabel xml:lang="en">Sheep parchment</skos:prefLabel>
        <skos:broader rdf:resource="http://gams.uni-graz.at/thesaurus/parchment"/>
    </skos:Concept>
    <skos:Concept rdf:about="http://gams.uni-graz.at/thesaurus/parchment_goat">
        <skos:inScheme rdf:resource="http://gams.uni-graz.at/thesaurus/mss-materials"/>
        <skos:prefLabel xml:lang="de">Ziegenpergament</skos:prefLabel>
        <skos:prefLabel xml:lang="en">Goat parchment</skos:prefLabel>
        <skos:broader rdf:resource="http://gams.uni-graz.at/thesaurus/parchment"/>
    </skos:Concept>
    <skos:Concept rdf:about="http://gams.uni-graz.at/thesaurus/parchment_calf">
        <skos:inScheme rdf:resource="http://gams.uni-graz.at/thesaurus/mss-materials"/>
        <skos:prefLabel xml:lang="de">Kalbspergament</skos:prefLabel>
        <skos:prefLabel xml:lang="en">Calf parchment</skos:prefLabel>
        <skos:broader rdf:resource="http://gams.uni-graz.at/thesaurus/parchment"/>
    </skos:Concept>
    
    <skos:Concept rdf:about="http://gams.uni-graz.at/thesaurus/paper">
        <skos:inScheme rdf:resource="http://gams.uni-graz.at/thesaurus/mss-materials"/>
        <skos:prefLabel xml:lang="de">Papier</skos:prefLabel>
        <skos:prefLabel xml:lang="en">Paper</skos:prefLabel>
        <skos:broader rdf:resource="http://gams.uni-graz.at/thesaurus/support"/>
    </skos:Concept>
    <skos:Concept rdf:about="http://gams.uni-graz.at/thesaurus/papyrus">
        <skos:inScheme rdf:resource="http://gams.uni-graz.at/thesaurus/mss-materials"/>
        <skos:prefLabel xml:lang="de">Papyrus</skos:prefLabel>
        <skos:prefLabel xml:lang="en">Papyrus</skos:prefLabel>
        <skos:broader rdf:resource="http://gams.uni-graz.at/thesaurus/support"/>
    </skos:Concept>    
    <skos:Concept rdf:about="http://gams.uni-graz.at/thesaurus/wood">
        <skos:inScheme rdf:resource="http://gams.uni-graz.at/thesaurus/mss-materials"/>
        <skos:prefLabel xml:lang="de">Holz</skos:prefLabel>
        <skos:prefLabel xml:lang="en">Wood</skos:prefLabel>
        <skos:broader rdf:resource="http://gams.uni-graz.at/thesaurus/support"/>
    </skos:Concept>
    <skos:Concept rdf:about="http://gams.uni-graz.at/thesaurus/palm_leaves">
        <skos:inScheme rdf:resource="http://gams.uni-graz.at/thesaurus/mss-materials"/>
        <skos:prefLabel xml:lang="de">Palmblätter</skos:prefLabel>
        <skos:prefLabel xml:lang="en">Palm leaves</skos:prefLabel>
        <skos:broader rdf:resource="http://gams.uni-graz.at/thesaurus/support"/>
    </skos:Concept>
    <skos:Concept rdf:about="http://gams.uni-graz.at/thesaurus/leather">
        <skos:inScheme rdf:resource="http://gams.uni-graz.at/thesaurus/mss-materials"/>
        <skos:prefLabel xml:lang="de">Leder</skos:prefLabel>
        <skos:prefLabel xml:lang="en">Leather</skos:prefLabel>
        <skos:broader rdf:resource="http://gams.uni-graz.at/thesaurus/support"/>
    </skos:Concept>
    <skos:Concept rdf:about="http://gams.uni-graz.at/thesaurus/wax">
        <skos:inScheme rdf:resource="http://gams.uni-graz.at/thesaurus/mss-materials"/>
        <skos:prefLabel xml:lang="de">Wachs</skos:prefLabel>
        <skos:prefLabel xml:lang="en">Wax</skos:prefLabel>
        <skos:broader rdf:resource="http://gams.uni-graz.at/thesaurus/support"/>
    </skos:Concept>
    <skos:Concept rdf:about="http://gams.uni-graz.at/thesaurus/textile">
        <skos:inScheme rdf:resource="http://gams.uni-graz.at/thesaurus/mss-materials"/>
        <skos:prefLabel xml:lang="de">Textilien</skos:prefLabel>
        <skos:prefLabel xml:lang="en">Textile</skos:prefLabel>
        <skos:broader rdf:resource="http://gams.uni-graz.at/thesaurus/support"/>
    </skos:Concept>
    <skos:Concept rdf:about="http://gams.uni-graz.at/thesaurus/linen">
        <skos:inScheme rdf:resource="http://gams.uni-graz.at/thesaurus/mss-materials"/>
        <skos:prefLabel xml:lang="de">Leinen</skos:prefLabel>
        <skos:prefLabel xml:lang="en">Linen</skos:prefLabel>
        <skos:broader rdf:resource="http://gams.uni-graz.at/thesaurus/textile"/>
    </skos:Concept>
    <skos:Concept rdf:about="http://gams.uni-graz.at/thesaurus/silk">
        <skos:inScheme rdf:resource="http://gams.uni-graz.at/thesaurus/mss-materials"/>
        <skos:prefLabel xml:lang="de">Seide</skos:prefLabel>
        <skos:prefLabel xml:lang="en">Silk</skos:prefLabel>
        <skos:broader rdf:resource="http://gams.uni-graz.at/thesaurus/textile"/>
    </skos:Concept>
    <skos:Concept rdf:about="http://gams.uni-graz.at/thesaurus/cotton">
        <skos:inScheme rdf:resource="http://gams.uni-graz.at/thesaurus/mss-materials"/>
        <skos:prefLabel xml:lang="de">Baumwolle</skos:prefLabel>
        <skos:prefLabel xml:lang="en">Cotton</skos:prefLabel>
        <skos:broader rdf:resource="http://gams.uni-graz.at/thesaurus/textile"/>
    </skos:Concept>
    <skos:Concept rdf:about="http://gams.uni-graz.at/thesaurus/hemp">
        <skos:inScheme rdf:resource="http://gams.uni-graz.at/thesaurus/mss-materials"/>
        <skos:prefLabel xml:lang="de">Hanf</skos:prefLabel>
        <skos:prefLabel xml:lang="en">Hemp</skos:prefLabel>
        <skos:broader rdf:resource="http://gams.uni-graz.at/thesaurus/textile"/>
    </skos:Concept>
    <skos:Concept rdf:about="http://gams.uni-graz.at/thesaurus/wool">
        <skos:inScheme rdf:resource="http://gams.uni-graz.at/thesaurus/mss-materials"/>
        <skos:prefLabel xml:lang="de">Wolle</skos:prefLabel>
        <skos:prefLabel xml:lang="en">Wool</skos:prefLabel>
        <skos:broader rdf:resource="http://gams.uni-graz.at/thesaurus/textile"/>
    </skos:Concept>   

    
<!--    ############### BINDING  AGENTS ########## -->
    <skos:Concept rdf:about="http://gams.uni-graz.at/thesaurus/binding-agents">
        <skos:inScheme rdf:resource="http://gams.uni-graz.at/thesaurus/mss-materials"/>
        <skos:prefLabel xml:lang="de">Bindemittel</skos:prefLabel>
        <skos:prefLabel xml:lang="en">Binding agents</skos:prefLabel>
        <skos:broader rdf:resource="http://gams.uni-graz.at/thesaurus/materials_role"/>
    </skos:Concept>
    <skos:Concept rdf:about="http://gams.uni-graz.at/thesaurus/proteinaceous">
        <skos:inScheme rdf:resource="http://gams.uni-graz.at/thesaurus/mss-materials"/>
        <skos:prefLabel xml:lang="de">Proteinhaltige Bindemittel</skos:prefLabel>
        <skos:prefLabel xml:lang="en">Proteinaceous binding agents</skos:prefLabel>
        <skos:broader rdf:resource="http://gams.uni-graz.at/thesaurus/binding-agents"/>
    </skos:Concept>
    <skos:Concept rdf:about="http://gams.uni-graz.at/thesaurus/egg-white">
        <skos:inScheme rdf:resource="http://gams.uni-graz.at/thesaurus/mss-materials"/>
        <skos:prefLabel xml:lang="de">Eiweiß</skos:prefLabel>
        <skos:prefLabel xml:lang="en">Egg white</skos:prefLabel>
        <skos:broader rdf:resource="http://gams.uni-graz.at/thesaurus/proteinaceous"/>
    </skos:Concept>
    <skos:Concept rdf:about="http://gams.uni-graz.at/thesaurus/parchment-glue">
        <skos:inScheme rdf:resource="http://gams.uni-graz.at/thesaurus/mss-materials"/>
        <skos:prefLabel xml:lang="de">Pergamentklebstoff</skos:prefLabel>
        <skos:prefLabel xml:lang="en">Parchment glue</skos:prefLabel>
        <skos:broader rdf:resource="http://gams.uni-graz.at/thesaurus/proteinaceous"/>
    </skos:Concept>
    <skos:Concept rdf:about="http://gams.uni-graz.at/thesaurus/carbohydrates">
        <skos:inScheme rdf:resource="http://gams.uni-graz.at/thesaurus/mss-materials"/>
        <skos:prefLabel xml:lang="de">Kohlenhydrate-Bindemittel</skos:prefLabel>
        <skos:prefLabel xml:lang="en">Carbohydrates binding agents</skos:prefLabel>
        <skos:broader rdf:resource="http://gams.uni-graz.at/thesaurus/binding-agents"/>
    </skos:Concept>
    <skos:Concept rdf:about="http://gams.uni-graz.at/thesaurus/gums">
        <skos:inScheme rdf:resource="http://gams.uni-graz.at/thesaurus/mss-materials"/>
        <skos:prefLabel xml:lang="de">Gummen</skos:prefLabel>
        <skos:prefLabel xml:lang="en">Gums</skos:prefLabel>
        <skos:broader rdf:resource="http://gams.uni-graz.at/thesaurus/carbohydrates"/>
    </skos:Concept>
<!--    ############ COLORANTS and Inks ########### -->
    <skos:Concept rdf:about="http://gams.uni-graz.at/thesaurus/colorants">
        <skos:inScheme rdf:resource="http://gams.uni-graz.at/thesaurus/mss-materials"/>
        <skos:prefLabel xml:lang="de">Farbmittel, Tinten und Metalle</skos:prefLabel>
        <skos:prefLabel xml:lang="en">Colorants, Inks and Metals</skos:prefLabel>
        <skos:altLabel xml:lang="en">Colourants, Inks and Metals</skos:altLabel>
        <skos:definition xml:lang="de">Dieses SKOS Dokument präsentiert eine Klassifikation von Farbmitteln (farbgebende Substanzen), Tinte und Metalle, die in mittelalterlichen Handschriften verwendet worden sind.
            Farbmittel ist eine Sammelbezeichnung für alle farbgebenden Stoffe, die nach ihrer 1) Löslichkeit: in Pigmente (unlöslich) und Farbstoffe (löslich); 2) chemischen Struktur in anorganische (Mineralien und Erde) und organische (hergestellt aus pflanzlichen und tierischen Produkten); 3)Herkunft: in natürliche und synthetische oder 4) nach der Farbqualität in rote, weiße, grüne usw. eingeteilt werden können. In dieser Klassifikation werden Farbmittel nach der Farbe eingeteilt.
        </skos:definition>
        <skos:definition xml:lang="en">The following SKOS document is meant as a classification of colourants (colouring materials), inks and metals used in mediaeval manuscripts. One can differentiate colourants based on their: 1) solubility: in this case we speak of pigments (insoluble) and dyes (soluble); 2) chemical structure: organic (made from plants and animal products) and inorganic (minerals and earths); 3) method of preparation: natural and synthetic; 4) colour: red, white, green etc. In this qualification we group colourants based on colour.
        </skos:definition>
        <skos:broader rdf:resource="http://gams.uni-graz.at/thesaurus/materials_role"/>
    </skos:Concept>
<!-- ################################## RED #######################-->
    <skos:Concept rdf:about="http://gams.uni-graz.at/thesaurus/red-colorants">
        <skos:inScheme rdf:resource="http://gams.uni-graz.at/thesaurus/mss-materials"/>
        <skos:prefLabel xml:lang="de">Rote Farbmittel</skos:prefLabel>
        <skos:prefLabel xml:lang="en">Red colorants</skos:prefLabel>
        <skos:example>https://upload.wikimedia.org/wikipedia/commons/8/82/Red_tints_and_shades.svg</skos:example>
        <skos:broader rdf:resource="http://gams.uni-graz.at/thesaurus/colorants"/>
    </skos:Concept>   
    
    <skos:Concept rdf:about="http://gams.uni-graz.at/thesaurus/red-ochre">
        <skos:inScheme rdf:resource="http://gams.uni-graz.at/thesaurus/mss-materials"/>
        <skos:prefLabel xml:lang="de">Roter Ocker</skos:prefLabel>
        <skos:altLabel xml:lang="de">Eisenoxyd</skos:altLabel>
        <skos:altLabel xml:lang="de">Rote Erde</skos:altLabel>
        <skos:prefLabel xml:lang="en">Red ochre</skos:prefLabel>
        <skos:altLabel xml:lang="en">Iron oxide red pigments</skos:altLabel>
        <skos:altLabel xml:lang="en">Red earth</skos:altLabel>
        <skos:definition xml:lang="en"> The term red ochre (ocher) or red earth describes various kinds of iron oxide pigments, which occur as natural clay rocks and soils. Helwig (2007) provides a list of historical names for iron oxide pigments such as Rubica, Sinopis etc. 
            Red ochres are prepared by washing the mineral in order to separate it from sand and other impurities. After draying it is being ground. The pigments are stable and are used for book illustrations, icons, indoor and outdoor frescos. Red ochre varied enormously in colour (Clemens 2007).
        Through extensive heat one can also change yellow ochre to red or burnt ochre. The process is described by ancient Roman authors and also known throughout the Middle Ages. By roasting (calcination) one could also obtain a richer more opaque earth colour (Clemens 2007).</skos:definition>
        <skos:definition rdf:parseType="Resource">
            <rdf:value>References</rdf:value>
            <dct:bibliographicCitation>Eastaugh, Nicholas, Valentine Walsh, Tracey Chaplin, and Ruth Siddall. Pigment Compendium: A Dictionary and Optical Microscopy of Historical Pigments. Amsterdam: Elsevier, Butterworth-Heinemann, 2008, pp. 326-327.</dct:bibliographicCitation>
            <dct:bibliographicCitation>Helwig, Kate. ‘Iron Oxide Pigments’. In Artists’ Pigments. A Handbook of Their History and Characteristics, edited by Barbara H. Berrie, 4:39–109. Washington: National Gallery of Art, 2007.</dct:bibliographicCitation>
            <dct:bibliographicCitation>Kühn, Hermann. Reclams Handbuch der künstlerischen Techniken. Vol. 1. Farbmittel, Buchmalerei, Tafel-und Leinwandmalerei. 3 vols. Stuttgart: Reclam, 1984, pp. 77-78.</dct:bibliographicCitation>
            <dct:bibliographicCitation>Clemens, Raymond, and Timothy Graham. Introduction to Manuscript Studies. Ithaca, NY: Cornell University Press, 2007.</dct:bibliographicCitation>
            <dct:bibliographicCitation>https://colourlex.com/project/red-ochre/</dct:bibliographicCitation>     
            <dct:bibliographicCitation>Spectra by A. Cosentino, Cultural Heritage Science Open Source (CHSOS): https://chsopensource.org/red-ochre-k-11574/</dct:bibliographicCitation>
        </skos:definition>
        <skos:example>https://upload.wikimedia.org/wikipedia/commons/e/e9/Drei_verschiedene_Ockert%C3%B6ne.JPG</skos:example>
        <skos:related rdf:resource="http://gams.uni-graz.at/thesaurus/iron"/>
        <skos:related rdf:resource="http://gams.uni-graz.at/thesaurus/oxygen"/>
        <skos:broader rdf:resource="http://gams.uni-graz.at/thesaurus/red-colorants"/>
    </skos:Concept>
    <skos:Concept rdf:about="http://gams.uni-graz.at/thesaurus/hematite">
        <skos:inScheme rdf:resource="http://gams.uni-graz.at/thesaurus/mss-materials"/>
        <skos:prefLabel xml:lang="de">Hämatit</skos:prefLabel>
        <skos:prefLabel xml:lang="en">Hematite</skos:prefLabel>
        <skos:definition xml:lang="en">Hematite is a mineral containing iron oxide (Fe2O3). In contrast to other pigments made of iron oxide such as red earths and ochers, the hematite pigment is produced by crushing the mineral (Helwig 2007).
            Cennini was the first artist writer to refer to hematite as a pigment (Helwig 2007). For manuscript illuminations dark red hematite was used either alone or mixed with orpiment to produce a brownish colour; the pigment was identified in a sixteenth-century miniature from Iran (Ricciardi et al. 2016).</skos:definition>
        <skos:definition rdf:parseType="Resource">
            <rdf:value>References</rdf:value>
            <dct:bibliographicCitation>Ricciardi, Paola, and Kristine Rose Beers. ‘The Illuminators’ Palette’. In Colour : The Art and Science of Illuminated Manuscripts, edited by Stella Panayotova, Deirdre Elizabeth Jackson, and Paola Ricciardi, 27–73. Turnhout: Brepols, 2016.</dct:bibliographicCitation>
            <dct:bibliographicCitation>Helwig, Kate. ‘Iron Oxide Pigments’. In Artists’ Pigments. A Handbook of Their History and Characteristics, edited by Barbara H. Berrie, 4:39–109. Washington: National Gallery of Art, 2007.</dct:bibliographicCitation>  
            <dct:bibliographicCitation>Material Archiv https://materialarchiv.ch/de/ma:material_1711/</dct:bibliographicCitation>
        </skos:definition>
        <skos:example>https://upload.wikimedia.org/wikipedia/commons/f/f1/Quartz-Hematite-113680.jpg</skos:example>
        <skos:broader rdf:resource="http://gams.uni-graz.at/thesaurus/red-ochre"/>
    </skos:Concept>
    <skos:Concept rdf:about="http://gams.uni-graz.at/thesaurus/sinopia">
        <skos:inScheme rdf:resource="http://gams.uni-graz.at/thesaurus/mss-materials"/>
        <skos:prefLabel xml:lang="de">Sinopia</skos:prefLabel>
        <skos:prefLabel xml:lang="en">Sinoper</skos:prefLabel>
        <skos:altLabel xml:lang="en">Sinopia</skos:altLabel>
        <skos:altLabel xml:lang="en">Sinopis</skos:altLabel>
        <skos:definition xml:lang="en">Sinoper is an iron oxide pigment, a variety of high-quality red ochre that was traded from the Ionian Greek port Sinope in modern day Turkey (Eastaugh). Red an yellow earth were used in recipes for pigment mixtures found in Latin medieval texts. Sinopia is mentioned by the Mappae Claviculae as an ingredient together with siricum (red lead or minium) to produce a red colour similar to cinnabar (Helwig 2007).</skos:definition>
        <skos:definition rdf:parseType="Resource">
            <rdf:value>References</rdf:value>
            <dct:bibliographicCitation>Eastaugh, Nicholas, Valentine Walsh, Tracey Chaplin, and Ruth Siddall. Pigment Compendium: A Dictionary and Optical Microscopy of Historical Pigments. Amsterdam: Elsevier, Butterworth-Heinemann, 2008, pp. 349-350.</dct:bibliographicCitation>
            <dct:bibliographicCitation>Helwig, Kate. ‘Iron Oxide Pigments’. In Artists’ Pigments. A Handbook of Their History and Characteristics, edited by Barbara H. Berrie, 4:39–109. Washington: National Gallery of Art, 2007.</dct:bibliographicCitation>
        </skos:definition>
        <skos:example></skos:example>
        <skos:related rdf:resource="http://gams.uni-graz.at/thesaurus/iron"/>
        <skos:related rdf:resource="http://gams.uni-graz.at/thesaurus/oxygen"/>
        <skos:broader rdf:resource="http://gams.uni-graz.at/thesaurus/red-ochre"/>
    </skos:Concept>    
    <skos:Concept rdf:about="http://gams.uni-graz.at/thesaurus/cinnabar">
        <skos:inScheme rdf:resource="http://gams.uni-graz.at/thesaurus/mss-materials"/>
        <skos:prefLabel xml:lang="de">Zinnober</skos:prefLabel>
        <skos:altLabel xml:lang="de">Cinnabarit</skos:altLabel>
        <skos:prefLabel xml:lang="en">Cinnabar</skos:prefLabel>
        <skos:altLabel xml:lang="en">Cinnabarite</skos:altLabel>
        <skos:altLabel xml:lang="de">Synthetischer Zinnober</skos:altLabel>
        <skos:altLabel xml:lang="de">Quicksilberzinnober</skos:altLabel>
        <skos:altLabel xml:lang="de">Vermillion</skos:altLabel>
        <skos:altLabel xml:lang="en">Vermilion</skos:altLabel>
        <skos:altLabel xml:lang="en">Vermillion</skos:altLabel>
        <skos:example>https://upload.wikimedia.org/wikipedia/commons/e/e5/Cinnabarit_01.jpg</skos:example>
        <skos:definition xml:lang="en">The natural cinnabar is a bright red inorganic pigment made of the mineral cinnabar (cinnabarite) containing mercury sulfide (HgS). The main source of cinnabar in Europe, according to Pliny the Elder (NH, XXXIII, 40) were the mercury deposits of Almadén in Spain. It was one of the most often used red pigments from Antiquity to the twentieth century.
            To make the pigment one had to ground and washed to remove as many mineral impurity as possible. Depending on its geological provenance, the pigment may contain the following elements: Sb, As, Se (Bi, Te, U, W) in the primary hydrothermal formation, or Ag, Au, Cu, Fe, Pb, Sn, Cr, Zn as secondary formation in the oxidation zone of ore deposits (Nöller, 2014). The elemental composition of different deposits is the most characteristic fingerprint for determining the local origin of the mercury ore (Nöller, 2012). For example the cinnabar imported from China has a characteristic light red colour due to the addition of antimony (Nöller, 2014).
            Cinnabar has also a synthetic analogue, referred to as vermilion. The two colourant are not always possible to distinguish analytically, since they have the same chemical composition (Nöller, 2013). To make vermilion, according to Theophilus (ch. 34), one took sulfur, broken into pieces, and added to it two equal parts of mercury. The mixtures was placed in a glass jar and buried in blazing coals until one hears a crashing inside, as mercury and sulfur combine. Cennini (ch. 40) suggested, there are many methods of preparation and receipts and advised his readers to buy vermilion from the druggists'.
            Cinnabar and vermilion are strong bright red pigments. However, when exposed to light for a long time and used with aqueous binders they may darken. This process depends also on the impurities of the red pigments and the additives found in neighbouring ones (Kühn 1984).</skos:definition>
        <skos:definition rdf:parseType="Resource">
            <rdf:value>References</rdf:value>
            <dct:bibliographicCitation>Nöller, Renate. ‘Cinnabar Reviewed: Characterization of the Red Pigment and Its Reactions’. Studies in Conservation 60 (2014): 1–9.</dct:bibliographicCitation>
            <dct:bibliographicCitation>Nöller, Renate. ‘Zinnoberlagerstätten im Vergleich. Auswahl historisch bedeutender Vorkommen’. Metalla, 19 (2012): 61–76.</dct:bibliographicCitation>
            <dct:bibliographicCitation>Nöller, Renate. ‘Zinnoberlagerstätten im Vergleich. Auswahl historisch bedeutender Vorkommen’. Metalla, 19 (2012): 61–76.</dct:bibliographicCitation>
            <dct:bibliographicCitation>FitzHugh, Elisabeth West. ‘Red Lead and Minium’. In Artists’ Pigments: A Handbook of Their History and Characteristics, edited by Robert L. Feller, 1:109–39. Washington, D.C.: National Gallery of Art, 1986. https://www.nga.gov/content/dam/ngaweb/research/publications/pdfs/artists-pigments-vol1.pdf</dct:bibliographicCitation>
            <dct:bibliographicCitation>Kühn, Hermann. Reclams Handbuch der künstlerischen Techniken. Vol. 1. Farbmittel, Buchmalerei, Tafel-und Leinwandmalerei. 3 vols. Stuttgart: Reclam, 1984, pp. 20-21.</dct:bibliographicCitation>
            <dct:bibliographicCitation>Material archiv https://materialarchiv.ch/de/ma:material_888</dct:bibliographicCitation>
            <dct:bibliographicCitation>Cennini, Cennino. The Craftsman’s Handbook: The Italian "Il Libro Dell’ Arte. Edited by Daniel Varney Thompson. New York: Dover, 1933.</dct:bibliographicCitation>
            <dct:bibliographicCitation>Theophilus, Presbyter. On Divers Arts: The Foremost Medieval Treatise on Painting, Glassmaking and Metalwork. Translated by John G. Hawthorne. New York: Dover, 1979.</dct:bibliographicCitation>
            <dct:bibliographicCitation>Material archiv https://materialarchiv.ch/de/ma:material_1851</dct:bibliographicCitation>
            <dct:bibliographicCitation>ColourLex https://colourlex.com/project/vermilion/</dct:bibliographicCitation>
            <dct:bibliographicCitation>Spectra by A. Cosentino, Cultural Heritage Science Open Source (CHSOS): https://chsopensource.org/vermilion-k-10610/</dct:bibliographicCitation>
        </skos:definition>
        <skos:related rdf:resource="http://gams.uni-graz.at/thesaurus/sulfur"/>
        <skos:related rdf:resource="http://gams.uni-graz.at/thesaurus/mercury"/>
        <skos:broader rdf:resource="http://gams.uni-graz.at/thesaurus/red-colorants"/>
    </skos:Concept>
    
    <skos:Concept rdf:about="http://gams.uni-graz.at/thesaurus/minium">
        <skos:inScheme rdf:resource="http://gams.uni-graz.at/thesaurus/mss-materials"/>
        <skos:prefLabel xml:lang="de">Mennige</skos:prefLabel>
        <skos:altLabel xml:lang="de">Bleimennige</skos:altLabel>
        <skos:prefLabel xml:lang="en">Minium</skos:prefLabel>
        <skos:altLabel xml:lang="en">Red lead pigment</skos:altLabel>        
        <skos:definition xml:lang="en">Minium is a red lead oxide mineral of composition Pb3O4. The mineral minium occurs in small amounts as a bright red or orange powder or crust by lead ore deposits. Its synthetic analogue was already known in antiquity. Theophilus gives the following recipe: pour vinegar or urine over lead plates; after a month collect the white lead built over them, grind it and set it on blazing coals until it gets the desired red colour. The pigment was used in medieval manuscripts both alone and in combination with cinnabar or vermilion. Exposed on light for a long time, minium can corrode and turn to dark brown or black lead dioxide (PbO2) especially when it was used with aqueous binders (Kühn 1984).
        For a list with notable occurrences from Europe, the Near East, India and the Far East see FitzHugh (FitzHugh 1984).</skos:definition> 
        <skos:example>https://upload.wikimedia.org/wikipedia/commons/a/ae/Red_lead.jpg</skos:example>
        <skos:related rdf:resource="http://gams.uni-graz.at/thesaurus/oxygen"/>
        <skos:related rdf:resource="http://gams.uni-graz.at/thesaurus/lead"/>
        <skos:broader rdf:resource="http://gams.uni-graz.at/thesaurus/red-colorants"/>
        <skos:definition rdf:parseType="Resource">
            <rdf:value>References</rdf:value>
            <dct:bibliographicCitation>Kühn, Hermann. Reclams Handbuch der künstlerischen Techniken. Vol. 1. Farbmittel, Buchmalerei, Tafel-und Leinwandmalerei. 3 vols. Stuttgart: Reclam, 1984.</dct:bibliographicCitation>
            <dct:bibliographicCitation>FitzHugh, Elisabeth West. ‘Red Lead and Minium’. In Artists’ Pigments: A Handbook of Their History and Characteristics, edited by Robert L. Feller, 1:109–39. Washington, D.C.: National Gallery of Art, 1986. https://www.nga.gov/content/dam/ngaweb/research/publications/pdfs/artists-pigments-vol1.pdf</dct:bibliographicCitation>
            <dct:bibliographicCitation>Theophilus, Presbyter. On Divers Arts: The Foremost Medieval Treatise on Painting, Glassmaking and Metalwork. Translated by John G. Hawthorne. New York: Dover, 1979.</dct:bibliographicCitation>
            <dct:bibliographicCitation>Material archiv https://materialarchiv.ch/de/ma:material_944/</dct:bibliographicCitation>
            <dct:bibliographicCitation>ColourLex https://colourlex.com/project/red-lead/</dct:bibliographicCitation>
            <dct:bibliographicCitation>Spectra by A. Cosentino, Cultural Heritage Science Open Source (CHSOS): https://chsopensource.org/red-lead-k-42500/</dct:bibliographicCitation>
        </skos:definition>
    </skos:Concept>
    <skos:Concept rdf:about="http://gams.uni-graz.at/thesaurus/organic-reds">
        <skos:inScheme rdf:resource="http://gams.uni-graz.at/thesaurus/mss-materials"/>
        <skos:prefLabel xml:lang="de">Organische rote Farbmittel</skos:prefLabel>
        <skos:prefLabel xml:lang="en">Organic red colorants</skos:prefLabel>
        <skos:definition xml:lang="en">The most common organics red are madder, Brazil wood, kermes. Other red-purple organic pigments  are listed under 'Purple colorants'.
            Organic colourants can be used as a dye, or turned into lake pigments (e.g. Madder lake) which allows them to be stored for later use.</skos:definition>
        <skos:example></skos:example>
        <skos:broader rdf:resource="http://gams.uni-graz.at/thesaurus/red-colorants"/>
    </skos:Concept>
    <skos:Concept rdf:about="http://gams.uni-graz.at/thesaurus/madder">
        <skos:inScheme rdf:resource="http://gams.uni-graz.at/thesaurus/mss-materials"/>
        <skos:prefLabel xml:lang="de">Krapp</skos:prefLabel>
        <skos:altLabel xml:lang="de">Färberkrapp</skos:altLabel>
        <skos:prefLabel xml:lang="en">Madder</skos:prefLabel>
        <skos:altLabel xml:lang="en">Rubia tinctorum</skos:altLabel>
        <skos:definition xml:lang="en">Madder is an organic dye made from dried and threshed madder root (Rubia tinctorum). The plant is native to Europe, the Mediterranean and western Asia. The range of colours achieved from it varies from yellow through orange to red and purple or brown, depending on the production of the organic colourants and the inorganic substrates (Eastaugh, 2008).
            To produce the dye, the madder root was dried and threshed. In order to store the dye, artists usually incorporated it into clothlets rather than lakes (Clemens 2007). Theophilus mentioned the colourant when discussing methods to colour animal bones (book III, ch. 94). According to his recipe, the dried roots of the plant are pounded in a mortar. After mixing it with a strong alkaline solution it is put to boil in a pot.</skos:definition>
        <skos:example>https://upload.wikimedia.org/wikipedia/commons/a/a9/Krapplack.JPG</skos:example>
        <skos:definition rdf:parseType="Resource">
            <rdf:value>References</rdf:value>
            <dct:bibliographicCitation>Eastaugh, Nicholas, Valentine Walsh, Tracey Chaplin, and Ruth Siddall. Pigment Compendium: A Dictionary and Optical Microscopy of Historical Pigments. Amsterdam: Elsevier, Butterworth-Heinemann, 2008, pp. 250-251.</dct:bibliographicCitation>
            <dct:bibliographicCitation>Theophilus, Presbyter. On Divers Arts: The Foremost Medieval Treatise on Painting, Glassmaking and Metalwork. Translated by John G. Hawthorne. New York: Dover, 1979.</dct:bibliographicCitation>
            <dct:bibliographicCitation>Clemens, Raymond, and Timothy Graham. Introduction to Manuscript Studies. Ithaca, NY: Cornell University Press, 2007.</dct:bibliographicCitation>
            <dct:bibliographicCitation>Material archiv https://materialarchiv.ch/de/ma:material_2001/</dct:bibliographicCitation>
            <dct:bibliographicCitation>ColourLex https://colourlex.com/project/madder-lake/</dct:bibliographicCitation>
            
        </skos:definition>
        <skos:related rdf:resource="http://gams.uni-graz.at/thesaurus/oxygen"/>
        <skos:related rdf:resource="http://gams.uni-graz.at/thesaurus/carbon"/>
        <skos:related rdf:resource="http://gams.uni-graz.at/thesaurus/hydrogen"/>
        <skos:broader rdf:resource="http://gams.uni-graz.at/thesaurus/organic-reds"/>
    </skos:Concept>
    <skos:Concept rdf:about="http://gams.uni-graz.at/thesaurus/madder-lake">
        <skos:inScheme rdf:resource="http://gams.uni-graz.at/thesaurus/mss-materials"/>
        <skos:prefLabel xml:lang="de">Krapplack</skos:prefLabel>
        <skos:prefLabel xml:lang="en">Madder lake</skos:prefLabel>
        <skos:definition xml:lang="en">Red organic pigment made from dried and threshed madder root (Rubia tinctorum), with additive aluminum to prepare a lake.
            Modern preparation following a 19th-century recipe described by Kremer: the shredded and washed madder roots are boiled in an alum solution, then filtered through a cloth. Sodium carbonate is added to the cold madder solution and brought to boiling point. The liquid is then pumped through a high pressure filter system, so that the extracted pigment stays in the filters. After the filters are left to dry, the pigment is collected and can be further pounded to powder.</skos:definition>
        <skos:definition rdf:parseType="Resource">
            <rdf:value>References</rdf:value>
            <dct:bibliographicCitation>Eastaugh, Nicholas, Valentine Walsh, Tracey Chaplin, and Ruth Siddall. Pigment Compendium: A Dictionary and Optical Microscopy of Historical Pigments. Amsterdam: Elsevier, Butterworth-Heinemann, 2008, p. 251.</dct:bibliographicCitation>            
            <dct:bibliographicCitation>https://www.kremer-pigmente.com/elements/resources/products/files/madder-lake-production.pdf</dct:bibliographicCitation>
            <dct:bibliographicCitation>Material archiv https://materialarchiv.ch/de/ma:material_2001/</dct:bibliographicCitation>
            <dct:bibliographicCitation>ColourLex https://colourlex.com/project/madder-lake/</dct:bibliographicCitation>
            <dct:bibliographicCitation>Spectra by A. Cosentino, Cultural Heritage Science Open Source (CHSOS): https://chsopensource.org/madder-lake-k-372051/</dct:bibliographicCitation>
        </skos:definition>
        <skos:related rdf:resource="http://gams.uni-graz.at/thesaurus/oxygen"/>
        <skos:related rdf:resource="http://gams.uni-graz.at/thesaurus/carbon"/>
        <skos:related rdf:resource="http://gams.uni-graz.at/thesaurus/hydrogen"/>
        <skos:related rdf:resource="http://gams.uni-graz.at/thesaurus/aluminium"/>
        <skos:broader rdf:resource="http://gams.uni-graz.at/thesaurus/organic-reds"/>
    </skos:Concept>
    <skos:Concept rdf:about="http://gams.uni-graz.at/thesaurus/brazilin">
        <skos:inScheme rdf:resource="http://gams.uni-graz.at/thesaurus/mss-materials"/>
        <skos:prefLabel xml:lang="de">Brasilin</skos:prefLabel>
        <skos:altLabel xml:lang="de">Brasilholz</skos:altLabel>
        <skos:prefLabel xml:lang="en">Brazilin</skos:prefLabel>
        <skos:altLabel xml:lang="en">Brazilwood</skos:altLabel>
        <skos:altLabel xml:lang="en">Sappanwood</skos:altLabel>
        <skos:definition xml:lang="en">Ther term 'brazilwood' encompasses a group of brown-red wood of the genus Caesalpinia and Haematoxylum, from which one produces a red dye with the colouring matter brazilin (Eastaugh et al. 2008). The wood, harvested in Asia in the Middle Ages, was chopped into small pieces and rasped to facilitate oxidation. The organic dye is almost always used as a lake (see Brazilwood lake). Mixed with woad it gave a purple colourant, and with lead white - a bright rose one (Clemens 2007).</skos:definition>
        <skos:definition rdf:parseType="Resource">
            <rdf:value>References</rdf:value>
            <dct:bibliographicCitation>Eastaugh, Nicholas, Valentine Walsh, Tracey Chaplin, and Ruth Siddall. Pigment Compendium: A Dictionary and Optical Microscopy of Historical Pigments. Amsterdam: Elsevier, Butterworth-Heinemann, 2008, p. 251.</dct:bibliographicCitation> 
            <dct:bibliographicCitation>Material archiv https://materialarchiv.ch/de/ma:material_2183/</dct:bibliographicCitation>          
        </skos:definition>
        <skos:related rdf:resource="http://gams.uni-graz.at/thesaurus/oxygen"/>
        <skos:related rdf:resource="http://gams.uni-graz.at/thesaurus/carbon"/>
        <skos:related rdf:resource="http://gams.uni-graz.at/thesaurus/hydrogen"/>
        <skos:broader rdf:resource="http://gams.uni-graz.at/thesaurus/organic-reds"/>
    </skos:Concept>
    <skos:Concept rdf:about="http://gams.uni-graz.at/thesaurus/brazilin-lake">
        <skos:inScheme rdf:resource="http://gams.uni-graz.at/thesaurus/mss-materials"/>
        <skos:prefLabel xml:lang="de">Brasilinlack</skos:prefLabel>
        <skos:prefLabel xml:lang="en">Brazilin lake</skos:prefLabel>
        <skos:definition xml:lang="en">The organic dye extracted from brazilwood was almost always used as a lake. It seems to have been rarely use, as relatively few identifications of brazilwood-based pigments have been made, including some 15th-century French manuscripts (Eastaugh et al. 2008).</skos:definition>
        <skos:definition rdf:parseType="Resource">
            <rdf:value>References</rdf:value>
            <dct:bibliographicCitation>Eastaugh, Nicholas, Valentine Walsh, Tracey Chaplin, and Ruth Siddall. Pigment Compendium: A Dictionary and Optical Microscopy of Historical Pigments. Amsterdam: Elsevier, Butterworth-Heinemann, 2008, p. 251.</dct:bibliographicCitation>                      
        </skos:definition>
        <skos:related rdf:resource="http://gams.uni-graz.at/thesaurus/oxygen"/>
        <skos:related rdf:resource="http://gams.uni-graz.at/thesaurus/carbon"/>
        <skos:related rdf:resource="http://gams.uni-graz.at/thesaurus/hydrogen"/>
        <skos:related rdf:resource="http://gams.uni-graz.at/thesaurus/calcium"/>
        <skos:broader rdf:resource="http://gams.uni-graz.at/thesaurus/organic-reds"/>
    </skos:Concept>
    <skos:Concept rdf:about="http://gams.uni-graz.at/thesaurus/kermes">
        <skos:inScheme rdf:resource="http://gams.uni-graz.at/thesaurus/mss-materials"/>
        <skos:prefLabel xml:lang="de">Kermes</skos:prefLabel>
        <skos:altLabel xml:lang="de">Cochenille</skos:altLabel>
        <skos:prefLabel xml:lang="en">Kermes</skos:prefLabel>
        <skos:altLabel xml:lang="en">Carmine</skos:altLabel>
        <skos:altLabel xml:lang="en">Cochineal</skos:altLabel>
        <skos:altLabel xml:lang="en">Crimson</skos:altLabel>
        <skos:definition xml:lang="en">Kermes is one of the oldest organic colorants. The red dyestuff is prepared from the larvae of various species of scale insects: cochineal, native to North, Central and South America and kermes, which was native to the Mediterranean region (Schweppe et al. 1986). The so-called Armenian cochineal was produced from another insect species (Porphyrophora hamelii) native to the Middle East and central Asia. The pigment was used for illuminated Armenian manuscripts (Phipps 2010). Another insect known as Polish cochineal (Porphyrophora polonica) was also used for producing red dye. Insects from the genus Porphyrophora are native to sandy areas in central and eastern Europe, Ukraine, Caucasus, Turkistan and western Siberia (Phipps 2010).
            The insect cases and larvae were collected together with the twig on which they had clustered, leading sometimes to the false conclusion that the dye derived from the leaves of trees (Eastaugh et al. 2008). 
            The dried insects had to be boiled in water in order to extract the carminic or kermesic acid. The dye was prepared then by precipitation of the extract from previously dyed material. To preserve the dye one had to add a mordant or mineral salt (aluminum sulfate) turning the dye to a lake. Cochineal has a naturally bright pink hue; using other additives (acids and alkali) however, one could achieve a deep crimson, purple or even black colour (Phipps 2010). 
             Cochineal could be extremely expensive. In the second half of the sixteenth century, kermes was largely replaced by the much cheaper chochineal made from female insects harvested from cactus plants in the New World (Clemens 2007; Phipps 2010).</skos:definition>
        <skos:definition rdf:parseType="Resource">
            <rdf:value>References</rdf:value>
            <dct:bibliographicCitation>Eastaugh, Nicholas, Valentine Walsh, Tracey Chaplin, and Ruth Siddall. Pigment Compendium: A Dictionary and Optical Microscopy of Historical Pigments. Amsterdam: Elsevier, Butterworth-Heinemann, 2008, pp. 216-217.</dct:bibliographicCitation>
            <dct:bibliographicCitation>Schweppe, Helmut, and Heinz Roosen-Runge. ‘Carmine - Cochineal Carmine and Kermes Carmine’. In Artists’ Pigments: A Handbook of Their History and Characteristics, edited by Robert L. Feller, 1:255–83. Washington, D.C.: National Gallery of Art, 1986.</dct:bibliographicCitation>
            <dct:bibliographicCitation>Clemens, Raymond, and Timothy Graham. Introduction to Manuscript Studies. Ithaca, NY: Cornell University Press, 2007.</dct:bibliographicCitation>
            <dct:bibliographicCitation>Phipps, Elena. ‘Cochineal Red: The Art History of a Color’. The Metropolitan Museum of Art Bulletin 67, no. 3 (2010): 1–48.</dct:bibliographicCitation>
            <dct:bibliographicCitation>ColourLex https://colourlex.com/project/carmine/</dct:bibliographicCitation>
        </skos:definition>
        <skos:example>https://upload.wikimedia.org/wikipedia/commons/2/21/Kermes_-_Neve_Tzuf.jpg</skos:example>
        <skos:related rdf:resource="http://gams.uni-graz.at/thesaurus/oxygen"/>
        <skos:related rdf:resource="http://gams.uni-graz.at/thesaurus/carbon"/>
        <skos:related rdf:resource="http://gams.uni-graz.at/thesaurus/hydrogen"/>
        <skos:broader rdf:resource="http://gams.uni-graz.at/thesaurus/organic-reds"/>
    </skos:Concept>
    <skos:Concept rdf:about="http://gams.uni-graz.at/thesaurus/kermes-lake">
        <skos:inScheme rdf:resource="http://gams.uni-graz.at/thesaurus/mss-materials"/>
        <skos:prefLabel xml:lang="de">Kermeslack</skos:prefLabel>
        <skos:prefLabel xml:lang="en">Kermes lake</skos:prefLabel>
        <skos:altLabel xml:lang="en">Carmine lake</skos:altLabel>
        <skos:definition xml:lang="en">A red lack produced by adding alum (aluminium (Al)) to the red dyestuff is prepared from the larvae of various species of scale insects: cochineal, native of North, Central and South America and kermes, which was native in the Mediterranean region (Schweppe et al. 1986).
            It produced a rich scarlet red that was extremely expensive. In the second half of the sixteenth century, kermes was largely replaced by the much cheaper chochineal made from female insects harvested from cactus plants in the New World (Clemens 2007).</skos:definition>
        <skos:definition rdf:parseType="Resource">
            <rdf:value>References</rdf:value>
            <dct:bibliographicCitation>Eastaugh, Nicholas, Valentine Walsh, Tracey Chaplin, and Ruth Siddall. Pigment Compendium: A Dictionary and Optical Microscopy of Historical Pigments. Amsterdam: Elsevier, Butterworth-Heinemann, 2008, pp. 216-217.</dct:bibliographicCitation>
            <dct:bibliographicCitation>Schweppe, Helmut, and Heinz Roosen-Runge. ‘Carmine - Cochineal Carmine and Kermes Carmine’. In Artists’ Pigments: A Handbook of Their History and Characteristics, edited by Robert L. Feller, 1:255–83. Washington, D.C.: National Gallery of Art, 1986.</dct:bibliographicCitation>
            <dct:bibliographicCitation>Clemens, Raymond, and Timothy Graham. Introduction to Manuscript Studies. Ithaca, NY: Cornell University Press, 2007.</dct:bibliographicCitation>
            <dct:bibliographicCitation>Phipps, Elena. ‘Cochineal Red: The Art History of a Color’. The Metropolitan Museum of Art Bulletin 67, no. 3 (2010): 1–48.</dct:bibliographicCitation>
            <dct:bibliographicCitation>ColourLex https://colourlex.com/project/carmine/</dct:bibliographicCitation>
            <dct:bibliographicCitation>Spectra by A. Cosentino, Cultural Heritage Science Open Source (CHSOS): https://chsopensource.org/carmine-lake-k-42100/</dct:bibliographicCitation>
        </skos:definition>
        <skos:related rdf:resource="http://gams.uni-graz.at/thesaurus/oxygen"/>
        <skos:related rdf:resource="http://gams.uni-graz.at/thesaurus/carbon"/>
        <skos:related rdf:resource="http://gams.uni-graz.at/thesaurus/hydrogen"/>
        <skos:related rdf:resource="http://gams.uni-graz.at/thesaurus/aluminium"/>
        <skos:broader rdf:resource="http://gams.uni-graz.at/thesaurus/organic-reds"/>
    </skos:Concept>
    <skos:Concept rdf:about="http://gams.uni-graz.at/thesaurus/dragons_blood">
        <skos:inScheme rdf:resource="http://gams.uni-graz.at/thesaurus/mss-materials"/>
        <skos:prefLabel xml:lang="de">Drachenblut</skos:prefLabel>
        <skos:prefLabel xml:lang="en">Dragon's blood</skos:prefLabel>
        <skos:definition xml:lang="en">Dragon's blood is a brown-red natural dye produced from the resin exuded by the plant Pterocarpus draco L. or Dracoena draco L. Pliny referred to it as 'cinnabaris', saying it was imported from India(XXIX, 25). Cennini (Ch. XLIII) says the red pigment was used occasionally on parchment for illuminating.</skos:definition>
        <skos:definition rdf:parseType="Resource">
            <rdf:value>References</rdf:value>
            <dct:bibliographicCitation>Kühn, Hermann. Reclams Handbuch der künstlerischen Techniken. Vol. 1. Farbmittel, Buchmalerei, Tafel-und Leinwandmalerei. 3 vols. Stuttgart: Reclam, 1984, pp. 25, 81-82.</dct:bibliographicCitation>
            <dct:bibliographicCitation>Cennini, Cennino. The Craftsman’s Handbook: The Italian "Il Libro Dell’ Arte. Edited by Daniel Varney Thompson. New York: Dover, 1933.</dct:bibliographicCitation>
            <dct:bibliographicCitation>ColourLex https://colourlex.com/project/dragon-s-blood/</dct:bibliographicCitation>
        </skos:definition>
        <skos:example>https://commons.wikimedia.org/wiki/File:Dragon%27s_blood_(Daemomorops_draco).jpg</skos:example>
        <skos:related rdf:resource="http://gams.uni-graz.at/thesaurus/oxygen"/>
        <skos:related rdf:resource="http://gams.uni-graz.at/thesaurus/carbon"/>
        <skos:related rdf:resource="http://gams.uni-graz.at/thesaurus/hydrogen"/>
        <skos:broader rdf:resource="http://gams.uni-graz.at/thesaurus/organic-reds"/>
    </skos:Concept>
    <skos:Concept rdf:about="http://gams.uni-graz.at/thesaurus/lac_dye">
        <skos:inScheme rdf:resource="http://gams.uni-graz.at/thesaurus/mss-materials"/>
        <skos:prefLabel xml:lang="de">Lac Dye</skos:prefLabel>
        <skos:altLabel xml:lang="de">Färberlack</skos:altLabel>
        <skos:altLabel xml:lang="de">Gummilack</skos:altLabel>
        <skos:prefLabel xml:lang="en">Lac dye</skos:prefLabel>
        <skos:definition xml:lang="en">Lac is a red dye extracted from a resin secreted by lac insects (Kerria lacca) native to Asia and particularly India. The dye is known to be imported to the western Mediterranean from the eleventh century onwards through Arab commercial routes. It was used as ink and pigment for illuminations either alone or together with other red pigments (vermilion) or with lead white (Castro et al. 2016). In Europe it was probably first imported as a dyestuff by the Catelans and Provencals about 1220; lac was also used as a lake pigment testified by a recipe in De Diversis Coloribus (Eastaugh et al. 2008).</skos:definition>
        <skos:definition rdf:parseType="Resource">
            <rdf:value>References</rdf:value>
            <dct:bibliographicCitation>Eastaugh, Nicholas, Valentine Walsh, Tracey Chaplin, and Ruth Siddall. Pigment Compendium: A Dictionary and Optical Microscopy of Historical Pigments. Amsterdam: Elsevier, Butterworth-Heinemann, 2008.</dct:bibliographicCitation>
            <dct:bibliographicCitation>Castro, Rita, Adelaide Miranda, and Maria Melo. ‘Interpreting Lac Dye in Medieval Written Sources: New Knowledge from the Reconstruction of Recipes Relating to Illuminations in Portuguese Manuscripts’, 88–99, 2016. https://www.researchgate.net/publication/298429268_Interpreting_lac_dye_in_medieval_written_sources_new_knowledge_from_the_reconstruction_of_recipes_relating_to_illuminations_in_Portuguese_manuscripts</dct:bibliographicCitation>
            <dct:bibliographicCitation>Material Archiv https://materialarchiv.ch/de/ma:material_1013</dct:bibliographicCitation>
            <dct:bibliographicCitation>Spectra by A. Cosentino, Cultural Heritage Science Open Source (CHSOS): https://chsopensource.org/lac-dye-k-36020/</dct:bibliographicCitation>
        </skos:definition>
        <skos:example>https://commons.wikimedia.org/wiki/File:Lac_as_a_natural_dye.jpg</skos:example>
        <skos:related rdf:resource="http://gams.uni-graz.at/thesaurus/oxygen"/>
        <skos:related rdf:resource="http://gams.uni-graz.at/thesaurus/carbon"/>
        <skos:related rdf:resource="http://gams.uni-graz.at/thesaurus/hydrogen"/>
        <skos:broader rdf:resource="http://gams.uni-graz.at/thesaurus/organic-reds"/>
    </skos:Concept>
    <skos:Concept rdf:about="http://gams.uni-graz.at/thesaurus/safflower">
        <skos:inScheme rdf:resource="http://gams.uni-graz.at/thesaurus/mss-materials"/>
        <skos:prefLabel xml:lang="de">Safflor</skos:prefLabel>
        <skos:altLabel xml:lang="de">Färberdistel</skos:altLabel>
        <skos:prefLabel xml:lang="en">Safflower</skos:prefLabel>
        <skos:altLabel xml:lang="en">Carthamin</skos:altLabel>
        <skos:altLabel xml:lang="en">Bastard saffron</skos:altLabel>
        <skos:definition xml:lang="en">Safflower is a red-orange-red dye obtained from the petals of the plant Carthamus tinctorius. The safflower plant originated in southern Asia (China, India, Persia, also Egypt) and was cultivated during the Middle Ages in Italy, France and Spain (Eastaugh et al. 2008). Islamic recipes suggest it was very difficult to obtain (Medlej 2020).</skos:definition>
        <skos:definition rdf:parseType="Resource">
            <rdf:value>References</rdf:value>
            <dct:bibliographicCitation>Medlej, Joumana. Inks and Paints of the Middle East: A Handbook of Abbasid Art Technology. London: Majnouna, 2020.</dct:bibliographicCitation>
            <dct:bibliographicCitation>Eastaugh, Nicholas, Valentine Walsh, Tracey Chaplin, and Ruth Siddall. Pigment Compendium: A Dictionary and Optical Microscopy of Historical Pigments. Amsterdam: Elsevier, Butterworth-Heinemann, 2008.</dct:bibliographicCitation>
            <dct:bibliographicCitation>Material Archiv https://materialarchiv.ch/de/ma:material_1034/</dct:bibliographicCitation>
        </skos:definition>
        <skos:example>https://upload.wikimedia.org/wikipedia/commons/7/76/Tuerkischer_safran.jpg</skos:example>
        <skos:related rdf:resource="http://gams.uni-graz.at/thesaurus/oxygen"/>
        <skos:related rdf:resource="http://gams.uni-graz.at/thesaurus/carbon"/>
        <skos:related rdf:resource="http://gams.uni-graz.at/thesaurus/hydrogen"/>
        <skos:broader rdf:resource="http://gams.uni-graz.at/thesaurus/organic-reds"/>
    </skos:Concept>
    <!-- #############  YELLOW  #############  -->
    <skos:Concept rdf:about="http://gams.uni-graz.at/thesaurus/yellow-colorants">
        <skos:inScheme rdf:resource="http://gams.uni-graz.at/thesaurus/mss-materials"/>
        <skos:prefLabel xml:lang="de">Gelbe Farbmittel</skos:prefLabel>
        <skos:prefLabel xml:lang="en">Yellow colorants</skos:prefLabel>
        <skos:example>https://upload.wikimedia.org/wikipedia/commons/d/d2/Yellow_tints_and_shades.svg</skos:example>
        <skos:broader rdf:resource="http://gams.uni-graz.at/thesaurus/colorants"/>
    </skos:Concept>
    <skos:Concept rdf:about="http://gams.uni-graz.at/thesaurus/yellow-ochre">
        <skos:inScheme rdf:resource="http://gams.uni-graz.at/thesaurus/mss-materials"/>
        <skos:prefLabel xml:lang="de">Gelber Ocker</skos:prefLabel>
        <skos:prefLabel xml:lang="en">Yellow ochre</skos:prefLabel>
        <skos:altLabel xml:lang="en">Yellow ocher</skos:altLabel>
        <skos:altLabel xml:lang="en">Gold ochre</skos:altLabel>
        <skos:altLabel xml:lang="en">Limonite</skos:altLabel>
        <skos:definition xml:lang="en">Yellow ochre is a naturally occurring pigment produced from rocks and soils primarily composed of oxides and hydroxides of iron (geothite or lepidocrocite). There are deposits worldwide but they are infrequently pure depending of the geological occurrences of the material (Eastaugh et al. 2008).
            Ochres are prepared by washing the mineral in order to separate it from sand and other impurities. After drying, it is being ground. Ochre can be burnt to produce brown, red an violet shades (Eastaugh et al. 2008). The pigments are stable and are used for book illustrations, icons, indoor and outdoor frescos. Known and used already in the Palaeolithic, yellow ochres remained important pigments in Byzantine and mediaeval western art (Eastaugh et al. 2008).</skos:definition>
        <skos:definition rdf:parseType="Resource">
            <rdf:value>References</rdf:value>
            <dct:bibliographicCitation>Eastaugh, Nicholas, Valentine Walsh, Tracey Chaplin, and Ruth Siddall. Pigment Compendium: A Dictionary and Optical Microscopy of Historical Pigments. Amsterdam: Elsevier, Butterworth-Heinemann, 2008, pp. 407-408.</dct:bibliographicCitation>
            <dct:bibliographicCitation>Helwig, Kate. ‘Iron Oxide Pigments’. In Artists’ Pigments. A Handbook of Their History and Characteristics, edited by Barbara H. Berrie, 4:39–109. Washington: National Gallery of Art, 2007.</dct:bibliographicCitation>
            <dct:bibliographicCitation>ColourLex https://colourlex.com/project/yellow-ochre/</dct:bibliographicCitation>
            <dct:bibliographicCitation>Material Archiv https://materialarchiv.ch/de/ma:material_1119/</dct:bibliographicCitation>           <dct:bibliographicCitation>Spectra by A. Cosentino, Cultural Heritage Science Open Source (CHSOS): https://chsopensource.org/yellow-ochre-k-40010/</dct:bibliographicCitation>
        </skos:definition>
        <skos:example></skos:example>
        <skos:related rdf:resource="http://gams.uni-graz.at/thesaurus/oxygen"/>
        <skos:related rdf:resource="http://gams.uni-graz.at/thesaurus/iron"/>
        <skos:broader rdf:resource="http://gams.uni-graz.at/thesaurus/yellow-colorants"/>
    </skos:Concept>
    <skos:Concept rdf:about="http://gams.uni-graz.at/thesaurus/orpiment">
        <skos:inScheme rdf:resource="http://gams.uni-graz.at/thesaurus/mss-materials"/>
        <skos:prefLabel xml:lang="de">Auripigment / Realgar</skos:prefLabel>
        <skos:altLabel xml:lang="de">Arsenblende</skos:altLabel>
        <skos:altLabel xml:lang="de">Gelbe Arsenblende</skos:altLabel>
        <skos:altLabel xml:lang="de">Rauschgelb</skos:altLabel>
        <skos:altLabel xml:lang="de">Operment / Realgar</skos:altLabel>
        <skos:prefLabel xml:lang="en">Orpiment / Realgar</skos:prefLabel>
        <skos:definition xml:lang="en">Orpiment is one of the most common yellow pigments identified in manuscripts (Panayotova 2016). It is a natural occurring yellow or greenish yellow mineral containing sulfide of arsenic (arsenic trisulfide: As2S3). Both orpiment and realgar, a closely related red-orange mineral (As4S4), are found as a massive encrusting or granular deposits; often the two are found together (Kühn 1984). In antiquity and the Middle Ages deposits were limited to Hungary, Macedonia and Asia Minor (Panayotova 2020). According to Thompson (1956) orpiment was imported into Europe in the Middle Ages mainly from Asia Minor. The synthetic form of orpiment was known already in the Middle Ages (Cennini, ch. 47). It was prepared either by heating or by precipitating a mixture of sulfur and arsenic by sublimation.
            Due to its toxicity the pigments have poisonous fumes and foul smell, making it unpleasant to work with. Cennini (ch. XLVIII) warns for its poisonous character. They can also react with copper and lead-based pigments, and particularly silver, to blacken them - a reason why they should be used in isolation from such pigments as in the case of heraldic blazonry (Naples MS; Eastaugh et al. 2008; Panayotova 2020). Orpiment was also used in mixture with indigo or azurite to produce green, as well as with red iron oxide to produce various shades of orange or pinkish brown (FitzHugh 1997).
        </skos:definition>
        <skos:definition rdf:parseType="Resource">
            <rdf:value>References</rdf:value>
            <dct:bibliographicCitation>Panayotova, Stella. ‘Painting Materials and Techniques in Western Illuminated  Manuscripts c. 600 -c. 1600’. In The Art and Science of Illuminated Manuscripts: A Handbook, edited by Stella Panayotova, 127–70. Turnhout: Brepols, 2020.</dct:bibliographicCitation>
            <dct:bibliographicCitation>FitzHugh, Elisabeth West. ‘Orpiment and Realgar’. In Artists’ Pigments: A Handbook of Their History and Characteristics, edited by Elisabeth West FitzHugh, Vol. 3. Washington: National Gallery of Art, 1997. https://www.nga.gov/content/dam/ngaweb/research/publications/pdfs/artists-pigments-vol3.pdf.</dct:bibliographicCitation>
            <dct:bibliographicCitation>Eastaugh, Nicholas, Valentine Walsh, Tracey Chaplin, and Ruth Siddall. Pigment Compendium: A Dictionary and Optical Microscopy of Historical Pigments. Amsterdam: Elsevier, Butterworth-Heinemann, 2008.</dct:bibliographicCitation>
            <dct:bibliographicCitation>Kühn, Hermann. Reclams Handbuch der künstlerischen Techniken. Vol. 1. Farbmittel, Buchmalerei, Tafel-und Leinwandmalerei. 3 vols. Stuttgart: Reclam, 1984.</dct:bibliographicCitation>
            <dct:bibliographicCitation>Panayotova, Stella, Deirdre Elizabeth Jackson, and Paola Ricciardi, eds. Colour : The Art and Science of Illuminated Manuscripts. Turnhout: Brepols, 2016.</dct:bibliographicCitation>
            <dct:bibliographicCitation>Thompson, Daniel Varney. The Materials and Techniques of Medieval Painting. Edited by Bernard Berenson. New York: Dover Publications, 1956.</dct:bibliographicCitation>
            <dct:bibliographicCitation>Cennini, Cennino. The Craftsman’s Handbook: The Italian "Il Libro Dell’ Arte. Edited by Daniel Varney Thompson. New York: Dover, 1933.</dct:bibliographicCitation>
            <dct:bibliographicCitation>Material archiv https://materialarchiv.ch/de/ma:material_887/</dct:bibliographicCitation>            
            <dct:bibliographicCitation>ColourLex https://colourlex.com/project/orpiment/</dct:bibliographicCitation>
            <dct:bibliographicCitation>ColourLex https://colourlex.com/project/realgar/</dct:bibliographicCitation>
            <dct:bibliographicCitation>https://www.mindat.org/min-3021.html</dct:bibliographicCitation>
            <dct:bibliographicCitation>Spectra by A. Cosentino, Cultural Heritage Science Open Source (CHSOS): https://chsopensource.org/orpiment-k-10700/</dct:bibliographicCitation>
        </skos:definition>
        <skos:example>https://upload.wikimedia.org/wikipedia/commons/4/46/Orpiment-148270.jpg</skos:example>
        <skos:related rdf:resource="http://gams.uni-graz.at/thesaurus/sulfur"/>
        <skos:related rdf:resource="http://gams.uni-graz.at/thesaurus/arsenic"/>
        <skos:broader rdf:resource="http://gams.uni-graz.at/thesaurus/yellow-colorants"/>
    </skos:Concept>    
    <skos:Concept rdf:about="http://gams.uni-graz.at/thesaurus/lead-tin-yellow">
        <skos:inScheme rdf:resource="http://gams.uni-graz.at/thesaurus/mss-materials"/>
        <skos:prefLabel xml:lang="de">Bleizinngelb</skos:prefLabel>
        <skos:prefLabel xml:lang="en">Lead-tin-yellow</skos:prefLabel>
        <skos:definition xml:lang="en">Lead-tin yellow is a synthetic pigment used almost exclusively in Europe or in places and cultures with specific trade with Europe (Eastaugh et al. 2008). According to its chemical composition there are two types: type I is a lead tin oxide (Pb2SnO4), type II is a silicate (Pb(Sn,Si)O3). Type I was more commonly used and identified in a large number of manuscripts and in paintings throughout Europe from the thirteenth until the first half of the eighteenth century. Lead-tin yellow of type II was used in the ancient glass industry; first seen in use by painters in thirteenth century Florence (Panayotova 2016).
        According to Kühn (1993) it can be assumed that the term giallorino, found in Italian treatises, and massicot, used in north-European texts, both mean lead-tin yellow.
        Lead-tin yellow was inexpensive, unaffected by light and unlike orpiment could be safely mixed with other pigments; it could however blacken over time (Clemens 2007).
        </skos:definition>
        <skos:definition rdf:parseType="Resource">
            <rdf:value>References</rdf:value>
            <dct:bibliographicCitation>Eastaugh, Nicholas, Valentine Walsh, Tracey Chaplin, and Ruth Siddall. Pigment Compendium: A Dictionary and Optical Microscopy of Historical Pigments. Amsterdam: Elsevier, Butterworth-Heinemann, 2008, pp. 238-239.</dct:bibliographicCitation>
            <dct:bibliographicCitation>Panayotova, Stella, Deirdre Elizabeth Jackson, and Paola Ricciardi, eds. Colour : The Art and Science of Illuminated Manuscripts. Turnhout: Brepols, 2016.</dct:bibliographicCitation>
            <dct:bibliographicCitation>Kühn, Hermann. ‘Lead-Tin Yellow’. In Artists’ Pigments: A Handbook of Their History and Characteristics, edited by Ashok Roy, 2:83–112. Washington, DC: National Gallery of Art, 1993. https://www.nga.gov/content/dam/ngaweb/research/publications/pdfs/artists-pigments-vol2.pdf.</dct:bibliographicCitation>
            <dct:bibliographicCitation>ColourLex https://colourlex.com/project/zinc-yellow/</dct:bibliographicCitation>
            <dct:bibliographicCitation>Material Archiv https://materialarchiv.ch/de/ma:material_938/</dct:bibliographicCitation>
            <dct:bibliographicCitation>Material Archiv https://materialarchiv.ch/de/ma:material_939/</dct:bibliographicCitation>
            <dct:bibliographicCitation>Spectra lead tin yellow I by A. Cosentino, Cultural Heritage Science Open Source (CHSOS): https://chsopensource.org/lead-tin-yellow-i-k-10100</dct:bibliographicCitation>
            <dct:bibliographicCitation>Spectra lead tin yellow II by A. Cosentino, Cultural Heritage Science Open Source (CHSOS): hhttps://chsopensource.org/lead-tin-yellow-ii-k-10120/</dct:bibliographicCitation>
        </skos:definition>
        <skos:example></skos:example>
        <skos:related rdf:resource="http://gams.uni-graz.at/thesaurus/oxygen"/>
        <skos:related rdf:resource="http://gams.uni-graz.at/thesaurus/tin"/>
        <skos:related rdf:resource="http://gams.uni-graz.at/thesaurus/lead"/>
        <skos:broader rdf:resource="http://gams.uni-graz.at/thesaurus/yellow-colorants"/>
    </skos:Concept>
    <skos:Concept rdf:about="http://gams.uni-graz.at/thesaurus/massicot">
        <skos:inScheme rdf:resource="http://gams.uni-graz.at/thesaurus/mss-materials"/>
        <skos:prefLabel xml:lang="de">Massicot</skos:prefLabel>
        <skos:altLabel xml:lang="de">Gelbe Bleiglätte</skos:altLabel>
        <skos:prefLabel xml:lang="en">Massicot</skos:prefLabel>
        <skos:altLabel xml:lang="en">Yellow litharge</skos:altLabel>
        <skos:definition xml:lang="en">Massicot refers today to a pale yellow pigment, a lead (II) oxide (PbO). The pigment can be produced from the natural mineral Massicotit or artificially by heating lead white long time over 300°C. The pigment was used in encaustinc, book illumination, as well as for colouring ceramics and glas (Material Archiv).
            Previously one thought the pigment was very common in medieval art, since one found often recipes for or references to 'massicot' or 'masticot' in medieval texts sources (Kühn 1984). The term massicot was at that time used to denote either the glaze on tin-enamelled ceramics or later (in association of tin and lead in ceramic glaze) a lead tin yellow pigment (Eastaught et al. 2008).</skos:definition>
        <skos:definition rdf:parseType="Resource">
            <rdf:value>References</rdf:value>
            <dct:bibliographicCitation>Eastaugh, Nicholas, Valentine Walsh, Tracey Chaplin, and Ruth Siddall. Pigment Compendium: A Dictionary and Optical Microscopy of Historical Pigments. Amsterdam: Elsevier, Butterworth-Heinemann, 2008, p. 337.</dct:bibliographicCitation>
            <dct:bibliographicCitation>Kühn, Hermann. Reclams Handbuch der künstlerischen Techniken. Vol. 1. Farbmittel, Buchmalerei, Tafel-und Leinwandmalerei. 3 vols. Stuttgart: Reclam, 1984.</dct:bibliographicCitation>
            <dct:bibliographicCitation>Material Archiv https://materialarchiv.ch/de/ma:material_940/</dct:bibliographicCitation>
            <dct:bibliographicCitation>Mindat https://www.mindat.org/min-2587.html</dct:bibliographicCitation>
        </skos:definition>
        <dct:bibliographicCitation>Spectra by A. Cosentino, Cultural Heritage Science Open Source (CHSOS): https://chsopensource.org/massicot-k-43010/</dct:bibliographicCitation> <skos:example>https://upload.wikimedia.org/wikipedia/commons/2/20/Massicot-177335.jpg</skos:example>
        <skos:related rdf:resource="http://gams.uni-graz.at/thesaurus/lead"/>
        <skos:related rdf:resource="http://gams.uni-graz.at/thesaurus/oxygen"/>
        <skos:broader rdf:resource="http://gams.uni-graz.at/thesaurus/yellow-colorants"/>
    </skos:Concept>
    <skos:Concept rdf:about="http://gams.uni-graz.at/thesaurus/mosaic-gold">
        <skos:inScheme rdf:resource="http://gams.uni-graz.at/thesaurus/mss-materials"/>
        <skos:prefLabel xml:lang="de">Mosaik-Gold</skos:prefLabel>
        <skos:altLabel xml:lang="de">Musivgold</skos:altLabel>
        <skos:prefLabel xml:lang="en">Mosaic gold</skos:prefLabel>
        <skos:definition xml:lang="en">Mosaic gold  is a tin(IV) sulfide used to imitate gilding. There are various recipes for its production; some call for melting equal parts tin, mercury, sulfur and ammonium chloride.  
            The earliest example of its use in manuscripts is from the second half of the thirteenth century produced in England and Italy (Panayotova 2020).
        </skos:definition>
        <skos:definition rdf:parseType="Resource">
            <rdf:value>References</rdf:value>
            <dct:bibliographicCitation>Eastaugh, Nicholas, Valentine Walsh, Tracey Chaplin, and Ruth Siddall. Pigment Compendium: A Dictionary and Optical Microscopy of Historical Pigments. Amsterdam: Elsevier, Butterworth-Heinemann, 2008.</dct:bibliographicCitation>
            <dct:bibliographicCitation>Panayotova, Stella. ‘Painting Materials and Techniques in Western Illuminated  Manuscripts c. 600 -c. 1600’. In The Art and Science of Illuminated Manuscripts: A Handbook, edited by Stella Panayotova, 127–70. Turnhout: Brepols, 2020.</dct:bibliographicCitation>
        </skos:definition>
        <skos:related rdf:resource="http://gams.uni-graz.at/thesaurus/tin"/>
        <skos:related rdf:resource="http://gams.uni-graz.at/thesaurus/mercury"/>
        <skos:related rdf:resource="http://gams.uni-graz.at/thesaurus/sulfur"/>
        <skos:broader rdf:resource="http://gams.uni-graz.at/thesaurus/yellow-colorants"/>
    </skos:Concept>
<!-- ################ORGANIC YELLOWS##########-->
    <skos:Concept rdf:about="http://gams.uni-graz.at/thesaurus/yellow-colorants-organic">
        <skos:inScheme rdf:resource="http://gams.uni-graz.at/thesaurus/mss-materials"/>
        <skos:prefLabel xml:lang="de">Organische gelbe Farbmittel</skos:prefLabel>
        <skos:prefLabel xml:lang="en">Organic yellow colorants</skos:prefLabel>
        <skos:definition xml:lang="en">Organic yellows can be derived from a variety of plants producing bright, vivid hues. As other organic colours, however, they are often not stable and lightfast (tend to fade when exposed to light). They cannot be securely distinguished using non-invasive analytical methods.</skos:definition>   
        <skos:broader rdf:resource="http://gams.uni-graz.at/thesaurus/yellow-colorants"/>
    </skos:Concept>
    <skos:Concept rdf:about="http://gams.uni-graz.at/thesaurus/gamboge">
        <skos:inScheme rdf:resource="http://gams.uni-graz.at/thesaurus/mss-materials"/>
        <skos:prefLabel xml:lang="de">Gummigutta</skos:prefLabel>
        <skos:altLabel xml:lang="de">Gamboge</skos:altLabel>
        <skos:prefLabel xml:lang="en">Gamboge</skos:prefLabel>
        <skos:definition xml:lang="en">Gamboge is an organic pigment derived from the resin of the Gacinia handburyi tree, which is native to Southeast Asia. The gum resin is produced in the form of a juice of leaves and shoots of the tree, which is then dried and rolled into cylinders (Kremer Pigmente). The organic pigment been identified in works from the Far East dating back to the eight century including an eighth-century illustrated scroll of the Ingakyo and an early twelfth-century Japanese hand scroll (Winter 1997). The pigment was also detected in thirteenth-century Armenian manuscripts (Merian et al. 1994). Its import in Europe started in the seventeenth century (Winter 1997).</skos:definition>
        <skos:definition rdf:parseType="Resource">
            <rdf:value>References</rdf:value>
            <dct:bibliographicCitation>Eastaugh, Nicholas, Valentine Walsh, Tracey Chaplin, and Ruth Siddall. Pigment Compendium: A Dictionary and Optical Microscopy of Historical Pigments. Amsterdam: Elsevier, Butterworth-Heinemann, 2008, p. 337.</dct:bibliographicCitation>
            <dct:bibliographicCitation>Winter, John. ‘Gamboge’. In Artists’ Pigments: A Handbook of Their History and Characteristics, edited by Elisabeth West FitzHugh, 3:143–55. Washington: National Gallery of Art, 1997. https://www.nga.gov/content/dam/ngaweb/research/publications/pdfs/artists-pigments-vol3.pdf.</dct:bibliographicCitation>
            <dct:bibliographicCitation>Merian, Sylvie, Thomas Mathews, and Mary Virginia Orna. ‘The Making of an Armenian Manuscript’. In Treasures in Heaven: Armenian Illuminated Manuscripts, edited by Thomas F. Mathews and Roger S. Wieck, 124–42. New York: Pierpont Morgan Library, 1994.</dct:bibliographicCitation>
            <dct:bibliographicCitation>Kremer Pigmente (accessed April 2022) https://www.kremer-pigmente.com/elements/resources/products/files/37050-37060e.pdf</dct:bibliographicCitation>
            <dct:bibliographicCitation>Spectra by A. Cosentino, Cultural Heritage Science Open Source (CHSOS): https://chsopensource.org/gamboge-k-37050/</dct:bibliographicCitation>
        </skos:definition>
        <skos:example>https://commons.wikimedia.org/wiki/File:Gummi_gutti1.JPG</skos:example>
        <skos:related rdf:resource="http://gams.uni-graz.at/thesaurus/oxygen"/>
        <skos:related rdf:resource="http://gams.uni-graz.at/thesaurus/carbon"/>
        <skos:related rdf:resource="http://gams.uni-graz.at/thesaurus/hydrogen"/>
        <skos:broader rdf:resource="http://gams.uni-graz.at/thesaurus/yellow-colorants-organic"/>
    </skos:Concept>
   <skos:Concept rdf:about="http://gams.uni-graz.at/thesaurus/indian_yellow">
        <skos:inScheme rdf:resource="http://gams.uni-graz.at/thesaurus/mss-materials"/>
        <skos:prefLabel xml:lang="de">Indischgelb</skos:prefLabel>
        <skos:prefLabel xml:lang="en">Indian yellow</skos:prefLabel>
       <skos:definition xml:lang="en">Indian yellow is a complex pigment consisting primarily of euxanthic acid salts (magnesium euxanthate and calcium euxanthate) (Eastaugh et al. 2008). The pigment was allegedly produced by the urine of cows, fed with indigestible mango leaves (Ploeger 2019).
           Indian yellow was not employed in Indian miniatures prior to the thirteenth and fourteenth centuries. Hence, scholars suppose it was introduced into India in the fifteenth century from Persia. Thereafter it was used in miniatures as for instance in Rajput-Mughal miniatures from the sixteenth to the nineteenth centuries. In Europe the pigment was used by some painters from the eighteenth century (Baer et al. 1986). Indian yellow was detected also using ultraviolet imaging in Islamic manuscripts dated from the thirteenth to the nineteenth centuries particularly those with Mughal influence (Knipe et al. 2018). 
           Indian yellow can be clearly distinguished by spectroscopic techniques (Ploeger 2019).</skos:definition>
        <skos:definition rdf:parseType="Resource">
            <rdf:value>References</rdf:value>
            <dct:bibliographicCitation>Eastaugh, Nicholas, Valentine Walsh, Tracey Chaplin, and Ruth Siddall. Pigment Compendium: A Dictionary and Optical Microscopy of Historical Pigments. Amsterdam: Elsevier, Butterworth-Heinemann, 2008.</dct:bibliographicCitation>               
            <dct:bibliographicCitation>Ploeger, R. et al. "Late 19th century accounts of Indian yellow: The analysis of samples from the Royal Botanic Gardens, Kew". Dyes and Pigments 160 (2019): 418–431. doi:10.1016/j.dyepig.2018.08.014.</dct:bibliographicCitation>
            <dct:bibliographicCitation>Baer, N.S., A. Joel, R.L. Feller, and N. Indictor. ‘Indian Yellow’. In Artists’ Pigments: A Handbook of Their History and Characteristics, edited by Robert L. Feller, 1:17–36. Washington, D.C.: National Gallery of Art, 1986.</dct:bibliographicCitation>
            <dct:bibliographicCitation>Knipe, Penley, Katherine Eremin, Marc Walton, Agnese Babini, and Georgina Rayner. ‘Materials and Techniques of Islamic Manuscripts’. Heritage Science 6, no. 1 (2018): 1–40. https://doi.org/10.1186/s40494-018-0217-y.</dct:bibliographicCitation>
            <dct:bibliographicCitation>Material Archiv https://materialarchiv.ch/de/ma:material_1014/</dct:bibliographicCitation>
            <dct:bibliographicCitation>ColourLex https://colourlex.com/project/indian-yellow/</dct:bibliographicCitation>
        </skos:definition>
       <skos:example>https://commons.wikimedia.org/wiki/File:Indisch-Gelb.jpg</skos:example> 
       <skos:related rdf:resource="http://gams.uni-graz.at/thesaurus/magnesium"/> 
       <skos:related rdf:resource="http://gams.uni-graz.at/thesaurus/oxygen"/>
       <skos:related rdf:resource="http://gams.uni-graz.at/thesaurus/carbon"/>
       <skos:related rdf:resource="http://gams.uni-graz.at/thesaurus/hydrogen"/>
       <skos:broader rdf:resource="http://gams.uni-graz.at/thesaurus/yellow-colorants-organic"/>
    </skos:Concept>
    <skos:Concept rdf:about="http://gams.uni-graz.at/thesaurus/weld">
        <skos:inScheme rdf:resource="http://gams.uni-graz.at/thesaurus/mss-materials"/>
        <skos:prefLabel xml:lang="de">Färber-Wau</skos:prefLabel>
        <skos:prefLabel xml:lang="en">Weld</skos:prefLabel>
        <skos:definition xml:lang="en">Weld is a natural dye made from the plant Reseda luteola, cultivated in Europe. It was widely used as a dye in mediaeval Europe (Eastaugh et al. 2008) and also mentioned in treaties on book illumination (Cennini for example referred to it as 'arzica' in ch. 50).  
            To produce the pigment one has to strew the whole dried plant in a wear solution of alum, precipitating it with the addition of calcium sulfate, eggshell or lead white (Eastaugh et al. 2008). It gave a lighfast yellow, which could be mixed with indigo to create green, with woad to make black, or with lead white to make it opaque (Clemens 2007).</skos:definition>
        <skos:definition rdf:parseType="Resource">
            <rdf:value>References</rdf:value>
            <dct:bibliographicCitation>Eastaugh, Nicholas, Valentine Walsh, Tracey Chaplin, and Ruth Siddall. Pigment Compendium: A Dictionary and Optical Microscopy of Historical Pigments. Amsterdam: Elsevier, Butterworth-Heinemann, 2008, pp. 400-401.</dct:bibliographicCitation>
            <dct:bibliographicCitation>Clemens, Raymond, and Timothy Graham. Introduction to Manuscript Studies. Ithaca, NY: Cornell University Press, 2007.</dct:bibliographicCitation>
            <dct:bibliographicCitation>Material Archiv https://materialarchiv.ch/de/ma:material_1039/</dct:bibliographicCitation>         
        </skos:definition>
        <skos:example>https://upload.wikimedia.org/wikipedia/commons/a/af/Wool_Dyed_with_Reseda._%281%29.jpg</skos:example>
        <skos:related rdf:resource="http://gams.uni-graz.at/thesaurus/oxygen"/>
        <skos:related rdf:resource="http://gams.uni-graz.at/thesaurus/hydrogen"/>
        <skos:broader rdf:resource="http://gams.uni-graz.at/thesaurus/yellow-colorants-organic"/>
    </skos:Concept>
    <skos:Concept rdf:about="http://gams.uni-graz.at/thesaurus/saffron">
        <skos:inScheme rdf:resource="http://gams.uni-graz.at/thesaurus/mss-materials"/>
        <skos:prefLabel xml:lang="de">Safran</skos:prefLabel>
        <skos:prefLabel xml:lang="en">Saffron</skos:prefLabel>
        <skos:definition xml:lang="en">Natural organic dye extracted from the stamens of the saffron crocus flower (crocus sativus). For producing the pigment they were mixed with alum. Saffron was labour intensive to harvest and expensive, but also appreciated for its golden hue and its quality to serve as a buffer to the corrosive properties of verdigris (Panayotova 2016).
            </skos:definition>
        <skos:definition rdf:parseType="Resource">
            <rdf:value>References</rdf:value>
            <dct:bibliographicCitation>Eastaugh, Nicholas, Valentine Walsh, Tracey Chaplin, and Ruth Siddall. Pigment Compendium: A Dictionary and Optical Microscopy of Historical Pigments. Amsterdam: Elsevier, Butterworth-Heinemann, 2008, p. 337.</dct:bibliographicCitation>
            <dct:bibliographicCitation>Panayotova, Stella, Deirdre Elizabeth Jackson, and Paola Ricciardi, eds. Colour : The Art and Science of Illuminated Manuscripts. Turnhout: Brepols, 2016.</dct:bibliographicCitation>
            <dct:bibliographicCitation>Material Archiv https://materialarchiv.ch/de/ma:material_1035/</dct:bibliographicCitation>         
            <dct:bibliographicCitation>Spectra by A. Cosentino, Cultural Heritage Science Open Source (CHSOS): https://chsopensource.org/saffron-k-37110/</dct:bibliographicCitation>
        </skos:definition>
        <skos:example>https://upload.wikimedia.org/wikipedia/commons/1/1c/Safran-Weinviertel_Niederreiter_2_Gramm_8285.jpg</skos:example>
        <skos:related rdf:resource="http://gams.uni-graz.at/thesaurus/oxygen"/>
        <skos:related rdf:resource="http://gams.uni-graz.at/thesaurus/hydrogen"/>
        <skos:broader rdf:resource="http://gams.uni-graz.at/thesaurus/yellow-colorants-organic"/>
    </skos:Concept>
    <skos:Concept rdf:about="http://gams.uni-graz.at/thesaurus/buckthorn-berries-yellow">
        <skos:inScheme rdf:resource="http://gams.uni-graz.at/thesaurus/mss-materials"/>
        <skos:prefLabel xml:lang="de">Kreuzdornbeeren (unreif)</skos:prefLabel>
        <skos:prefLabel xml:lang="en">Buckthorn unripe</skos:prefLabel>
        <skos:definition xml:lang="en">The yellow dye is made of various species of the Rhamnaceae family (most common species throughout Europe were the Rhamnus catharticus). As a lake the pigment was quite popular with a wide geographical production (Eastaugh et al. 2008).
            To get a yellow dye the berries must be unripe (ripe ones make a green colour). For producing the pigment they were mixed with alum.</skos:definition>
        <skos:definition rdf:parseType="Resource">
            <rdf:value>References</rdf:value>
            <dct:bibliographicCitation>Eastaugh, Nicholas, Valentine Walsh, Tracey Chaplin, and Ruth Siddall. Pigment Compendium: A Dictionary and Optical Microscopy of Historical Pigments. Amsterdam: Elsevier, Butterworth-Heinemann, 2008, p. 71.</dct:bibliographicCitation>
            <dct:bibliographicCitation>Material Archiv https://materialarchiv.ch/de/ma:material_2118/</dct:bibliographicCitation> </skos:definition>
        <skos:example>https://commons.wikimedia.org/wiki/File:Rhamnus_catharticus_leaves_and_fruit.jpg</skos:example>
        <skos:related rdf:resource="http://gams.uni-graz.at/thesaurus/oxygen"/>
        <skos:related rdf:resource="http://gams.uni-graz.at/thesaurus/hydrogen"/>
        <skos:broader rdf:resource="http://gams.uni-graz.at/thesaurus/yellow-colorants-organic"/>
    </skos:Concept>
    
<!--    ############# BLUE ###############-->
    <skos:Concept rdf:about="http://gams.uni-graz.at/thesaurus/blue-colorants">
        <skos:inScheme rdf:resource="http://gams.uni-graz.at/thesaurus/mss-materials"/>
        <skos:prefLabel xml:lang="de">Blaue Farbmittel</skos:prefLabel>
        <skos:prefLabel xml:lang="en">Blue colorants</skos:prefLabel>
        <skos:definition xml:lang="en">There are three main blues used in manuscript illumination in the middle ages: ultramarine, azurite and indigo. Recently one was able to detect also the use of Egyptian blue in some Anglo-Saxon manuscripts, as well as smalt in some fifteenth-century manuscripts from Venice.</skos:definition>
        <skos:example>https://upload.wikimedia.org/wikipedia/commons/7/7d/Blue_tints_and_shades.svg</skos:example>
        <skos:broader rdf:resource="http://gams.uni-graz.at/thesaurus/colorants"/>
    </skos:Concept>
    <skos:Concept rdf:about="http://gams.uni-graz.at/thesaurus/ultramarine">
        <skos:inScheme rdf:resource="http://gams.uni-graz.at/thesaurus/mss-materials"/>
        <skos:prefLabel xml:lang="de">Ultramarin</skos:prefLabel>
        <skos:altLabel xml:lang="en">Lapis lazuli</skos:altLabel>
        <skos:prefLabel xml:lang="en">Ultramarine</skos:prefLabel>
        <skos:definition xml:lang="en">Natural inorganic pigment made from the mineral lapis lazuli, complex sulfur-containing sodium-silicate (Na8–10Al6Si6O24S2–4). The mineral was found in the medieval period only in modern-day Afghanistan. Due to the long transportation and the labour-intensive process of production ultramarine was an expensive pigment. Ultramarine is a stable pigment and although it contains sulfur, it was regularly mixed with lead white without causing any blackening of the lead pigment (Plesters 1993).
            In antiquity lapis lazuli was used as a gem and decoration but there are no reference of its use as a pigment prior to the early middle ages (Kühn 1984). It has been identified in manuscripts from the tenth century onwards; from the early fourteenth century its use diminished as azurite became more prevalent (Panayotova 2020).
        Outside Europe ultramarine has been identified on Persian miniatures of the thirteenth and fourteenth centuries, on Chinese paintings of the tenth to eleventh century, in Indian mural paintings of the eleventh, twelfth and seventeenth centuries (Plesters 1993); in illuminations in Byzantine, Armenian manuscripts from the tenth century onwards, in Iranian manuscripts from the fourteenth to the seventeenth centuries, in Indian, Persian and Turkish manuscripts from the fifteenth century onwards (Merian et al. 1994).
        </skos:definition>
        <skos:definition rdf:parseType="Resource">
            <rdf:value>References</rdf:value>
            <dct:bibliographicCitation>Panayotova, Stella. ‘Painting Materials and Techniques in Western Illuminated  Manuscripts c. 600 -c. 1600’. In The Art and Science of Illuminated Manuscripts: A Handbook, edited by Stella Panayotova, 127–70. Turnhout: Brepols, 2020.
            </dct:bibliographicCitation>
            <dct:bibliographicCitation>Kühn, Hermann. Reclams Handbuch der künstlerischen Techniken. Vol. 1. Farbmittel, Buchmalerei, Tafel-und Leinwandmalerei. 3 vols. Stuttgart: Reclam, 1984, pp. 35-36, 93-95.</dct:bibliographicCitation>
            <dct:bibliographicCitation>Plesters, Joyce. ‘Ultramarine Blue, Natural and Artificial’. In Artists’ Pigments: A Handbook of Their History and Characteristics, edited by Ashok Roy, 2:37–65. Washington, DC: National Gallery of Art, 1993. https://www.nga.gov/content/dam/ngaweb/research/publications/pdfs/artists-pigments-vol2.pdf.</dct:bibliographicCitation>
            <dct:bibliographicCitation>Merian, Sylvie, Thomas Mathews, and Mary Virginia Orna. ‘The Making of an Armenian Manuscript’. In Treasures in Heaven: Armenian Illuminated Manuscripts, edited by Thomas F. Mathews and Roger S. Wieck, 124–42. New York: Pierpont Morgan Library, 1994.</dct:bibliographicCitation>
            <dct:bibliographicCitation>Material Archiv https://materialarchiv.ch/de/ma:material_940/</dct:bibliographicCitation>
            <dct:bibliographicCitation>ColourLex https://colourlex.com/project/ultramarine-natural/</dct:bibliographicCitation>
            <dct:bibliographicCitation>Mindat https://www.mindat.org/min-2357.html</dct:bibliographicCitation>
            <dct:bibliographicCitation>Spectra by A. Cosentino, Cultural Heritage Science Open Source (CHSOS): https://chsopensource.org/ultramarine-natural-k-10510/</dct:bibliographicCitation>
        </skos:definition>
        <skos:example>https://upload.wikimedia.org/wikipedia/commons/8/8a/Natural_ultramarine_pigment.jpg</skos:example>
        <skos:related rdf:resource="http://gams.uni-graz.at/thesaurus/aluminium"/>
        <skos:related rdf:resource="http://gams.uni-graz.at/thesaurus/kalium"/>
        <skos:related rdf:resource="http://gams.uni-graz.at/thesaurus/calcium"/>
        <skos:related rdf:resource="http://gams.uni-graz.at/thesaurus/sulfur"/>
        <skos:related rdf:resource="http://gams.uni-graz.at/thesaurus/silicon"/>
        <skos:related rdf:resource="http://gams.uni-graz.at/thesaurus/iron"/>
        <skos:broader rdf:resource="http://gams.uni-graz.at/thesaurus/blue-colorants"/>
    </skos:Concept>
    <skos:Concept rdf:about="http://gams.uni-graz.at/thesaurus/azurite">
        <skos:inScheme rdf:resource="http://gams.uni-graz.at/thesaurus/mss-materials"/>
        <skos:prefLabel xml:lang="de">Azurit</skos:prefLabel>
        <skos:altLabel xml:lang="de">Bergblau</skos:altLabel>
        <skos:altLabel xml:lang="de">Verditer</skos:altLabel>
        <skos:prefLabel xml:lang="en">Azurite</skos:prefLabel>
        <skos:altLabel xml:lang="en">Cyprian blue</skos:altLabel>
        <skos:altLabel xml:lang="en">Blue verditer</skos:altLabel>
        <skos:definition xml:lang="en">Azurite is a bright blue hydrated copper carbonate mineral (2 CuCO3·Cu(OH)2). The pigment has been prepared either from naturally occurring mineral or produced synthetically. Blue verditer, the synthetic form of azurite, was allegedly an accidental discovery in the seventeenth century (Eastaugh et al. 2008).
            Azurite was known already in antiquity and was the most used blue pigment in European painting till the seventeenth century. Natural deposits were found in antiquity in Mount Sinai; in the mediaeval period in south Italy and Spain, also north of the Alps in England, Germany and Hungary (Kühn 1984). Hungary was, however, the principal source of azurite in Europe until the Ottoman invasion in mid seventeenth century, when supplies from there were cut off (Rutherford et FitzHugh 1993). Although mined locally in Europe azurite could fetch considerable prices if free of impurities and coarsely ground (Panayotova 2020). The colour of azurite varied according to the level of grind: the more coarse powder was dark blue, the finer - more grey. Artists could thus achieve different hues - from pale blue to light green (Clemens 2007).
            The pigment was heavily used in Carolingian manuscripts, especially from the tenth century onwards. It may be applied alone or as mixed or layered with ultramarine (Panayotova 2020). Azurite has been identified in several Eastern Armenian manuscripts from the fourteenth century as well as in a thirteenth-century Byzantine manuscript and in Persian ones from the sixteenth and seventeenth century (Merian et al. 1994).
            Outside Europe azurite was also used in the Far East as for example in wall paintings of the Sung and Ming dynasties in Central China or for Japanese paintings of the Ukiyo-e School (Rutherford et FitzHugh 1993).
            </skos:definition>
        <skos:example>https://commons.wikimedia.org/wiki/File:Azuritepigment.jpg</skos:example>
        <skos:definition rdf:parseType="Resource">
            <rdf:value>References</rdf:value>
            <dct:bibliographicCitation>Kühn, Hermann. Reclams Handbuch der künstlerischen Techniken. Vol. 1. Farbmittel, Buchmalerei, Tafel-und Leinwandmalerei. 3 vols. Stuttgart: Reclam, 1984, pp. 34-35, 95-96.</dct:bibliographicCitation>
            <dct:bibliographicCitation>Rutherford, J. Gettens, and Elisabeth West FitzHugh. ‘Azurite and Blue Verditer’. In Artists’ Pigments: A Handbook of Their History and Characteristics, edited by Ashok Roy, 2:23–35. Washington, DC: National Gallery of Art, 1993. https://www.nga.gov/content/dam/ngaweb/research/publications/pdfs/artists-pigments-vol2.pdf.</dct:bibliographicCitation>
            <dct:bibliographicCitation>Panayotova, Stella. ‘Painting Materials and Techniques in Western Illuminated  Manuscripts c. 600 -c. 1600’. In The Art and Science of Illuminated Manuscripts: A Handbook, edited by Stella Panayotova, 127–70. Turnhout: Brepols, 2020.
            </dct:bibliographicCitation>
            <dct:bibliographicCitation>Merian, Sylvie, Thomas Mathews, and Mary Virginia Orna. ‘The Making of an Armenian Manuscript’. In Treasures in Heaven: Armenian Illuminated Manuscripts, edited by Thomas F. Mathews and Roger S. Wieck, 124–42. New York: Pierpont Morgan Library, 1994.</dct:bibliographicCitation>
            <dct:bibliographicCitation>Clemens, Raymond, and Timothy Graham. Introduction to Manuscript Studies. Ithaca, NY: Cornell University Press, 2007.</dct:bibliographicCitation>
            <dct:bibliographicCitation>Eastaugh, Nicholas, Valentine Walsh, Tracey Chaplin, and Ruth Siddall. Pigment Compendium: A Dictionary and Optical Microscopy of Historical Pigments. Amsterdam: Elsevier, Butterworth-Heinemann, 2008, p. 39.</dct:bibliographicCitation>
            <dct:bibliographicCitation>Material Archiv https://materialarchiv.ch/de/ma:material_905/</dct:bibliographicCitation>
            <dct:bibliographicCitation>ColourLex https://colourlex.com/project/azurite/</dct:bibliographicCitation>
            <dct:bibliographicCitation>Mindat https://www.mindat.org/min-447.html</dct:bibliographicCitation>
            <dct:bibliographicCitation>Spectra by A. Cosentino, Cultural Heritage Science Open Source (CHSOS): https://chsopensource.org/azurite-k-10200/</dct:bibliographicCitation>
        </skos:definition>
        <skos:related rdf:resource="http://gams.uni-graz.at/thesaurus/carbon"/>
        <skos:related rdf:resource="http://gams.uni-graz.at/thesaurus/copper"/>
        <skos:related rdf:resource="http://gams.uni-graz.at/thesaurus/oxygen"/>
        <skos:broader rdf:resource="http://gams.uni-graz.at/thesaurus/blue-colorants"/>
    </skos:Concept>
    <skos:Concept rdf:about="http://gams.uni-graz.at/thesaurus/organic-blue-colorants">
        <skos:inScheme rdf:resource="http://gams.uni-graz.at/thesaurus/mss-materials"/>
        <skos:prefLabel xml:lang="en">Organic blue colourants</skos:prefLabel>
        <skos:prefLabel xml:lang="de">Organische blaue Farbmittel</skos:prefLabel>
        <skos:definition>There is a variety of plants, the extract of which makes an organic blue dye including the blue/purple iris blooms, the petals of the cornflower or the saffron crocus, hyacinth flower and berries of the dogwood tree. The most common and widely used in the Middle Ages was however was the blue from woad and indigo.</skos:definition>
        <skos:broader rdf:resource="http://gams.uni-graz.at/thesaurus/blue-colorants"/>
    </skos:Concept>
    <skos:Concept rdf:about="http://gams.uni-graz.at/thesaurus/indigo">
        <skos:inScheme rdf:resource="http://gams.uni-graz.at/thesaurus/mss-materials"/>
        <skos:prefLabel xml:lang="de">Indigo</skos:prefLabel>
        <skos:altLabel xml:lang="de">Indigotin</skos:altLabel>
        <skos:altLabel xml:lang="de">Färberwaid</skos:altLabel>
        <skos:altLabel xml:lang="de">Waid</skos:altLabel>
        <skos:prefLabel xml:lang="en">Indigo</skos:prefLabel>   
        <skos:altLabel xml:lang="en">Indigotin</skos:altLabel>
        <skos:altLabel xml:lang="en">Woad</skos:altLabel>
        <skos:altLabel xml:lang="en">Wood</skos:altLabel>
        <skos:definition xml:lang="en">Indigo is a generic term used for the blue dyes prepared from various plants of the Indigofera (indigo) and the Isatis tinctoria (woad) species, grown in Asia and Europe (Schweppe 1997; Eastaugh 2007). The two are chemically identical and cannot be distinguished with non-invasive techniques. 
            In antiquity indigo was mainly imported in Europe from India and China, while woad was cultivated already prior to Hellenism in Egypt and Mesopotamia. Woad was also native in Eastern Europe and spread throughout Northern Europe. In the medieval period it was cultivated in Southern France, Picardy, Spain, northern Italy, northern Germany and above all in Thuringia, also in England (Kühn 1984; Clemens 2007). Hence, woad was a likelier source for the blue indigo colour used in manuscript illumination, either on its own or mixed with lead white to create shades of blue, violet and grey (Panayotova 2020).</skos:definition>
        <skos:example>https://commons.wikimedia.org/wiki/File:Indigo-guizhou.jpg</skos:example>
        <skos:definition rdf:parseType="Resource">
            <rdf:value>References</rdf:value>
            <dct:bibliographicCitation>Kühn, Hermann. Reclams Handbuch der künstlerischen Techniken. Vol. 1. Farbmittel, Buchmalerei, Tafel-und Leinwandmalerei. 3 vols. Stuttgart: Reclam, 1984, pp. 39, 96-98.</dct:bibliographicCitation>
            <dct:bibliographicCitation>Schweppe, Helmut. ‘Indigo and Woad’. In Artists’ Pigments: A Handbook of Their History and Characteristics, edited by Elisabeth West FitzHugh, 3:81–107. Washington: National Gallery of Art, 1997. https://www.nga.gov/content/dam/ngaweb/research/publications/pdfs/artists-pigments-vol3.pdf.</dct:bibliographicCitation>
            <dct:bibliographicCitation>Panayotova, Stella. ‘Painting Materials and Techniques in Western Illuminated  Manuscripts c. 600 -c. 1600’. In The Art and Science of Illuminated Manuscripts: A Handbook, edited by Stella Panayotova, 127–70. Turnhout: Brepols, 2020.
            </dct:bibliographicCitation>
            <dct:bibliographicCitation>Clemens, Raymond, and Timothy Graham. Introduction to Manuscript Studies. Ithaca, NY: Cornell University Press, 2007.</dct:bibliographicCitation>
            <dct:bibliographicCitation>Eastaugh, Nicholas, Valentine Walsh, Tracey Chaplin, and Ruth Siddall. Pigment Compendium: A Dictionary and Optical Microscopy of Historical Pigments. Amsterdam: Elsevier, Butterworth-Heinemann, 2008, pp. 200-201.</dct:bibliographicCitation>
            <dct:bibliographicCitation>Material Archiv https://materialarchiv.ch/de/ma:material_990/</dct:bibliographicCitation>
            <dct:bibliographicCitation>ColourLex https://colourlex.com/project/indigo/</dct:bibliographicCitation>
            <dct:bibliographicCitation>Spectra by A. Cosentino, Cultural Heritage Science Open Source (CHSOS): https://chsopensource.org/indigo-k-36005/</dct:bibliographicCitation>
        </skos:definition>
        <skos:related rdf:resource="http://gams.uni-graz.at/thesaurus/carbon"/>
        <skos:related rdf:resource="http://gams.uni-graz.at/thesaurus/hydrogen"/>
        <skos:related rdf:resource="http://gams.uni-graz.at/thesaurus/nitrogen"/>
        <skos:related rdf:resource="http://gams.uni-graz.at/thesaurus/oxygen"/>
        <skos:broader rdf:resource="http://gams.uni-graz.at/thesaurus/organic-blue-colorants"/>
    </skos:Concept>    
    <skos:Concept rdf:about="http://gams.uni-graz.at/thesaurus/egyptian_blue">
        <skos:inScheme rdf:resource="http://gams.uni-graz.at/thesaurus/mss-materials"/>
        <skos:prefLabel xml:lang="de">Ägyptischblau</skos:prefLabel>
        <skos:prefLabel xml:lang="en">Egyptian blue</skos:prefLabel>
        <skos:definition xml:lang="en">Egyptian blue is a synthetic blue pigment, a calcium copper silicate (CaCuSi2O5, CaCuSi4O10 or CaOCuO(SiO2)4). It was produced by heating together a calcium compound (such as powdered limestone), a copper compound (such as malachite), and silica (usually in the form of quartz sand). Depending on its exact composition and process of manufacture its colour varies from a dark blue to a whitish blue. It is completely stable in all media (Riederer 1997). 
            Egyptian blue was widely used in antiquity in Egypt, Greece and Rome. It was used also in ancient Mesopotamia and Persia as well as in West Asia. There are no reported use of the pigment in India, central and East Asia, suggesting that the other blue pigments available in sufficient quantities such as ultramarine, azurite and indigo made the production of Egyptian blue unnecessary (Riederer 1997). 
            The pigment fell from use after the Roman era suggesting that its recipe was forgotten during the Migration Period (Kühn 1984). There are a few reports of Egyptian blue used on wall paintings from the early Middle Ages in Rome and in Müstair, Switzerland (Riederer 1997). During some recent material analysis of medieval manuscripts, however, scientists found Egyptian blue either as the dominant blue used in blue mixtures. The pigment in these cases may have been reused from Roman sites but it is also possible that its production survived into the ninth century (Panayotova 2020; Denoël et al. 2018).
        </skos:definition>
        <skos:definition rdf:parseType="Resource">
            <rdf:value>References</rdf:value>
            <dct:bibliographicCitation>Kühn, Hermann. Reclams Handbuch der künstlerischen Techniken. Vol. 1. Farbmittel, Buchmalerei, Tafel-und Leinwandmalerei. 3 vols. Stuttgart: Reclam, 1984, p. 35.</dct:bibliographicCitation>
            <dct:bibliographicCitation>Panayotova, Stella. ‘Painting Materials and Techniques in Western Illuminated  Manuscripts c. 600 -c. 1600’. In The Art and Science of Illuminated Manuscripts: A Handbook, edited by Stella Panayotova, 127–70. Turnhout: Brepols, 2020.
            </dct:bibliographicCitation>  
            <dct:bibliographicCitation>Denoël, Charlotte, Patricia Roger Puyo, Anne-Marie Brunet, and Nathalie Poulain Siloe. ‘Illuminating the Carolingian Era: New Discoveries as a Result of Scientific Analyses’. Heritage Science 6, no. 1 (2018): 1–19. https://doi.org/10.1186/s40494-018-0194-1.</dct:bibliographicCitation>
            <dct:bibliographicCitation>Riederer, Josef. ‘Egyptian Blue’. In Artists’ Pigments: A Handbook of Their History and Characteristics, edited by Elisabeth West FitzHugh, 3:23–45. Washington: National Gallery of Art, 1997. https://www.nga.gov/content/dam/ngaweb/research/publications/pdfs/artists-pigments-vol3.pdf.
            </dct:bibliographicCitation>
            <dct:bibliographicCitation>Material Archiv https://materialarchiv.ch/de/ma:material_936/</dct:bibliographicCitation>
            <dct:bibliographicCitation>ColourLex https://colourlex.com/project/egyptian-blue/</dct:bibliographicCitation>
        </skos:definition>
        <dct:bibliographicCitation>Spectra by A. Cosentino, Cultural Heritage Science Open Source (CHSOS): https://chsopensource.org/egyptian-blue-k-10060/</dct:bibliographicCitation>
        <skos:example>https://commons.wikimedia.org/wiki/File:Egyptian_blue.jpg</skos:example>
        <skos:related rdf:resource="http://gams.uni-graz.at/thesaurus/calcium"/>
        <skos:related rdf:resource="http://gams.uni-graz.at/thesaurus/copper"/>
        <skos:related rdf:resource="http://gams.uni-graz.at/thesaurus/silicon"/>
        <skos:related rdf:resource="http://gams.uni-graz.at/thesaurus/oxygen"/>
        <skos:broader rdf:resource="http://gams.uni-graz.at/thesaurus/blue-colorants"/>
    </skos:Concept>
    <skos:Concept rdf:about="http://gams.uni-graz.at/thesaurus/smalt">
        <skos:inScheme rdf:resource="http://gams.uni-graz.at/thesaurus/mss-materials"/>
        <skos:prefLabel xml:lang="de">Smalte</skos:prefLabel>
        <skos:prefLabel xml:lang="en">Smalt</skos:prefLabel>
        <skos:definition xml:lang="en">Smalt is a cobalt-containing glass (Co(SiO2)), that was ground into a fine powder and used as a pigment. The pigment was used in Europe at least from the fifteenth century onwards. In the Near East smalt was first produced several centuries earlier (Mühlethaler et Thissen 1993) but there is no record of its use for book illuminations.
            Its earliest use in manuscript illumination was reported in manuscripts made c. 1420-1440 on the island of Murano in the Venetian lagoon (Panayotova 2020). Smalt has been identified also in at least one Armenian manuscript from the fifteenth cenutry and in Persian and Turkish manuscripts from the sixteenth to the eighteenth century (Merian et al. 1994). Mühlethaler et Thissen (1993) suggest the use of smalt increased in the seventeenth century when other blue pigments such as ultramarine and azurite became scarce. Since however smalt is a glass and its particles are transparent, it was employed for skies and backgrounds of paintings where an intense blue was not needed (Mühlethaler et Thissen 1993).
            </skos:definition>        
        <skos:example>https://upload.wikimedia.org/wikipedia/commons/9/9c/Smalte-Historische_Farbstoffsammlung.jpg</skos:example>
        <skos:definition rdf:parseType="Resource">
            <rdf:value>References</rdf:value>
            <dct:bibliographicCitation>Kühn, Hermann. Reclams Handbuch der künstlerischen Techniken. Vol. 1. Farbmittel, Buchmalerei, Tafel-und Leinwandmalerei. 3 vols. Stuttgart: Reclam, 1984, p. 37.</dct:bibliographicCitation>
            <dct:bibliographicCitation>Panayotova, Stella. ‘Painting Materials and Techniques in Western Illuminated  Manuscripts c. 600 -c. 1600’. In The Art and Science of Illuminated Manuscripts: A Handbook, edited by Stella Panayotova, 127–70. Turnhout: Brepols, 2020, p. 142.
            </dct:bibliographicCitation> 
            <dct:bibliographicCitation>Mühlethaler, Bruno, and Jean Thissen. ‘Smalt’. In Artists’ Pigments: A Handbook of Their History and Characteristics, edited by Ashok Roy, 2:113–30. Washington, DC: National Gallery of Art, 1993. https://www.nga.gov/content/dam/ngaweb/research/publications/pdfs/artists-pigments-vol2.pdf.</dct:bibliographicCitation>
            <dct:bibliographicCitation>Merian, Sylvie, Thomas Mathews, and Mary Virginia Orna. ‘The Making of an Armenian Manuscript’. In Treasures in Heaven: Armenian Illuminated Manuscripts, edited by Thomas F. Mathews and Roger S. Wieck, 124–42. New York: Pierpont Morgan Library, 1994.</dct:bibliographicCitation>
            <dct:bibliographicCitation>Material Archiv https://materialarchiv.ch/de/ma:material_933/</dct:bibliographicCitation>
            <dct:bibliographicCitation>ColourLex https://colourlex.com/project/smalt/</dct:bibliographicCitation>
            <dct:bibliographicCitation>Spectra by A. Cosentino, Cultural Heritage Science Open Source (CHSOS): https://chsopensource.org/smalt-k-10000/</dct:bibliographicCitation>
        </skos:definition>
        <skos:related rdf:resource="http://gams.uni-graz.at/thesaurus/cobalt"/>
        <skos:related rdf:resource="http://gams.uni-graz.at/thesaurus/silicon"/>
        <skos:related rdf:resource="http://gams.uni-graz.at/thesaurus/oxygen"/>
        <skos:broader rdf:resource="http://gams.uni-graz.at/thesaurus/blue-colorants"/>
    </skos:Concept>
    
<!--    ########### Purple ########## -->
    <skos:Concept rdf:about="http://gams.uni-graz.at/thesaurus/purple-colorants">
        <skos:inScheme rdf:resource="http://gams.uni-graz.at/thesaurus/mss-materials"/>
        <skos:prefLabel xml:lang="de">Purpur Farbmittel</skos:prefLabel>
        <skos:prefLabel xml:lang="en">Purple colorant</skos:prefLabel>
        <skos:definition xml:lang="en">Artists in the medieval period achieved purple and violet colour either by applying organic purple dyes or by mixing organic reds with ultramarine, indigo or azurite (either by mixing the substance or by layering the colours). Apart from illuminations, there are also parchment leaves dyed in purple.</skos:definition>
        <skos:example>https://upload.wikimedia.org/wikipedia/commons/7/78/Purple_tints_and_shades.svg</skos:example>
        <skos:broader rdf:resource="http://gams.uni-graz.at/thesaurus/colorants"/>
    </skos:Concept>
    <skos:Concept rdf:about="http://gams.uni-graz.at/thesaurus/orcein">
        <skos:inScheme rdf:resource="http://gams.uni-graz.at/thesaurus/mss-materials"/>
        <skos:prefLabel xml:lang="de">Orcein</skos:prefLabel>
        <skos:prefLabel xml:lang="en">Orchil</skos:prefLabel>
        <skos:altLabel xml:lang="en">Orcein</skos:altLabel>
        <skos:definition xml:lang="en">Orchil (or orcein) is an organic purple-blue pigment produced from different types of lichens, both from sea and land sources (Rabitsch et al. 2020). It has been identified in numerous manuscripts dating from the sixth to the sixteenth century (Panayotova 2020). The dye was applied alone or in combination with other organic blue or red dyes for the colouration of textile fibres (Rabitsch et al. 2020). For the preparation of the dye see Rabitsch et al. 2020.</skos:definition>
        <skos:definition rdf:parseType="Resource">
            <rdf:value>References</rdf:value>            
            <dct:bibliographicCitation>Panayotova, Stella. ‘Painting Materials and Techniques in Western Illuminated  Manuscripts c. 600 -c. 1600’. In The Art and Science of Illuminated Manuscripts: A Handbook, edited by Stella Panayotova, 127–70. Turnhout: Brepols, 2020, esp. p. 146.
            </dct:bibliographicCitation>
            <dct:bibliographicCitation>Rabitsch, Sophie, Inge Boesken Kanold, and Christa Hoffmann. ‘Purple Dyeing of Parchment’. In The Vienna Genesis: Material Analysis and Conservation of a Late Antique Illuminated Manuscript on Purple Parchment, edited by Christa Hofmann, 71–101. Vienna: Böhlau Verlag, 2020.</dct:bibliographicCitation>
            <dct:bibliographicCitation>Eastaugh, Nicholas, Valentine Walsh, Tracey Chaplin, and Ruth Siddall. Pigment Compendium: A Dictionary and Optical Microscopy of Historical Pigments. Amsterdam: Elsevier, Butterworth-Heinemann, 2008, p. 289.</dct:bibliographicCitation>    
            <dct:bibliographicCitation>Aceto, Maurizio et al. "On the identification of folium and orchil on illuminated manuscripts." In Spectrochimica acta. Part A, Molecular and biomolecular spectroscopy (2016) 171: 461-469. 10.1016/j.saa.2016.08.046. </dct:bibliographicCitation>
        </skos:definition>
        <skos:example>https://commons.wikimedia.org/wiki/File:Orcein2.jpg</skos:example>
        <skos:related rdf:resource="http://gams.uni-graz.at/thesaurus/carbon"/>
        <skos:related rdf:resource="http://gams.uni-graz.at/thesaurus/hydrogen"/>
        <skos:related rdf:resource="http://gams.uni-graz.at/thesaurus/nitrogen"/>
        <skos:related rdf:resource="http://gams.uni-graz.at/thesaurus/oxygen"/>
        <skos:broader rdf:resource="http://gams.uni-graz.at/thesaurus/purple-colorants"/>
    </skos:Concept>
    <skos:Concept rdf:about="http://gams.uni-graz.at/thesaurus/chrozophora-tinctoria">
        <skos:inScheme rdf:resource="http://gams.uni-graz.at/thesaurus/mss-materials"/>
        <skos:prefLabel xml:lang="de">Chrozophora tinctoria</skos:prefLabel>
        <skos:altLabel xml:lang="en">Chrozophora tinctoria</skos:altLabel>
        <skos:prefLabel xml:lang="en">Folium</skos:prefLabel>
        <skos:altLabel xml:lang="en">Tournasol</skos:altLabel>
        <skos:altLabel xml:lang="en">Turnsole</skos:altLabel>
        <skos:definition xml:lang="en">Folium is an organic dye, which offered three different hues depending on the preparation method: purple, red or blue (Panayotova 2020). It is extracted from the fruits and parts of the plant Chrozophora tinctoria, which is native to the Mediterranean region and central/south Asia. Like orchil, it was cheaper and easier to extract than shellfish purple but much more light-sensitive (Rabitsch 2020).</skos:definition>
        <skos:definition rdf:parseType="Resource">
            <rdf:value>References</rdf:value>            
            <dct:bibliographicCitation>Panayotova, Stella. ‘Painting Materials and Techniques in Western Illuminated  Manuscripts c. 600 -c. 1600’. In The Art and Science of Illuminated Manuscripts: A Handbook, edited by Stella Panayotova, 127–70. Turnhout: Brepols, 2020, p. 146.
            </dct:bibliographicCitation>
            <dct:bibliographicCitation>Rabitsch, Sophie, Inge Boesken Kanold, and Christa Hoffmann. ‘Purple Dyeing of Parchment’. In The Vienna Genesis: Material Analysis and Conservation of a Late Antique Illuminated Manuscript on Purple Parchment, edited by Christa Hofmann, 71–101. Vienna: Böhlau Verlag, 2020.</dct:bibliographicCitation>
            <dct:bibliographicCitation>Aceto, Maurizio et al. "On the identification of folium and orchil on illuminated manuscripts." In Spectrochimica acta. Part A, Molecular and biomolecular spectroscopy (2016) 171: 461-469. 10.1016/j.saa.2016.08.046. </dct:bibliographicCitation>
        </skos:definition>
        <skos:related rdf:resource="http://gams.uni-graz.at/thesaurus/carbon"/>
        <skos:related rdf:resource="http://gams.uni-graz.at/thesaurus/hydrogen"/>
        <skos:related rdf:resource="http://gams.uni-graz.at/thesaurus/nitrogen"/>
        <skos:related rdf:resource="http://gams.uni-graz.at/thesaurus/oxygen"/>
        <skos:broader rdf:resource="http://gams.uni-graz.at/thesaurus/purple-colorants"/>
    </skos:Concept>  
    <skos:Concept rdf:about="http://gams.uni-graz.at/thesaurus/tyrian-purple">
        <skos:inScheme rdf:resource="http://gams.uni-graz.at/thesaurus/mss-materials"/>
        <skos:prefLabel xml:lang="de">Purpur</skos:prefLabel>
        <skos:prefLabel xml:lang="en">Tyrian purple</skos:prefLabel>
        <skos:altLabel xml:lang="en">Shellfish purple</skos:altLabel>
        <skos:altLabel xml:lang="en">Byzantine purple</skos:altLabel>
        <skos:altLabel xml:lang="en">Royal purple</skos:altLabel>
        <skos:altLabel xml:lang="en">Imperial purple</skos:altLabel>
        <skos:definition xml:lang="en">Tyrian or shellfish purple is derived from different purple-producing marine shellfish found in warm seas around the world. In antiquity, the marine snails were mainly fished in the Mediterranean Sea; the most expensive purple came from the city of Tyre in Phoenicia (Rabitsch 2020, Eastaugh et al. 2008). Bede the Venerable reported of abundance of purple-producing snails on English shores probably referring to the native purpura lapillus (Kühn 1984).</skos:definition>
        <skos:example>https://commons.wikimedia.org/wiki/File:Purple_Purpur_(retouched).jpg</skos:example>
        <skos:definition rdf:parseType="Resource">
            <rdf:value>References</rdf:value>
            <dct:bibliographicCitation>Kühn, Hermann. Reclams Handbuch der künstlerischen Techniken. Vol. 1. Farbmittel, Buchmalerei, Tafel-und Leinwandmalerei. 3 vols. Stuttgart: Reclam, 1984, pp. 24-25, 83-85.</dct:bibliographicCitation>
            <dct:bibliographicCitation>Rabitsch, Sophie, Inge Boesken Kanold, and Christa Hoffmann. ‘Purple Dyeing of Parchment’. In The Vienna Genesis: Material Analysis and Conservation of a Late Antique Illuminated Manuscript on Purple Parchment, edited by Christa Hofmann, 71–101. Vienna: Böhlau Verlag, 2020.</dct:bibliographicCitation>
            <dct:bibliographicCitation>Panayotova, Stella. ‘Painting Materials and Techniques in Western Illuminated  Manuscripts c. 600 -c. 1600’. In The Art and Science of Illuminated Manuscripts: A Handbook, edited by Stella Panayotova, 127–70. Turnhout: Brepols, 2020, esp. p. 144.
            </dct:bibliographicCitation>
            <dct:bibliographicCitation>Eastaugh, Nicholas, Valentine Walsh, Tracey Chaplin, and Ruth Siddall. Pigment Compendium: A Dictionary and Optical Microscopy of Historical Pigments. Amsterdam: Elsevier, Butterworth-Heinemann, 2008, p. 379-380.</dct:bibliographicCitation>  
            <dct:bibliographicCitation>ColourLex https://colourlex.com/project/tyrian-purple/</dct:bibliographicCitation>
        </skos:definition>
        <skos:related rdf:resource="http://gams.uni-graz.at/thesaurus/bromine"/>
        <skos:related rdf:resource="http://gams.uni-graz.at/thesaurus/carbon"/>
        <skos:related rdf:resource="http://gams.uni-graz.at/thesaurus/hydrogen"/>
        <skos:related rdf:resource="http://gams.uni-graz.at/thesaurus/nitrogen"/>
        <skos:related rdf:resource="http://gams.uni-graz.at/thesaurus/oxygen"/>
        <skos:broader rdf:resource="http://gams.uni-graz.at/thesaurus/purple-colorants"/>
    </skos:Concept>
    <!-- #############  WHITE  #############  -->
    <skos:Concept rdf:about="http://gams.uni-graz.at/thesaurus/white-colorants">
        <skos:inScheme rdf:resource="http://gams.uni-graz.at/thesaurus/mss-materials"/>
        <skos:prefLabel xml:lang="de">Weiße Farbmittel</skos:prefLabel>
        <skos:prefLabel xml:lang="en">White colorants</skos:prefLabel>
        <skos:definition xml:lang="en">Apart from the wide-spread synthetic pigment lead white medieval artists could use whites based on calcium carbonate (such as chalk, shell white or calcite) or calcium phospate (calcinated bone). These calcium compounds were however mainly used for the preparation and whitening of parchment prior to writing and illumination (Ricciardi et al. 2016).</skos:definition>
        <skos:definition rdf:parseType="Resource">
            <rdf:value>References</rdf:value>
            <dct:bibliographicCitation>Ricciardi, Paola, and Kristine Rose Beers. ‘The Illuminators’ Palette’. In Colour : The Art and Science of Illuminated Manuscripts, edited by Stella Panayotova, Deirdre Elizabeth Jackson, and Paola Ricciardi, 27–73. Turnhout: Brepols, 2016.</dct:bibliographicCitation>    
        </skos:definition>
        <skos:example>https://upload.wikimedia.org/wikipedia/commons/0/07/White_tints_and_shades.svg</skos:example>
        <skos:broader rdf:resource="http://gams.uni-graz.at/thesaurus/colorants"/>
    </skos:Concept>
    <skos:Concept rdf:about="http://gams.uni-graz.at/thesaurus/bone-white">
        <skos:inScheme rdf:resource="http://gams.uni-graz.at/thesaurus/mss-materials"/>
        <skos:prefLabel xml:lang="de">Knochenkohle</skos:prefLabel>
        <skos:prefLabel xml:lang="en">Bone calcined</skos:prefLabel>
        <skos:altLabel xml:lang="en">Bone white</skos:altLabel>
        <skos:altLabel xml:lang="en">Bone ash</skos:altLabel>
        <skos:definition xml:lang="en">The white pigment can be produced from white calcinated bone dust in some recipes mixing it with pumice powder, adding them to oil, which is then boiled. Such white has been found in the Glajor gospel, an illustrated Armenian gospel book of the fourteenth century (Eastaugh et al. 2008).</skos:definition>
        <skos:definition rdf:parseType="Resource">
            <rdf:value>References</rdf:value>            
            <dct:bibliographicCitation>Eastaugh, Nicholas, Valentine Walsh, Tracey Chaplin, and Ruth Siddall. Pigment Compendium: A Dictionary and Optical Microscopy of Historical Pigments. Amsterdam: Elsevier, Butterworth-Heinemann, 2008.</dct:bibliographicCitation>            
        </skos:definition>
        <skos:related rdf:resource="http://gams.uni-graz.at/thesaurus/calcium"/>
        <skos:related rdf:resource="http://gams.uni-graz.at/thesaurus/phosphorus"/>
        <skos:broader rdf:resource="http://gams.uni-graz.at/thesaurus/white-colorants"/>
    </skos:Concept>
    <skos:Concept rdf:about="http://gams.uni-graz.at/thesaurus/lead-white">
        <skos:inScheme rdf:resource="http://gams.uni-graz.at/thesaurus/mss-materials"/>
        <skos:prefLabel xml:lang="de">Bleiweiß</skos:prefLabel>
        <skos:prefLabel xml:lang="en">Lead white</skos:prefLabel>
        <skos:definition xml:lang="en">Lead white, often called ceruse in Latin sources, is a lead carbonate hydroxide (2 PbCO3·Pb(OH)2). It is found in nature as basic lead carbonate, but was routinely manufactured in the medieval period by exposing leaf strips to the vapours of vinegar in a pot sealed and buried under hot manute (Panayotova 2020). The manufacture is described in several antique and medieval; see for instance Theophilus (I, 37). The pigment was supplied either in dried cakes or ground with oil. The latter method was safer as it reduced the dispersion of poisonous dusts (Eastaugh et al. 2008).
            Lead white was used extensively since antiquity and especially for painting flesh tones. It was commonly adulterated with other white pigments, particularly chalk, baryte and kaolinite (Eastaugh et al. 2008). A thin layer of lead white applied over the underdrawing provided a smooth white surface and enhanced the brightness of pigments (Panayotova 2020). To whiten the parchment leaves some artists used a thin wash of lead white instead the usual treatment with chalk (Cheese 2020). 
            Lead white mixed with aqueous binders reacts with sulfur and turns black Leadsulfid (PbS). Medieval treatises mention the incompatibility of lead white and orpiment (which consists of sulfur) and recommend the use of another white for mixing with orpiment - either chalk or a pigment produced from burnt bones (ossa combusta) (Kühn 1984).</skos:definition>
        <skos:example>https://commons.wikimedia.org/wiki/File:BleiweissDuerer.JPG</skos:example>
        <skos:definition rdf:parseType="Resource">
            <rdf:value>References</rdf:value>
            <dct:bibliographicCitation>Kühn, Hermann. Reclams Handbuch der künstlerischen Techniken. Vol. 1. Farbmittel, Buchmalerei, Tafel-und Leinwandmalerei. 3 vols. Stuttgart: Reclam, 1984.</dct:bibliographicCitation>
            <dct:bibliographicCitation>Panayotova, Stella. ‘Painting Materials and Techniques in Western Illuminated  Manuscripts c. 600 -c. 1600’. In The Art and Science of Illuminated Manuscripts: A Handbook, edited by Stella Panayotova, 127–70. Turnhout: Brepols, 2020.</dct:bibliographicCitation>
            <dct:bibliographicCitation>Cheese, Edward. ‘From Pelt to Painted Page: Western Medieval Manuscript Parchments’. In The Art and Science of Illuminated Manuscripts: A Handbook, edited by Stella Panayotova, 73–94. Turnhout: Brepols, 2020.</dct:bibliographicCitation>
            <dct:bibliographicCitation>Theophilus, Presbyter. On Divers Arts: The Foremost Medieval Treatise on Painting, Glassmaking and Metalwork. Translated by John G. Hawthorne. New York: Dover, 1979.</dct:bibliographicCitation>
            <dct:bibliographicCitation>Eastaugh, Nicholas, Valentine Walsh, Tracey Chaplin, and Ruth Siddall. Pigment Compendium: A Dictionary and Optical Microscopy of Historical Pigments. Amsterdam: Elsevier, Butterworth-Heinemann, 2008.</dct:bibliographicCitation>
            <dct:bibliographicCitation>Material Archiv https://materialarchiv.ch/de/ma:material_982/</dct:bibliographicCitation>
            <dct:bibliographicCitation>ColourLex https://colourlex.com/project/lead-white/</dct:bibliographicCitation>
            <dct:bibliographicCitation>Spectra by A. Cosentino, Cultural Heritage Science Open Source (CHSOS): https://chsopensource.org/lead-white-k-46000/</dct:bibliographicCitation>
        </skos:definition>
        <skos:related rdf:resource="http://gams.uni-graz.at/thesaurus/carbon"/>
        <skos:related rdf:resource="http://gams.uni-graz.at/thesaurus/oxygen"/>
        <skos:related rdf:resource="http://gams.uni-graz.at/thesaurus/lead"/>
        <skos:broader rdf:resource="http://gams.uni-graz.at/thesaurus/white-colorants"/>
    </skos:Concept>   
    <skos:Concept rdf:about="http://gams.uni-graz.at/thesaurus/gypsum">
        <skos:inScheme rdf:resource="http://gams.uni-graz.at/thesaurus/mss-materials"/>
        <skos:prefLabel xml:lang="de">Gips</skos:prefLabel>
        <skos:prefLabel xml:lang="en">Gypsum</skos:prefLabel>
        <skos:altLabel xml:lang="en">Plaster of Paris</skos:altLabel>
        <skos:definition xml:lang="en">Gypsum is a calciumsulfat (CaSO4·2H2O). Significant deposits are found in Thuringia, Franken, Württemberg, in the Baltic reagion (Courland and Livonia), Italy. Gypsum was rarely used as a white pigment per se. It was mixed with animal glue binder and chalk to make gesso used for ground for illumination and gilding (Panayotova 2020).</skos:definition>
        <skos:definition rdf:parseType="Resource">
            <rdf:value>References</rdf:value>            
            <dct:bibliographicCitation>Panayotova, Stella. ‘Painting Materials and Techniques in Western Illuminated  Manuscripts c. 600 -c. 1600’. In The Art and Science of Illuminated Manuscripts: A Handbook, edited by Stella Panayotova, 127–70. Turnhout: Brepols, 2020.</dct:bibliographicCitation>   
            <dct:bibliographicCitation>Spectra by A. Cosentino, Cultural Heritage Science Open Source (CHSOS): https://chsopensource.org/gypsum-k-58300/</dct:bibliographicCitation>
        </skos:definition>
        <skos:example>https://commons.wikimedia.org/wiki/File:Gypsum_(12249949575).jpg</skos:example>
        <skos:related rdf:resource="http://gams.uni-graz.at/thesaurus/calcium"/>
        <skos:related rdf:resource="http://gams.uni-graz.at/thesaurus/oxygen"/>
        <skos:related rdf:resource="http://gams.uni-graz.at/thesaurus/sulfur"/>
        <skos:related rdf:resource="http://gams.uni-graz.at/thesaurus/hydrogen"/>
        <skos:broader rdf:resource="http://gams.uni-graz.at/thesaurus/white-colorants"/>
    </skos:Concept>
    <skos:Concept rdf:about="http://gams.uni-graz.at/thesaurus/kaolin">
        <skos:inScheme rdf:resource="http://gams.uni-graz.at/thesaurus/mss-materials"/>
        <skos:prefLabel xml:lang="de">Kaolin</skos:prefLabel>
        <skos:altLabel xml:lang="de">Porzellanerde</skos:altLabel>
        <skos:prefLabel xml:lang="en">Kaolin</skos:prefLabel>
        <skos:altLabel xml:lang="en">Kaolinite</skos:altLabel>
        <skos:definition xml:lang="en">Kaolin, a common name for kaolinite, is a white clay, an aluminium silicate hydroxide mineral of composition Al4[Si4O10](OH)8. Calcium, iron, magnesium and potassium can be found as trace elements or impurities (Eastaugh et al. 2008).
            Chemically very resistant, it decreases the crack formation and increases the surface stability of paintings (Kremer-pigmente.com).</skos:definition>
        <skos:example>https://commons.wikimedia.org/wiki/File:Erbsl%C3%B6h_Geisenheim_Kaolin_(02).jpg</skos:example>
        <skos:definition rdf:parseType="Resource">
            <rdf:value>References</rdf:value>            
            <dct:bibliographicCitation>Eastaugh, Nicholas, Valentine Walsh, Tracey Chaplin, and Ruth Siddall. Pigment Compendium: A Dictionary and Optical Microscopy of Historical Pigments. Amsterdam: Elsevier, Butterworth-Heinemann, 2008.</dct:bibliographicCitation>
            <dct:bibliographicCitation>Material Archiv https://materialarchiv.ch/de/ma:material_932/</dct:bibliographicCitation>
            <dct:bibliographicCitation>Kremer Pigmente https://shop.kremerpigments.com/elements/resources/products/files/58250e.pdf</dct:bibliographicCitation>
        </skos:definition>
        <skos:related rdf:resource="http://gams.uni-graz.at/thesaurus/carbon"/>
        <skos:related rdf:resource="http://gams.uni-graz.at/thesaurus/oxygen"/>
        <skos:related rdf:resource="http://gams.uni-graz.at/thesaurus/silicon"/>
        <skos:related rdf:resource="http://gams.uni-graz.at/thesaurus/aluminium"/>
        <skos:broader rdf:resource="http://gams.uni-graz.at/thesaurus/white-colorants"/>
    </skos:Concept>
    <skos:Concept rdf:about="http://gams.uni-graz.at/thesaurus/calcium-carbonate-white">
        <skos:inScheme rdf:resource="http://gams.uni-graz.at/thesaurus/mss-materials"/>
        <skos:prefLabel xml:lang="de">Calciumcarbonat</skos:prefLabel>
        <skos:prefLabel xml:lang="en">Calcium carbonate white</skos:prefLabel>
        <skos:definition xml:lang="en">While calcium carbonate (CaCO3) is found in a number of compounds used as pigment. They can be divided into four groups based on origin: 1) mineral origin including calcite, aragonite and vaterite (mainly found in sedimentary rocks such as chalk and limestone, and in marble); 2) biological origin including shells; 3) fossilisation of shells; and 4) synthetically produced calcite (Eastaugh et al. 2008). Calcium carbonate is one of the easiest materials to identify by chemical and microscopical methods, but it is difficult to identify the specific varieties, which are differentiated mainly by particle characteristics (Rutherford et al. 1993).</skos:definition>
        <skos:definition rdf:parseType="Resource">
            <rdf:value>References</rdf:value>            
            <dct:bibliographicCitation>CAMEO Database https://cameo.mfa.org/wiki/Calcium_carbonate</dct:bibliographicCitation>
            <dct:bibliographicCitation>Eastaugh, Nicholas, Valentine Walsh, Tracey Chaplin, and Ruth Siddall. Pigment Compendium: A Dictionary and Optical Microscopy of Historical Pigments. Amsterdam: Elsevier, Butterworth-Heinemann, 2008.</dct:bibliographicCitation>
            <dct:bibliographicCitation>Rutherford, J. Gettens, Elisabeth West FitzHugh, and Robert L. Feller. ‘Calcium Carbonate Whites’. In Artists’ Pigments: A Handbook of Their History and Characteristics, edited by Ashok Roy, 2:203–26. Washington, DC: National Gallery of Art, 1993. https://www.nga.gov/content/dam/ngaweb/research/publications/pdfs/artists-pigments-vol2.pdf.</dct:bibliographicCitation>
        </skos:definition>
        <skos:example>https://upload.wikimedia.org/wikipedia/commons/0/04/Calcium_carbonate.jpg</skos:example>
        <skos:related rdf:resource="http://gams.uni-graz.at/thesaurus/carbon"/>
        <skos:related rdf:resource="http://gams.uni-graz.at/thesaurus/oxygen"/>
        <skos:related rdf:resource="http://gams.uni-graz.at/thesaurus/calcium"/>
        <skos:broader rdf:resource="http://gams.uni-graz.at/thesaurus/white-colorants"/>
    </skos:Concept>
    <skos:Concept rdf:about="http://gams.uni-graz.at/thesaurus/calcite">
        <skos:inScheme rdf:resource="http://gams.uni-graz.at/thesaurus/mss-materials"/>
        <skos:prefLabel xml:lang="de">Kalzit, Aragonit, Vaterit</skos:prefLabel>
        <skos:altLabel xml:lang="de">Calcit, Aragonit, Vaterit</skos:altLabel>
        <skos:prefLabel xml:lang="en">Calcite, aragonite, vaterite</skos:prefLabel>
        <skos:altLabel xml:lang="en">Marble</skos:altLabel>
        <skos:altLabel xml:lang="en">Limestone</skos:altLabel>
        <skos:definition xml:lang="en">The most common mineral form of calcium carbonate is calcite (CaCO3); less common are the minerals aragonite and vaterite. Calcite is found in sedimentary rocks such as chalk and limestone, and in marble. The generic term limestone refers to a range of sedimentary rocks consisting primarily of calcite, aragonite and vaterite, and dolomite (Eastaugh et al. 2008). The so-called 'Lime white' or 'St. John's white' is a calcinated form of calcite (usually limestone or marble). It is mentioned by Cennini as a form of a pasty used as white pigment, which does not require binding medium (Rutherford et al. 1993).
            In art calcite could be used as a white pigment per se or as an extender or bulking agent for other paints. Artists used it also as a ground for painting when mixed with animal glues (Eastaught et al. 2008). Flieder identified calcite in 19 illuminated manuscripts from the tenth to the sixteenth century (Flieder 1968).</skos:definition>
        <skos:example>https://upload.wikimedia.org/wikipedia/commons/0/02/Calcite-67881.jpg</skos:example>
        <skos:definition rdf:parseType="Resource">
            <rdf:value>References</rdf:value> 
            <dct:bibliographicCitation>Eastaugh, Nicholas, Valentine Walsh, Tracey Chaplin, and Ruth Siddall. Pigment Compendium: A Dictionary and Optical Microscopy of Historical Pigments. Amsterdam: Elsevier, Butterworth-Heinemann, 2008.</dct:bibliographicCitation>
            <dct:bibliographicCitation>Rutherford, J. Gettens, Elisabeth West FitzHugh, and Robert L. Feller. ‘Calcium Carbonate Whites’. In Artists’ Pigments: A Handbook of Their History and Characteristics, edited by Ashok Roy, 2:203–26. Washington, DC: National Gallery of Art, 1993. https://www.nga.gov/content/dam/ngaweb/research/publications/pdfs/artists-pigments-vol2.pdf.</dct:bibliographicCitation>
            <dct:bibliographicCitation>Flieder, Françoise. ‘Mise au point des techniques d’identification des pigments et des liants inclus dans la couche picturale des enluminures de manuscrits’. Studies in conservation 13, no. 2 (1968): 49–86. https://doi.org/10.1179/sic.1968.005.</dct:bibliographicCitation>
        </skos:definition>
        <skos:related rdf:resource="http://gams.uni-graz.at/thesaurus/carbon"/>
        <skos:related rdf:resource="http://gams.uni-graz.at/thesaurus/oxygen"/>
        <skos:related rdf:resource="http://gams.uni-graz.at/thesaurus/calcium"/>
        <skos:broader rdf:resource="http://gams.uni-graz.at/thesaurus/calcium-carbonate-white"/>
    </skos:Concept>
    <skos:Concept rdf:about="http://gams.uni-graz.at/thesaurus/chalk">
        <skos:inScheme rdf:resource="http://gams.uni-graz.at/thesaurus/mss-materials"/>
        <skos:prefLabel xml:lang="de">Kreide</skos:prefLabel>
        <skos:prefLabel xml:lang="en">Chalk</skos:prefLabel>
        <skos:definition xml:lang="en">Chalk is a specific variety of limestone formed entirely from fossilised algae, coccolithophore (Eastaugh et al. 2008). Chalk deposits exist in the UK, western continental Europe (France, Denmark, Sweden), in the eastern Mediterranean, on the coast of the Baltic Sea, and in Austria (Müllendorf).
            Since the pigment was abundant and easily processed, it was cherished for its whiteness, softness and fine-grained nature. Being transparent, it is often used in combination with other pigments and with animal glues as a ground for painting rather than as a white pigment on its own (Eastaugh et al. 2008). It is also find on parchment leaves, which were treated with chalk during manufacture to remove remaining grease and fat or for whitening the skin (Cheese 2020).</skos:definition>
        <skos:example>https://commons.wikimedia.org/wiki/File:Chalk_(%22Upper_Chalk%22_Formation,_Upper_Cretaceous;_White_Cliffs_of_Dover,_England,_southern_Britain).jpg</skos:example>
        <skos:definition rdf:parseType="Resource">
            <rdf:value>References</rdf:value>            
            <dct:bibliographicCitation>Panayotova, Stella. ‘Painting Materials and Techniques in Western Illuminated  Manuscripts c. 600 -c. 1600’. In The Art and Science of Illuminated Manuscripts: A Handbook, edited by Stella Panayotova, 127–70. Turnhout: Brepols, 2020.</dct:bibliographicCitation>
            <dct:bibliographicCitation>Rutherford, J. Gettens, Elisabeth West FitzHugh, and Robert L. Feller. ‘Calcium Carbonate Whites’. In Artists’ Pigments: A Handbook of Their History and Characteristics, edited by Ashok Roy, 2:203–26. Washington, DC: National Gallery of Art, 1993. https://www.nga.gov/content/dam/ngaweb/research/publications/pdfs/artists-pigments-vol2.pdf.</dct:bibliographicCitation>
            <dct:bibliographicCitation>Cheese, Edward. ‘From Pelt to Painted Page: Western Medieval Manuscript Parchments’. In The Art and Science of Illuminated Manuscripts: A Handbook, edited by Stella Panayotova, 73–94. Turnhout: Brepols, 2020.</dct:bibliographicCitation>
            <dct:bibliographicCitation>Eastaugh, Nicholas, Valentine Walsh, Tracey Chaplin, and Ruth Siddall. Pigment Compendium: A Dictionary and Optical Microscopy of Historical Pigments. Amsterdam: Elsevier, Butterworth-Heinemann, 2008.</dct:bibliographicCitation>
            <dct:bibliographicCitation>ColourLex https://colourlex.com/project/calcite/</dct:bibliographicCitation>
            <dct:bibliographicCitation>Spectra by A. Cosentino, Cultural Heritage Science Open Source (CHSOS): https://chsopensource.org/chalk-k-58000/</dct:bibliographicCitation>
        </skos:definition>
        <skos:related rdf:resource="http://gams.uni-graz.at/thesaurus/carbon"/>
        <skos:related rdf:resource="http://gams.uni-graz.at/thesaurus/oxygen"/>
        <skos:related rdf:resource="http://gams.uni-graz.at/thesaurus/calcium"/>
        <skos:broader rdf:resource="http://gams.uni-graz.at/thesaurus/calcium-carbonate-white"/>
    </skos:Concept>
    <skos:Concept rdf:about="http://gams.uni-graz.at/thesaurus/shell-white">
        <skos:inScheme rdf:resource="http://gams.uni-graz.at/thesaurus/mss-materials"/>
        <skos:prefLabel xml:lang="de">Muschelweiß</skos:prefLabel>
        <skos:prefLabel xml:lang="en">Shell white</skos:prefLabel>
        <skos:altLabel xml:lang="en">Eggshell white</skos:altLabel>
        <skos:definition xml:lang="en">The term shell white is used to describe the white powder produced either from the shells of molluscs (sea shells, cuttlefish bone etc.)or from crushed eggshells. The powdered substance can be used as whiting or ground limestone (Rutherford et al. 1993).</skos:definition>
        <skos:example></skos:example>
        <skos:definition rdf:parseType="Resource">
            <rdf:value>References</rdf:value>            
            <dct:bibliographicCitation>Rutherford, J. Gettens, Elisabeth West FitzHugh, and Robert L. Feller. ‘Calcium Carbonate Whites’. In Artists’ Pigments: A Handbook of Their History and Characteristics, edited by Ashok Roy, 2:203–26. Washington, DC: National Gallery of Art, 1993. https://www.nga.gov/content/dam/ngaweb/research/publications/pdfs/artists-pigments-vol2.pdf.</dct:bibliographicCitation>
        </skos:definition>
        <skos:related rdf:resource="http://gams.uni-graz.at/thesaurus/carbon"/>
        <skos:related rdf:resource="http://gams.uni-graz.at/thesaurus/oxygen"/>
        <skos:related rdf:resource="http://gams.uni-graz.at/thesaurus/calcium"/>
        <skos:broader rdf:resource="http://gams.uni-graz.at/thesaurus/calcium-carbonate-white"/>
    </skos:Concept>   
    
    <skos:Concept rdf:about="http://gams.uni-graz.at/thesaurus/coral">
        <skos:inScheme rdf:resource="http://gams.uni-graz.at/thesaurus/mss-materials"/>
        <skos:prefLabel xml:lang="de">Koralle</skos:prefLabel>
        <skos:prefLabel xml:lang="en">Coral</skos:prefLabel>
        <skos:definition xml:lang="en">Ground coral consists essentially of calcium carbonate. In Japan it is used as a specialty pigment employed for decorative effects. The white form of coral is common in Europe but there are no references in European literary sources of its use as pigment (Rutherford et al. 1993). </skos:definition>
        <skos:definition rdf:parseType="Resource">
            <rdf:value>References</rdf:value>            
            <dct:bibliographicCitation>Rutherford, J. Gettens, Elisabeth West FitzHugh, and Robert L. Feller. ‘Calcium Carbonate Whites’. In Artists’ Pigments: A Handbook of Their History and Characteristics, edited by Ashok Roy, 2:203–26. Washington, DC: National Gallery of Art, 1993. https://www.nga.gov/content/dam/ngaweb/research/publications/pdfs/artists-pigments-vol2.pdf.</dct:bibliographicCitation>
        </skos:definition>
        <skos:related rdf:resource="http://gams.uni-graz.at/thesaurus/carbon"/>
        <skos:related rdf:resource="http://gams.uni-graz.at/thesaurus/oxygen"/>
        <skos:related rdf:resource="http://gams.uni-graz.at/thesaurus/calcium"/>
        <skos:broader rdf:resource="http://gams.uni-graz.at/thesaurus/calcium-carbonate-white"/>
    </skos:Concept>
    <!-- #############  GREEN  #############  -->
    <skos:Concept rdf:about="http://gams.uni-graz.at/thesaurus/green-colorants">
        <skos:inScheme rdf:resource="http://gams.uni-graz.at/thesaurus/mss-materials"/>
        <skos:prefLabel xml:lang="de">Grüne Farbmittel</skos:prefLabel>
        <skos:prefLabel xml:lang="en">Green colorants</skos:prefLabel>
        <skos:definition xml:lang="en">Mediaeval artists used both green organic and inorganic colourant as well as mixtures of blue and yellow colourants. In some miniatures the green colour was obtained not by mixing but by layering and overlapping blue and yellow pigments. Using organic pigments over copper-based greens also gave more stability and diminished the corrosive character of the latter (Panayotova 2020).</skos:definition>
        <skos:example>https://upload.wikimedia.org/wikipedia/commons/f/fb/Green_tints_and_shades.svg</skos:example>
        <skos:definition rdf:parseType="Resource">
            <rdf:value>References</rdf:value>            
            <dct:bibliographicCitation>Panayotova, Stella. ‘Painting Materials and Techniques in Western Illuminated  Manuscripts c. 600 -c. 1600’. In The Art and Science of Illuminated Manuscripts: A Handbook, edited by Stella Panayotova, 127–70. Turnhout: Brepols, 2020.</dct:bibliographicCitation>            
        </skos:definition>
        <skos:broader rdf:resource="http://gams.uni-graz.at/thesaurus/colorants"/>
    </skos:Concept>    
    <skos:Concept rdf:about="http://gams.uni-graz.at/thesaurus/green-earth">
        <skos:inScheme rdf:resource="http://gams.uni-graz.at/thesaurus/mss-materials"/>
        <skos:prefLabel xml:lang="de">Grüne Erde</skos:prefLabel>
        <skos:prefLabel xml:lang="en">Green earth</skos:prefLabel>
        <skos:altLabel xml:lang="en">Terre verte</skos:altLabel>
        <skos:definition xml:lang="en">Green earth is a natural inorganic pigment prepared from the complex silicate minerals glaukonite and seladonite. Other chemical elements present are Mg, Al, Fe, Ca (Kühn 1984).
            Green earth is a permanent, stable and non-reactive pigment. As other earth colourant, the preparation includes washing, grinding and picking to remove impurities (Eastaugh et al. 2008).
            The green hue depends on the local deposit and may vary from neutral green to yellowish green or greenish grey (Kühn 1984). Allegedly the best green earth was from Verona and hence called Verona green; Bohemian green had a more yellow-brown hue and was used by artist as an underlayer to flesh tones (Clemens 2007). Green earth turns brown on heating and is referred to then as burnt green earth. 
            The pigment was used already in antiquity for pottery and wall paintings (Grissom 1986). Rarely used in Northern European manuscripts, the pigment was employed extensively in Byzantine manuscripts and icons, as well as in manuscripts made between 1128 and 1130 in the Latin Kingdom of Jerusalem (Panayotova 2020).</skos:definition>
        <skos:example>https://commons.wikimedia.org/wiki/File:Gr%C3%BCnerde-_Pigment.JPG</skos:example>
        <skos:definition rdf:parseType="Resource">
            <rdf:value>References</rdf:value>
            <dct:bibliographicCitation>Kühn, Hermann. Reclams Handbuch der künstlerischen Techniken. Vol. 1. Farbmittel, Buchmalerei, Tafel-und Leinwandmalerei. 3 vols. Stuttgart: Reclam, 1984, pp. 30-31, 89.</dct:bibliographicCitation>
            <dct:bibliographicCitation>Panayotova, Stella. ‘Painting Materials and Techniques in Western Illuminated  Manuscripts c. 600 -c. 1600’. In The Art and Science of Illuminated Manuscripts: A Handbook, edited by Stella Panayotova, 127–70. Turnhout: Brepols, 2020.</dct:bibliographicCitation>
            <dct:bibliographicCitation>Grissom, Carol A. ‘Green Earth’. In Artists’ Pigments: A Handbook of Their History and Characteristics, edited by Robert L. Feller, 1:141–67. Washington, D.C.: National Gallery of Art, 1986.</dct:bibliographicCitation>
            <dct:bibliographicCitation>Eastaugh, Nicholas, Valentine Walsh, Tracey Chaplin, and Ruth Siddall. Pigment Compendium: A Dictionary and Optical Microscopy of Historical Pigments. Amsterdam: Elsevier, Butterworth-Heinemann, 2008, pp. 180-181.</dct:bibliographicCitation>
            <dct:bibliographicCitation>ColourLex https://colourlex.com/project/green-earth/</dct:bibliographicCitation>
            <dct:bibliographicCitation>Clemens, Raymond, and Timothy Graham. Introduction to Manuscript Studies. Ithaca, NY: Cornell University Press, 2007.</dct:bibliographicCitation>
            <dct:bibliographicCitation>Spectra by A. Cosentino, Cultural Heritage Science Open Source (CHSOS): https://chsopensource.org/green-earth-k-11000/</dct:bibliographicCitation>
        </skos:definition>
        <skos:related rdf:resource="http://gams.uni-graz.at/thesaurus/silicon"/>
        <skos:broader rdf:resource="http://gams.uni-graz.at/thesaurus/green-colorants"/>
    </skos:Concept>
    <skos:Concept rdf:about="http://gams.uni-graz.at/thesaurus/green-copper-colorants">
        <skos:inScheme rdf:resource="http://gams.uni-graz.at/thesaurus/mss-materials"/>
        <skos:prefLabel xml:lang="de">Grüne Kupferpigmente</skos:prefLabel>
        <skos:prefLabel xml:lang="en">Green copper-based pigments</skos:prefLabel>
        <skos:definition xml:lang="en">There is a variety of copper-based green pigments either derived from natural minerals containing copper, or produced synthetically when copper is exposed to outdoor atmosphere (air, moisture and acid) and then covered by natural patina. The copper group can be subdivided into various groups depending on their chemical structure as for instance copper carbonates (including malachite), copper sulfates and hydroxide sulfates (including brochantite), or copper halides (including atacamite) (Eastaugh et al. 2008).</skos:definition>
        <skos:definition rdf:parseType="Resource">
            <rdf:value>References</rdf:value>
            <dct:bibliographicCitation>Eastaugh, Nicholas, Valentine Walsh, Tracey Chaplin, and Ruth Siddall. Pigment Compendium: A Dictionary and Optical Microscopy of Historical Pigments. Amsterdam: Elsevier, Butterworth-Heinemann, 2008.</dct:bibliographicCitation>    
        </skos:definition>
        <skos:example>https://upload.wikimedia.org/wikipedia/commons/0/07/Patina_an_Kupfer.jpg</skos:example>
        <skos:broader rdf:resource="http://gams.uni-graz.at/thesaurus/green-colorants"/>
    </skos:Concept>
    <skos:Concept rdf:about="http://gams.uni-graz.at/thesaurus/malachite">
        <skos:inScheme rdf:resource="http://gams.uni-graz.at/thesaurus/mss-materials"/>
        <skos:prefLabel xml:lang="de">Malachit</skos:prefLabel>
        <skos:altLabel xml:lang="de">Berggrün</skos:altLabel>
        <skos:prefLabel xml:lang="en">Malachite</skos:prefLabel>
        <skos:altLabel xml:lang="en">Mountain green</skos:altLabel>
        <skos:altLabel xml:lang="en">Copper green</skos:altLabel>
        <skos:definition xml:lang="en">Malachit is a basic copper carbonate (CuCO3·Cu(OH)2). As mineral it is found often together with azurite. There are also recipes for its artificial production but the synthetic form is of lesser quality in terms both of colour and stability (Kühn 1984). As with other minerals, the production of the pigment included crushing, grinding, washing and levigating the mineral (Eastaugh et al. 2008).
            The sources of malchite in mediaeval times are not well known; the copper mines in Hungary, Central Europe and France may have been used (Eastaugh et al. 2008). Malachite has been identified in very few Western European manuscripts predating the fifteenth century. Similarly, there are exceedingly rare mentions of malachite in archival records and artists' treatises before c. 1400 (Panayotova 2020). Some modern studies explain this with the fact that malachite grind to a small grain size has a much paler green colour. Artists may have therefore preferred using synthetic copper green (Eastaugh et al. 2008).
        </skos:definition>
        <skos:example>https://commons.wikimedia.org/wiki/Category:Malachite?uselang=de#/media/File:2013-03_Malachit_aus_Gumeschewsk,_Ural_anagoria.JPG</skos:example>
        <skos:definition rdf:parseType="Resource">
            <rdf:value>References</rdf:value>
            <dct:bibliographicCitation>Kühn, Hermann. Reclams Handbuch der künstlerischen Techniken. Vol. 1. Farbmittel, Buchmalerei, Tafel-und Leinwandmalerei. 3 vols. Stuttgart: Reclam, 1984, pp. 31, 89-90.</dct:bibliographicCitation>            
            <dct:bibliographicCitation>Panayotova, Stella. ‘Painting Materials and Techniques in Western Illuminated  Manuscripts c. 600 -c. 1600’. In The Art and Science of Illuminated Manuscripts: A Handbook, edited by Stella Panayotova, 127–70. Turnhout: Brepols, 2020.</dct:bibliographicCitation>            
            <dct:bibliographicCitation>Eastaugh, Nicholas, Valentine Walsh, Tracey Chaplin, and Ruth Siddall. Pigment Compendium: A Dictionary and Optical Microscopy of Historical Pigments. Amsterdam: Elsevier, Butterworth-Heinemann, 2008.</dct:bibliographicCitation>
            <dct:bibliographicCitation>ColourLex https://colourlex.com/project/malachite/</dct:bibliographicCitation> 
            <dct:bibliographicCitation>Mindat https://www.mindat.org/min-2550.html</dct:bibliographicCitation>
            <dct:bibliographicCitation>Spectra by A. Cosentino, Cultural Heritage Science Open Source (CHSOS): https://chsopensource.org/malachite-k-10300/</dct:bibliographicCitation>
        </skos:definition>
        <skos:related rdf:resource="http://gams.uni-graz.at/thesaurus/carbon"/>
        <skos:related rdf:resource="http://gams.uni-graz.at/thesaurus/oxygen"/>
        <skos:related rdf:resource="http://gams.uni-graz.at/thesaurus/copper"/>
        <skos:broader rdf:resource="http://gams.uni-graz.at/thesaurus/green-copper-colorants"/>
    </skos:Concept>
    <skos:Concept rdf:about="http://gams.uni-graz.at/thesaurus/brochantite">
        <skos:inScheme rdf:resource="http://gams.uni-graz.at/thesaurus/mss-materials"/>
        <skos:prefLabel xml:lang="de">Brochantit</skos:prefLabel>
        <skos:prefLabel xml:lang="en">Brochantite</skos:prefLabel>
        <skos:definition xml:lang="en">Brochantite is a green copper sulfate hydroxide mineral (Cu4SO4(OH)6). The mineral is relatively common found at copper deposits in Europe, England, Morocco, Namibia (Eastaugh et al. 2008). Apart from natural occurring mineral, brochantite is found as a synthetic corrosion product on bronze sculptures.</skos:definition>
        <skos:definition rdf:parseType="Resource">
            <rdf:value>References</rdf:value>
            <dct:bibliographicCitation>Eastaugh, Nicholas, Valentine Walsh, Tracey Chaplin, and Ruth Siddall. Pigment Compendium: A Dictionary and Optical Microscopy of Historical Pigments. Amsterdam: Elsevier, Butterworth-Heinemann, 2008.</dct:bibliographicCitation>
            <dct:bibliographicCitation>CAMEO Database https://cameo.mfa.org/wiki/Brochantite</dct:bibliographicCitation> 
            <dct:bibliographicCitation>Mindat https://www.mindat.org/min-779.html</dct:bibliographicCitation>
        </skos:definition>
        <skos:example>https://upload.wikimedia.org/wikipedia/commons/e/e9/Brochantite-md75a.jpg</skos:example>
        <skos:related rdf:resource="http://gams.uni-graz.at/thesaurus/copper"/>
        <skos:related rdf:resource="http://gams.uni-graz.at/thesaurus/sulfur"/>
        <skos:related rdf:resource="http://gams.uni-graz.at/thesaurus/oxygen"/>
        <skos:related rdf:resource="http://gams.uni-graz.at/thesaurus/hydrogen"/>
        <skos:broader rdf:resource="http://gams.uni-graz.at/thesaurus/green-copper-colorants"/>
    </skos:Concept>
    <skos:Concept rdf:about="http://gams.uni-graz.at/thesaurus/atacamite">
        <skos:inScheme rdf:resource="http://gams.uni-graz.at/thesaurus/mss-materials"/>
        <skos:prefLabel xml:lang="de">Atacamit</skos:prefLabel>
        <skos:prefLabel xml:lang="en">Atacamite</skos:prefLabel>
        <skos:definition xml:lang="en">Atacamite is a relatively rare copper mineral with the formula Cu2Cl(OH)3. As synthetic pigment it occurs as patina or alteration on bronze and copper material. It is probably the synthetic form (copper chloride hydroxide, atacamite type) that was used as pigment in medieval illuminations, as attested by numerous medaeval recipes for green copper pigment (Eastaugh et al. 2008). 
        </skos:definition>
        <skos:definition rdf:parseType="Resource">
            <rdf:value>References</rdf:value>
            <dct:bibliographicCitation>Eastaugh, Nicholas, Valentine Walsh, Tracey Chaplin, and Ruth Siddall. Pigment Compendium: A Dictionary and Optical Microscopy of Historical Pigments. Amsterdam: Elsevier, Butterworth-Heinemann, 2008.</dct:bibliographicCitation>
            <dct:bibliographicCitation>CAMEO Database https://cameo.mfa.org/wiki/Atacamite</dct:bibliographicCitation>            
        </skos:definition>
        <skos:example>https://upload.wikimedia.org/wikipedia/commons/4/4e/Atacamite-235102.jpg</skos:example>
        <skos:related rdf:resource="http://gams.uni-graz.at/thesaurus/copper"/>
        <skos:related rdf:resource="http://gams.uni-graz.at/thesaurus/chlorine"/>
        <skos:related rdf:resource="http://gams.uni-graz.at/thesaurus/oxygen"/>
        <skos:related rdf:resource="http://gams.uni-graz.at/thesaurus/hydrogen"/>
        <skos:broader rdf:resource="http://gams.uni-graz.at/thesaurus/green-copper-colorants"/>
    </skos:Concept>
    <skos:Concept rdf:about="http://gams.uni-graz.at/thesaurus/verdigris">
        <skos:inScheme rdf:resource="http://gams.uni-graz.at/thesaurus/mss-materials"/>
        <skos:prefLabel xml:lang="de">Grünspan</skos:prefLabel>
        <skos:prefLabel xml:lang="en">Verdigris</skos:prefLabel>
        <skos:definition xml:lang="en">Verdigris is a collective name for various copper-based greens including copper acetate compounds but also copper carbonate and chloride compounds. They were produced synthetically by placing copper plates over acidic damp (hot vinegar, distilled wine or urine) and scraping off the encrustination from the surface. The product can then be further refined by dissolution in vinegar and subsequent recrystallisation through evaporation (Eastaugh et al. 2008). Depending on the exact chemical composition its colour can vary from deep sea green to yellowish-green, blue-green or whitish bright green (Kühn 1984). 
            Used in manuscript illumination, verdigris is highly unstable as it can crumble and flake off. Moreover it is often corrosive and can 'eat through' the writing support (Panayotova 2020). Although its incompatibility with lead-containing pigments was well-known, artists from the eleventh century onwards tried to modify the hue of verdigris with lead white but by also adding organic yellows to stabilise the mixture (Panayotova 2020). Another shortcoming is that the pigment darkens when mixed with sulfur-containing pigments such as ultramarine or orpiment (ColourLex).</skos:definition>
        <skos:definition rdf:parseType="Resource">
            <rdf:value>References</rdf:value>
            <dct:bibliographicCitation>Kühn, Hermann. Reclams Handbuch der künstlerischen Techniken. Vol. 1. Farbmittel, Buchmalerei, Tafel-und Leinwandmalerei. 3 vols. Stuttgart: Reclam, 1984, pp. 31-32, 90-91.</dct:bibliographicCitation>            
            <dct:bibliographicCitation>Panayotova, Stella. ‘Painting Materials and Techniques in Western Illuminated  Manuscripts c. 600 -c. 1600’. In The Art and Science of Illuminated Manuscripts: A Handbook, edited by Stella Panayotova, 127–70. Turnhout: Brepols, 2020.</dct:bibliographicCitation>            
            <dct:bibliographicCitation>Eastaugh, Nicholas, Valentine Walsh, Tracey Chaplin, and Ruth Siddall. Pigment Compendium: A Dictionary and Optical Microscopy of Historical Pigments. Amsterdam: Elsevier, Butterworth-Heinemann, 2008.</dct:bibliographicCitation>
            <dct:bibliographicCitation>ColourLex https://colourlex.com/project/verdigris/</dct:bibliographicCitation>  
            <dct:bibliographicCitation>Spectra by A. Cosentino, Cultural Heritage Science Open Source (CHSOS): https://chsopensource.org/verdigris-k-44450/</dct:bibliographicCitation>
        </skos:definition>
        <skos:example>https://commons.wikimedia.org/wiki/File:Copper(II)-acetate.jpg</skos:example>
        <skos:related rdf:resource="http://gams.uni-graz.at/thesaurus/copper"/>
        <skos:related rdf:resource="http://gams.uni-graz.at/thesaurus/carbon"/>
        <skos:related rdf:resource="http://gams.uni-graz.at/thesaurus/oxygen"/>
        <skos:related rdf:resource="http://gams.uni-graz.at/thesaurus/hydrogen"/>
        <skos:broader rdf:resource="http://gams.uni-graz.at/thesaurus/green-copper-colorants"/>
    </skos:Concept>
    <skos:Concept rdf:about="http://gams.uni-graz.at/thesaurus/vergaut">
        <skos:inScheme rdf:resource="http://gams.uni-graz.at/thesaurus/mss-materials"/>
        <skos:prefLabel xml:lang="de">Vergaut</skos:prefLabel>
        <skos:prefLabel xml:lang="en">Vergaut</skos:prefLabel>
        <skos:definition xml:lang="en">Vergaut is a generic term for pigment mixtures using blue and yellow. Heraclius (Lib. III, 56) for instance suggests mixing orpiment with indigo or ultramarine, yellow ochre with indigo or verdigris. Cennini (ch. XLVIIII) advices for using a mixture of verdigris and saffron to make "the most perfect grass color imaginable". He also gives recipes for mixing orpiment with indigo (ch. LIII), azurite and 'giallorino' (ch. LIIII), ultramarine and orpiment (ch. LV), lead-white or lime white and green earth (LVII).</skos:definition>
        <skos:definition rdf:parseType="Resource">
            <rdf:value>References</rdf:value>
            <dct:bibliographicCitation>Kühn, Hermann. Reclams Handbuch der künstlerischen Techniken. Vol. 1. Farbmittel, Buchmalerei, Tafel-und Leinwandmalerei. 3 vols. Stuttgart: Reclam, 1984, p. 91, 91.</dct:bibliographicCitation>            
            <dct:bibliographicCitation>Panayotova, Stella. ‘Painting Materials and Techniques in Western Illuminated  Manuscripts c. 600 -c. 1600’. In The Art and Science of Illuminated Manuscripts: A Handbook, edited by Stella Panayotova, 127–70. Turnhout: Brepols, 2020.</dct:bibliographicCitation> 
            <dct:bibliographicCitation>Cennini, Cennino. The Craftsman’s Handbook: The Italian "Il Libro Dell’ Arte. Edited by Daniel Varney Thompson. New York: Dover, 1933.</dct:bibliographicCitation>
        </skos:definition>
        <skos:broader rdf:resource="http://gams.uni-graz.at/thesaurus/green-colorants"/>
    </skos:Concept>
    <skos:Concept rdf:about="http://gams.uni-graz.at/thesaurus/green-colorants-organic">
        <skos:inScheme rdf:resource="http://gams.uni-graz.at/thesaurus/mss-materials"/>
        <skos:prefLabel xml:lang="de">Grüne organische Farbmittel</skos:prefLabel>
        <skos:prefLabel xml:lang="en">Organic green colourants</skos:prefLabel>
        <skos:definition xml:lang="en">There are a few organic green colorants. Green on the basis of chlorophyll is a cheap and easy to extract, but also less light-resistant. Artists' treatises mention various plants as sources for green colourants such as iris, buckthorn berries, cabbage, leek, elderberry, rue, parsley and columbine, honeysuckle and nightshade (Kühn 1984; Eastaugh et al. 2008).</skos:definition>
        <skos:definition rdf:parseType="Resource">
            <rdf:value>References</rdf:value>
            <dct:bibliographicCitation>Kühn, Hermann. Reclams Handbuch der künstlerischen Techniken. Vol. 1. Farbmittel, Buchmalerei, Tafel-und Leinwandmalerei. 3 vols. Stuttgart: Reclam, 1984, pp. 92-93.</dct:bibliographicCitation>
            <dct:bibliographicCitation>Eastaugh, Nicholas, Valentine Walsh, Tracey Chaplin, and Ruth Siddall. Pigment Compendium: A Dictionary and Optical Microscopy of Historical Pigments. Amsterdam: Elsevier, Butterworth-Heinemann, 2008.</dct:bibliographicCitation>
        </skos:definition>
        <skos:broader rdf:resource="http://gams.uni-graz.at/thesaurus/green-colorants"/>
    </skos:Concept>
    <skos:Concept rdf:about="http://gams.uni-graz.at/thesaurus/weld-indigo">
        <skos:inScheme rdf:resource="http://gams.uni-graz.at/thesaurus/mss-materials"/>
        <skos:prefLabel xml:lang="de">Färber-Wau mit Indigo</skos:prefLabel>
        <skos:prefLabel xml:lang="en">Weld with indigo</skos:prefLabel>
        <skos:definition xml:lang="en">Mixture of weld (plant reseda luteola) and indigo.</skos:definition>
        <skos:related rdf:resource="http://gams.uni-graz.at/thesaurus/nitrogen"/>
        <skos:related rdf:resource="http://gams.uni-graz.at/thesaurus/carbon"/>
        <skos:related rdf:resource="http://gams.uni-graz.at/thesaurus/oxygen"/>
        <skos:related rdf:resource="http://gams.uni-graz.at/thesaurus/hydrogen"/>
        <skos:broader rdf:resource="http://gams.uni-graz.at/thesaurus/green-colorants-organic"/>
    </skos:Concept>
    <skos:Concept rdf:about="http://gams.uni-graz.at/thesaurus/iris-green">
        <skos:inScheme rdf:resource="http://gams.uni-graz.at/thesaurus/mss-materials"/>
        <skos:prefLabel xml:lang="de">Schwertlilien (Iris) grün</skos:prefLabel>
        <skos:prefLabel xml:lang="en">Iris green</skos:prefLabel>
        <skos:definition xml:lang="en">The dye is extracted from the petals of iris flowers. In mediaeval sources sometimes the dye is referred to as sap green. The dye was prepared for use either as clothlet (a piece of linen dipped into the juice) or by extracting the juice and mixing it with an aluminium hydroxide (alum) base (Eastaugh et al. 2008). Some recipes call for adding giallorino - lead-tin yellow - to get a more green and less green blue colour).</skos:definition>
        <skos:definition rdf:parseType="Resource">
            <rdf:value>References</rdf:value>            
            <dct:bibliographicCitation>Eastaugh, Nicholas, Valentine Walsh, Tracey Chaplin, and Ruth Siddall. Pigment Compendium: A Dictionary and Optical Microscopy of Historical Pigments. Amsterdam: Elsevier, Butterworth-Heinemann, 2008.</dct:bibliographicCitation>
        </skos:definition>
        <skos:related rdf:resource="http://gams.uni-graz.at/thesaurus/carbon"/>
        <skos:related rdf:resource="http://gams.uni-graz.at/thesaurus/oxygen"/>
        <skos:related rdf:resource="http://gams.uni-graz.at/thesaurus/hydrogen"/>
        <skos:broader rdf:resource="http://gams.uni-graz.at/thesaurus/green-colorants-organic"/>
    </skos:Concept>    
    <skos:Concept rdf:about="http://gams.uni-graz.at/thesaurus/buckthorn-berries-green">
        <skos:inScheme rdf:resource="http://gams.uni-graz.at/thesaurus/mss-materials"/>
        <skos:prefLabel xml:lang="de">Kreuzdornbeeren (reif)</skos:prefLabel>
        <skos:prefLabel xml:lang="en">Buckthorn berries ripe</skos:prefLabel>
        <skos:definition xml:lang="en">An organic green is also made from the ripe berries of various species of the Rhamnaceae family (most common species throughout Europe were the Rhamnus catharticus). As a lake the pigment was quite popular with a wide geographical production (Eastaugh et al. 2008).</skos:definition>
        <skos:definition rdf:parseType="Resource">
            <rdf:value>References</rdf:value>
            <dct:bibliographicCitation>Eastaugh, Nicholas, Valentine Walsh, Tracey Chaplin, and Ruth Siddall. Pigment Compendium: A Dictionary and Optical Microscopy of Historical Pigments. Amsterdam: Elsevier, Butterworth-Heinemann, 2008.</dct:bibliographicCitation>
            <dct:bibliographicCitation>Material Archiv https://materialarchiv.ch/de/ma:material_2118/</dct:bibliographicCitation> 
        </skos:definition>
        <skos:example>https://commons.wikimedia.org/wiki/File:Rhamnus_catharticus_leaves_and_fruit.jpg</skos:example>
        <skos:related rdf:resource="http://gams.uni-graz.at/thesaurus/aluminium"/>
        <skos:related rdf:resource="http://gams.uni-graz.at/thesaurus/kalium"/>
        <skos:related rdf:resource="http://gams.uni-graz.at/thesaurus/sulfur"/>
        <skos:related rdf:resource="http://gams.uni-graz.at/thesaurus/oxygen"/>
        <skos:related rdf:resource="http://gams.uni-graz.at/thesaurus/hydrogen"/>
        <skos:broader rdf:resource="http://gams.uni-graz.at/thesaurus/green-colorants-organic"/>
    </skos:Concept>
    
    <!-- #############  BROWN  #############  -->
    <skos:Concept rdf:about="http://gams.uni-graz.at/thesaurus/brown-colorants">
        <skos:inScheme rdf:resource="http://gams.uni-graz.at/thesaurus/mss-materials"/>
        <skos:prefLabel xml:lang="de">Braune Farbmittel</skos:prefLabel>
        <skos:prefLabel xml:lang="en">Brown colorants</skos:prefLabel>
        <skos:definition xml:lang="en">Brown colours are often produced by mixing red, yellow, blue and black colourants together. There are also natural occurring brown pigments, the most common being brown ochre and umber, which receive their brown colour due to the iron and manganese content.</skos:definition>
        <skos:example>https://upload.wikimedia.org/wikipedia/commons/e/ef/Brown_tints_and_shades.svg</skos:example>
        <skos:broader rdf:resource="http://gams.uni-graz.at/thesaurus/colorants"/>
    </skos:Concept>
    <skos:Concept rdf:about="http://gams.uni-graz.at/thesaurus/organic-brown-colorants">
        <skos:inScheme rdf:resource="http://gams.uni-graz.at/thesaurus/mss-materials"/>
        <skos:prefLabel xml:lang="de">Organische braune Farbmittel</skos:prefLabel>
        <skos:prefLabel xml:lang="en">Organic brown colorants</skos:prefLabel>
        <skos:definition xml:lang="en">Among the organic brown colorants are sepia and bister, which came in use during the late middle ages.</skos:definition>
        <skos:broader rdf:resource="http://gams.uni-graz.at/thesaurus/brown-colorants"/>
    </skos:Concept>
    <skos:Concept rdf:about="http://gams.uni-graz.at/thesaurus/sepia">
        <skos:inScheme rdf:resource="http://gams.uni-graz.at/thesaurus/mss-materials"/>
        <skos:prefLabel xml:lang="de">Sepia</skos:prefLabel>
        <skos:prefLabel xml:lang="en">Sepia</skos:prefLabel>
        <skos:definition xml:lang="en">Sepia is a brown organic pigment produced from the ink of the cuttlefish (Sepia officinalis). </skos:definition>
        <skos:definition rdf:parseType="Resource">
            <rdf:value>References</rdf:value>
            <dct:bibliographicCitation>Eastaugh, Nicholas, Valentine Walsh, Tracey Chaplin, and Ruth Siddall. Pigment Compendium: A Dictionary and Optical Microscopy of Historical Pigments. Amsterdam: Elsevier, Butterworth-Heinemann, 2008.</dct:bibliographicCitation>
            <dct:bibliographicCitation>Ricciardi, Paola, and Kristine Rose Beers. ‘The Illuminators’ Palette’. In Colour : The Art and Science of Illuminated Manuscripts, edited by Stella Panayotova, Deirdre Elizabeth Jackson, and Paola Ricciardi, 27–73. Turnhout: Brepols, 2016.</dct:bibliographicCitation>   
            <dct:bibliographicCitation>Spectra by A. Cosentino, Cultural Heritage Science Open Source (CHSOS): https://chsopensource.org/sepia-k-12401/</dct:bibliographicCitation>
        </skos:definition>
        <skos:related rdf:resource="http://gams.uni-graz.at/thesaurus/oxygen"/>
        <skos:related rdf:resource="http://gams.uni-graz.at/thesaurus/hydrogen"/>
        <skos:related rdf:resource="http://gams.uni-graz.at/thesaurus/nitrogen"/>
        <skos:broader rdf:resource="http://gams.uni-graz.at/thesaurus/organic-brown-colorants"/>
    </skos:Concept>
   <skos:Concept rdf:about="http://gams.uni-graz.at/thesaurus/bister">
        <skos:inScheme rdf:resource="http://gams.uni-graz.at/thesaurus/mss-materials"/>
        <skos:prefLabel xml:lang="de">Bister</skos:prefLabel>
        <skos:prefLabel xml:lang="en">Bister</skos:prefLabel>
        <skos:definition xml:lang="en">Bister is a carbon-based brown-black pigment produced from the soot of burnt wood, tar and resin. The soot is washed with water and allowed to settle; then collected and dried (Winter et al. 2007). Bister was used in manuscript illumination since at least the fourteenth century (Ball 2002).</skos:definition>
       <skos:definition rdf:parseType="Resource">
            <rdf:value>References</rdf:value>
            <dct:bibliographicCitation>Winter, John, and Elisabeth West FitzHugh. ‘Pigments Based on Carbon’. In Artists’ Pigments. A Handbook of Their History and Characteristics, edited by Barbara H. Berrie, 4:1–37. Washington: National Gallery of Art, 2007.</dct:bibliographicCitation>
            <dct:bibliographicCitation>Kühn, Hermann. Reclams Handbuch der künstlerischen Techniken. Vol. 1. Farbmittel, Buchmalerei, Tafel-und Leinwandmalerei. 3 vols. Stuttgart: Reclam, 1984, p. 41.</dct:bibliographicCitation>
            <dct:bibliographicCitation>Eastaugh, Nicholas, Valentine Walsh, Tracey Chaplin, and Ruth Siddall. Pigment Compendium: A Dictionary and Optical Microscopy of Historical Pigments. Amsterdam: Elsevier, Butterworth-Heinemann, 2008.</dct:bibliographicCitation>
            <dct:bibliographicCitation>Ball, Philip. Bright earth : art and the invention of color. London: Viking, 2001.</dct:bibliographicCitation>
            <dct:bibliographicCitation>ColourLex https://colourlex.com/project/bister-bistre/</dct:bibliographicCitation>    
        </skos:definition>
       <skos:example>https://commons.wikimedia.org/wiki/File:Jhfragonard2.jpg</skos:example>
       <skos:related rdf:resource="http://gams.uni-graz.at/thesaurus/carbon"/>
       <skos:broader rdf:resource="http://gams.uni-graz.at/thesaurus/organic-brown-colorants"/>
    </skos:Concept>    
    <skos:Concept rdf:about="http://gams.uni-graz.at/thesaurus/brown-ochre">
        <skos:inScheme rdf:resource="http://gams.uni-graz.at/thesaurus/mss-materials"/>
        <skos:prefLabel xml:lang="de">Braunocker</skos:prefLabel>
        <skos:altLabel xml:lang="de">Brauner Ocker</skos:altLabel>
        <skos:prefLabel xml:lang="en">Brown Ochre</skos:prefLabel>
        <skos:altLabel xml:lang="en">Brown Ocher</skos:altLabel>
        <skos:definition xml:lang="en"></skos:definition>
        <skos:definition rdf:parseType="Resource">
            <rdf:value>References</rdf:value>
            <dct:bibliographicCitation>Kühn, Hermann. Reclams Handbuch der künstlerischen Techniken. Vol. 1. Farbmittel, Buchmalerei, Tafel-und Leinwandmalerei. 3 vols. Stuttgart: Reclam, 1984, pp. , .</dct:bibliographicCitation>
            <dct:bibliographicCitation>Eastaugh, Nicholas, Valentine Walsh, Tracey Chaplin, and Ruth Siddall. Pigment Compendium: A Dictionary and Optical Microscopy of Historical Pigments. Amsterdam: Elsevier, Butterworth-Heinemann, 2008.</dct:bibliographicCitation>
            <dct:bibliographicCitation>Material Archiv </dct:bibliographicCitation>
            <dct:bibliographicCitation>ColourLex </dct:bibliographicCitation>    
        </skos:definition>
        <skos:example></skos:example>
        <skos:related rdf:resource="http://gams.uni-graz.at/thesaurus/iron"/>
        <skos:related rdf:resource="http://gams.uni-graz.at/thesaurus/silicon"/>
        <skos:related rdf:resource="http://gams.uni-graz.at/thesaurus/oxygen"/>
        <skos:broader rdf:resource="http://gams.uni-graz.at/thesaurus/brown-colorants"/>
    </skos:Concept>
    <skos:Concept rdf:about="http://gams.uni-graz.at/thesaurus/brown-earth">
        <skos:inScheme rdf:resource="http://gams.uni-graz.at/thesaurus/mss-materials"/>
        <skos:prefLabel xml:lang="de">Braune Erde</skos:prefLabel>
        <skos:prefLabel xml:lang="en">Brown earth</skos:prefLabel>
        <skos:altLabel xml:lang="en">Manganese brown</skos:altLabel>
        <skos:definition xml:lang="en"></skos:definition>
        <skos:definition rdf:parseType="Resource">
            <rdf:value>References</rdf:value>
            <dct:bibliographicCitation>Kühn, Hermann. Reclams Handbuch der künstlerischen Techniken. Vol. 1. Farbmittel, Buchmalerei, Tafel-und Leinwandmalerei. 3 vols. Stuttgart: Reclam, 1984.</dct:bibliographicCitation>
            <dct:bibliographicCitation>Eastaugh, Nicholas, Valentine Walsh, Tracey Chaplin, and Ruth Siddall. Pigment Compendium: A Dictionary and Optical Microscopy of Historical Pigments. Amsterdam: Elsevier, Butterworth-Heinemann, 2008.</dct:bibliographicCitation>
            <dct:bibliographicCitation>Material Archiv </dct:bibliographicCitation>
            <dct:bibliographicCitation>ColourLex </dct:bibliographicCitation>    
        </skos:definition>
        <skos:example></skos:example>
        <skos:broader rdf:resource="http://gams.uni-graz.at/thesaurus/brown-colorants"/>
    </skos:Concept>
    <skos:Concept rdf:about="http://gams.uni-graz.at/thesaurus/umber">
        <skos:inScheme rdf:resource="http://gams.uni-graz.at/thesaurus/mss-materials"/>
        <skos:prefLabel xml:lang="de">Umbra</skos:prefLabel>
        <skos:prefLabel xml:lang="en">Umber</skos:prefLabel>
        <skos:altLabel xml:lang="en">Burnt umber</skos:altLabel>
        <skos:definition xml:lang="en">Umber is a generic term for sedimentary mineral substance with a significant manganese oxide content besides iron oxides. It is the high amount of manganese compounds (5 to 20%) which defines a sedimentary rock as an umber and not as ochre. Umber in sensu stricto sediment occurs in limited geographical regions and the principal source are deposits in Cyprus, Levant and the Middle East. Under the term umber may be included, however, also weathering and alteration product of magnesian limestones, deposits of which are found in central England (Eastaugh et al. 2008).
            The ground pigment  is prepared by washing, levigation and drying. Calcinated umber, often referred to as burnt umber, has a more dark red colour. Compatible with all other pigments, it was used on its own (especially to create shadows) or to darken other colours.
            Thompson (1956) suggest that umber was introduce into general use in Europe before the close of the fifteenth century. According to Helwig (2007) while the general term 'brown earth' was used in earlier treatises, the more specific name 'umber' did not appear until the sixteenth cenutry; the brown pigment containing manganese and iron is identified in sixteenth-century paintings.
            </skos:definition>
        <skos:definition rdf:parseType="Resource">
            <rdf:value>References</rdf:value>            
            <dct:bibliographicCitation>Eastaugh, Nicholas, Valentine Walsh, Tracey Chaplin, and Ruth Siddall. Pigment Compendium: A Dictionary and Optical Microscopy of Historical Pigments. Amsterdam: Elsevier, Butterworth-Heinemann, 2008.</dct:bibliographicCitation>
            <dct:bibliographicCitation>Helwig, Kate. ‘Iron Oxide Pigments’. In Artists’ Pigments. A Handbook of Their History and Characteristics, edited by Barbara H. Berrie, 4:39–109. Washington: National Gallery of Art, 2007.</dct:bibliographicCitation>
            <dct:bibliographicCitation>Thompson, Daniel Varney. The Materials and Techniques of Medieval Painting. Edited by Bernard Berenson. New York: Dover Publications, 1956.</dct:bibliographicCitation>
            <dct:bibliographicCitation>Material Archiv https://materialarchiv.ch/de/ma:material_1720/</dct:bibliographicCitation>
            <dct:bibliographicCitation>ColourLex https://colourlex.com/project/umber/</dct:bibliographicCitation> 
            <dct:bibliographicCitation>Spectra by A. Cosentino, Cultural Heritage Science Open Source (CHSOS): https://chsopensource.org/raw-umber-k-40610/</dct:bibliographicCitation>
        </skos:definition>
        <skos:example>https://upload.wikimedia.org/wikipedia/commons/5/54/Terra_ombra_naturale_umber.jpg</skos:example>
        <skos:related rdf:resource="http://gams.uni-graz.at/thesaurus/iron"/>
        <skos:related rdf:resource="http://gams.uni-graz.at/thesaurus/manganese"/>
        <skos:related rdf:resource="http://gams.uni-graz.at/thesaurus/oxygen"/>
        <skos:broader rdf:resource="http://gams.uni-graz.at/thesaurus/brown-earth"/>
    </skos:Concept>
    
    <!-- #############  BLACK  #############  -->
    <skos:Concept rdf:about="http://gams.uni-graz.at/thesaurus/black-colorants">
        <skos:inScheme rdf:resource="http://gams.uni-graz.at/thesaurus/mss-materials"/>
        <skos:prefLabel xml:lang="de">Schwarze Farbmittel</skos:prefLabel>
        <skos:prefLabel xml:lang="en">Black colorants</skos:prefLabel>
        <skos:definition xml:lang="en">Among black colorants carbon-based black pigments were probably the most easily available and widely used for writing as inks and pigments. Apart from using black colourants, one could also mix dark blue and red pigments or use them in combination with black ones to achieve a wide range of shades of black.</skos:definition>
        <skos:example>https://upload.wikimedia.org/wikipedia/commons/2/26/Black_tints_and_shades.svg</skos:example>
        <skos:broader rdf:resource="http://gams.uni-graz.at/thesaurus/colorants"/>
    </skos:Concept>
    <skos:Concept rdf:about="http://gams.uni-graz.at/thesaurus/iron-gall">
        <skos:inScheme rdf:resource="http://gams.uni-graz.at/thesaurus/mss-materials"/>
        <skos:prefLabel xml:lang="de">Eisengallustinte</skos:prefLabel>
        <skos:altLabel xml:lang="de">Gallustinte</skos:altLabel>
        <skos:prefLabel xml:lang="en">Iron-gall</skos:prefLabel>
        <skos:altLabel xml:lang="en">Iron gall ink</skos:altLabel>
        <skos:altLabel xml:lang="en">Oak gall ink</skos:altLabel>
        <skos:altLabel xml:lang="en">Iron gall nut ink</skos:altLabel>
        <skos:altLabel xml:lang="en">Tannine ink</skos:altLabel>
        <skos:definition xml:lang="en">Iron gall ink is primarily made from tannin (plant-based mordant), vitriol (iron sulfate), gum, and water. To prevent mold one added also carbolic acid, vinegar, alcohol, cloves, different salts or alum. There are numerous sources of tannin, which can be used for the production of ink. The usual source is, however, oak galls, created by parasites which lay eggs on the leaf buds of oak trees. 
            The mixture reacts with the writing surface so that it cannot be accidentally erased. The mixture is usually used as ink (incaustum) but also used to temper colourants.</skos:definition>
        <skos:example>https://upload.wikimedia.org/wikipedia/commons/7/75/Oak_galls_and_iron%28II%29_sulfate_-_California_State_Archives.jpg</skos:example>
        <skos:related rdf:resource="http://gams.uni-graz.at/thesaurus/oxygen"/>
        <skos:related rdf:resource="http://gams.uni-graz.at/thesaurus/iron"/>
        <skos:related rdf:resource="http://gams.uni-graz.at/thesaurus/sulfur"/>
        <skos:broader rdf:resource="http://gams.uni-graz.at/thesaurus/black-colorants"/>
        <skos:definition rdf:parseType="Resource">
            <rdf:value>References</rdf:value>
            <dct:bibliographicCitation>The Iron Gall Ink Website https://irongallink.org/index.html</dct:bibliographicCitation>   
            <dct:bibliographicCitation>Spectra by A. Cosentino, Cultural Heritage Science Open Source (CHSOS): https://chsopensource.org/iron-gall-ink-k12030/</dct:bibliographicCitation>
        </skos:definition>       
    </skos:Concept>
    <skos:Concept rdf:about="http://gams.uni-graz.at/thesaurus/black-ink-mixtures">
        <skos:inScheme rdf:resource="http://gams.uni-graz.at/thesaurus/mss-materials"/>
        <skos:prefLabel xml:lang="de">Mischungen aus Eisengallustinte und Rußschwarz</skos:prefLabel>
        <skos:prefLabel xml:lang="en">Mixtures of carbon-based black and iron gall</skos:prefLabel>
        <skos:altLabel xml:lang="en">Compound ink</skos:altLabel>
        <skos:altLabel xml:lang="en">Carbon-tannin ink</skos:altLabel>
        <skos:definition xml:lang="en">A mixture of carbon-based and iron-gall substances combines the qualities of both inks - the reactive nature of the iron-gall and the thick structure of carbon-based colourants. A basic recipe would include carbon-based black as for instance soot, to which would be added gum, tannic and sulphate solutions.</skos:definition>
        <skos:broader rdf:resource="http://gams.uni-graz.at/thesaurus/black-colorants"/>
    </skos:Concept>
    <skos:Concept rdf:about="http://gams.uni-graz.at/thesaurus/carbon-based-black">
        <skos:inScheme rdf:resource="http://gams.uni-graz.at/thesaurus/mss-materials"/>
        <skos:prefLabel xml:lang="de">Rußschwarz</skos:prefLabel>
        <skos:altLabel xml:lang="de">Rußtinte</skos:altLabel>
        <skos:altLabel xml:lang="de">Ruß</skos:altLabel>
        <skos:prefLabel xml:lang="en">Carbon-based black pigments and inks</skos:prefLabel>
        <skos:altLabel xml:lang="en">Carbon-based black ink</skos:altLabel>
        <skos:altLabel xml:lang="en">Carbon ink</skos:altLabel>
        <skos:definition xml:lang="en">The group of carbon-based pigments comprises black or dark-brown writing and drawing pigments composed primarily of carbon. Depending on their preparation or nature occurrence carbon-based blacks can be divided into 1) chars, produced by carbonised plant ingredients (vegetable or plant blacks, charcoal); 2) cokes, made from animal material and yeasts (bone and ivory black); 3) flame carbons, produced in gas phase (lampblack) and 4) the natural occurring ones (graphite) (Eastaugh et al. 2008; Winter et al. 2007). 
            In order to produce an ink or colourant one needed a binder - gum arabicum sometimes in combination with milk, or egg glair. Carbon blacks are stable pigments, lightfast and compatible with all other pigments. However unlike iron gall ink it does not react with the writing surface and can be relatively easy washed off.</skos:definition>
        <skos:definition rdf:parseType="Resource">
            <rdf:value>References</rdf:value>
            <dct:bibliographicCitation>Eastaugh, Nicholas, Valentine Walsh, Tracey Chaplin, and Ruth Siddall. Pigment Compendium: A Dictionary and Optical Microscopy of Historical Pigments. Amsterdam: Elsevier, Butterworth-Heinemann, 2008.</dct:bibliographicCitation>
            <dct:bibliographicCitation>Winter, John, and Elisabeth West FitzHugh. ‘Pigments Based on Carbon’. In Artists’ Pigments. A Handbook of Their History and Characteristics, edited by Barbara H. Berrie, 4:1–37. Washington: National Gallery of Art, 2007.</dct:bibliographicCitation>    
        </skos:definition> 
        <skos:example>https://en.wikipedia.org/wiki/Carbon_black#/media/File:Carbon_black.jpg</skos:example>
        <skos:related rdf:resource="http://gams.uni-graz.at/thesaurus/carbon"/>
        <skos:broader rdf:resource="http://gams.uni-graz.at/thesaurus/black-colorants"/>
    </skos:Concept>
    <skos:Concept rdf:about="http://gams.uni-graz.at/thesaurus/graphite">
        <skos:inScheme rdf:resource="http://gams.uni-graz.at/thesaurus/mss-materials"/>
        <skos:prefLabel xml:lang="de">Graphit</skos:prefLabel>
        <skos:prefLabel xml:lang="en">Graphite</skos:prefLabel>
        <skos:definition xml:lang="en">Graphite, also known as black lead, occurs as a mineral and can be manufactured. (Winter et al. 2007). There are natural deposits worldwide (Eastaugh et al. 2008).
            Graphite was used in art from early on and has been detected on Greek pottery from the fifth millennium B.C.E. In medieval and Renaissance art it has been identified as pigment only in mural paintings (Winter et al. 2007).</skos:definition>
        <skos:definition rdf:parseType="Resource">
            <rdf:value>References</rdf:value>
            <dct:bibliographicCitation>Eastaugh, Nicholas, Valentine Walsh, Tracey Chaplin, and Ruth Siddall. Pigment Compendium: A Dictionary and Optical Microscopy of Historical Pigments. Amsterdam: Elsevier, Butterworth-Heinemann, 2008.</dct:bibliographicCitation>
            <dct:bibliographicCitation>Kühn, Hermann. Reclams Handbuch der künstlerischen Techniken. Vol. 1. Farbmittel, Buchmalerei, Tafel-und Leinwandmalerei. 3 vols. Stuttgart: Reclam, 1984.</dct:bibliographicCitation>
            <dct:bibliographicCitation>Winter, John, and Elisabeth West FitzHugh. ‘Pigments Based on Carbon’. In Artists’ Pigments. A Handbook of Their History and Characteristics, edited by Barbara H. Berrie, 4:1–37. Washington: National Gallery of Art, 2007.</dct:bibliographicCitation> 
            <dct:bibliographicCitation>Colourlex https://colourlex.com/project/graphite/</dct:bibliographicCitation>
        </skos:definition>
        <skos:example>https://upload.wikimedia.org/wikipedia/commons/3/3d/Graphite-233436.jpg</skos:example>
        <skos:related rdf:resource="http://gams.uni-graz.at/thesaurus/carbon"/>
        <skos:broader rdf:resource="http://gams.uni-graz.at/thesaurus/carbon-based-black"/>
    </skos:Concept>
    <skos:Concept rdf:about="http://gams.uni-graz.at/thesaurus/lampblack">
        <skos:inScheme rdf:resource="http://gams.uni-graz.at/thesaurus/mss-materials"/>
        <skos:prefLabel xml:lang="de">Lampenschwarz</skos:prefLabel>
        <skos:altLabel xml:lang="de">Flammruss</skos:altLabel>
        <skos:prefLabel xml:lang="en">Lampblack</skos:prefLabel>
        <skos:altLabel xml:lang="en">Lamp black</skos:altLabel>
        <skos:altLabel xml:lang="en">Lamp-black</skos:altLabel>
        <skos:altLabel xml:lang="en">Soot</skos:altLabel>
        <skos:definition xml:lang="en">Lampblack is produced by collecting carbon from a soothing flame (Winter et al. 2007). The material (usually oils or resin) is not burn completely (incomplete combustion) but the fine carbon particles remain as soot along with other unburned chemicals. It was originally made from soot collected from oil lamps, hence the name. Winter (1983) proposed a stricter distinction between 'lamp black' - products made by burning oil at a wick, and soot - carbon pigment made by burning wood. The narrow definition in modern technology for carbon pigments made by the burning or pyrolysis of gas and oil is 'carbon black' (Winter et al. 2007). 
            The very fine particles give an intense black color with extreme opacity. As other carbon-based pigment it is stable, lightfast and compatible with all other pigments.
        </skos:definition>
        <skos:definition rdf:parseType="Resource">
            <rdf:value>References</rdf:value>            
            <dct:bibliographicCitation>Winter, John, and Elisabeth West FitzHugh. ‘Pigments Based on Carbon’. In Artists’ Pigments. A Handbook of Their History and Characteristics, edited by Barbara H. Berrie, 4:1–37. Washington: National Gallery of Art, 2007.</dct:bibliographicCitation>
            <dct:bibliographicCitation>Eastaugh, Nicholas, Valentine Walsh, Tracey Chaplin, and Ruth Siddall. Pigment Compendium: A Dictionary and Optical Microscopy of Historical Pigments. Amsterdam: Elsevier, Butterworth-Heinemann, 2008.</dct:bibliographicCitation>
            <dct:bibliographicCitation>Colourlex https://colourlex.com/project/lampblack/</dct:bibliographicCitation>
            <dct:bibliographicCitation>Material-Archiv  https://materialarchiv.ch/de/ma:material_1770/</dct:bibliographicCitation>
            <dct:bibliographicCitation>Spectra by A. Cosentino, Cultural Heritage Science Open Source (CHSOS): https://chsopensource.org/lamp-black-k-47250/</dct:bibliographicCitation>
        </skos:definition>
        <skos:example>https://upload.wikimedia.org/wikipedia/commons/9/98/Carbon_black.jpg</skos:example>
        <skos:related rdf:resource="http://gams.uni-graz.at/thesaurus/carbon"/>
        <skos:broader rdf:resource="http://gams.uni-graz.at/thesaurus/carbon-based-black"/>
    </skos:Concept>
    <skos:Concept rdf:about="http://gams.uni-graz.at/thesaurus/plant-black">
        <skos:inScheme rdf:resource="http://gams.uni-graz.at/thesaurus/mss-materials"/>
        <skos:prefLabel xml:lang="de">Pflanzenschwarz</skos:prefLabel>
        <skos:altLabel xml:lang="de">Holzkohleschwarz</skos:altLabel>
        <skos:prefLabel xml:lang="en">Vegetable or plant blacks</skos:prefLabel>
        <skos:altLabel xml:lang="en">Charcoal black</skos:altLabel>
        <skos:altLabel xml:lang="en">Char black</skos:altLabel>
        <skos:definition>Plant black is made by charring (carbonising) a variety of plant materials. Often one used wood, hence the narrower term 'charcoal black' (Winter et al. 2007). A particular type is the so-called vine black produced by charring vine stalks, twigs or grape skins. Pliny the Elder referred to it as 'tryginon' saying it was used by Athenian painters (Kühl 1984; Winter et al. 2007).
        Charcoal was probably the earliest carbon-based pigment, available from the remains of fires in prehistoric times. The medieval treatises transmitted under the name of Heraclius lists a variety of soft wood material, peach stones or twigs, which when burnt should be doused with wine (Kühl 1984). Charcoal used to produce a blue colour was detected in two early English mediaeval paintings; the pigment wa also found on German playing cards from the fifteenth century (Eastaugh 2007).
        </skos:definition>
        <skos:definition rdf:parseType="Resource">
            <rdf:value>References</rdf:value>
            <dct:bibliographicCitation>Kühn, Hermann. Reclams Handbuch der künstlerischen Techniken. Vol. 1. Farbmittel, Buchmalerei, Tafel-und Leinwandmalerei. 3 vols. Stuttgart: Reclam, 1984.</dct:bibliographicCitation>
            <dct:bibliographicCitation>Winter, John, and Elisabeth West FitzHugh. ‘Pigments Based on Carbon’. In Artists’ Pigments. A Handbook of Their History and Characteristics, edited by Barbara H. Berrie, 4:1–37. Washington: National Gallery of Art, 2007.</dct:bibliographicCitation>
            <dct:bibliographicCitation>Eastaugh, Nicholas, Valentine Walsh, Tracey Chaplin, and Ruth Siddall. Pigment Compendium: A Dictionary and Optical Microscopy of Historical Pigments. Amsterdam: Elsevier, Butterworth-Heinemann, 2008.</dct:bibliographicCitation>
            <dct:bibliographicCitation>Colourlex https://colourlex.com/project/charcoal-black/</dct:bibliographicCitation>
            <dct:bibliographicCitation>Material-Archiv  https://materialarchiv.ch/de/ma:material_996/</dct:bibliographicCitation>
        </skos:definition>
        <skos:example>https://upload.wikimedia.org/wikipedia/commons/4/4a/Charcoal_sticks_051907.jpg</skos:example>
        <skos:related rdf:resource="http://gams.uni-graz.at/thesaurus/carbon"/>
        <skos:broader rdf:resource="http://gams.uni-graz.at/thesaurus/carbon-based-black"/>
    </skos:Concept>    
    <skos:Concept rdf:about="http://gams.uni-graz.at/thesaurus/bone-black">
        <skos:inScheme rdf:resource="http://gams.uni-graz.at/thesaurus/mss-materials"/>
        <skos:prefLabel xml:lang="de">Beinschwarz</skos:prefLabel>
        <skos:altLabel xml:lang="de">Knochenkohle</skos:altLabel>
        <skos:altLabel xml:lang="de">Knochenschwarz</skos:altLabel>
        <skos:altLabel xml:lang="de">Elfenbeinschwarz</skos:altLabel>
        <skos:prefLabel xml:lang="en">Bone black</skos:prefLabel>
        <skos:altLabel xml:lang="en">Ivory black</skos:altLabel>
        <skos:altLabel xml:lang="en">Carbon animal</skos:altLabel>
        <skos:altLabel xml:lang="en">Animal bone charcoal</skos:altLabel>
        <skos:definition xml:lang="en">Bone black is produced from calcinated bone dust (in some recipes mixing the substance with pumice powder, adding them to oil and boiling them). As other carbon-based pigments, bone black is stable, lightfast and compatible with all other pigments. Fairly definite identification of ivory and bone black is possible due to the presence of calcium phosphate using chemical methods or X-ray diffraction (Winter et al. 2007).
        Bone black may have been used already in ancient Egypt. It was detected in Greek gravestones from the third- to second-century B.C.E., in Roman sites in England. Descriptions of bone and ivory black are found in medieval treatises on painting and the pigments have been detected in  fifteenth-century paintings (Winter et al. 2007). Eastaugh lists further identification of bone/ivory black including Armenian Glajor Gospel book (Eastaugh et al. 2008).</skos:definition>
        <skos:definition rdf:parseType="Resource">
            <rdf:value>References</rdf:value>
            <dct:bibliographicCitation>Kühn, Hermann. Reclams Handbuch der künstlerischen Techniken. Vol. 1. Farbmittel, Buchmalerei, Tafel-und Leinwandmalerei. 3 vols. Stuttgart: Reclam, 1984, pp. , .</dct:bibliographicCitation>
            <dct:bibliographicCitation>Eastaugh, Nicholas, Valentine Walsh, Tracey Chaplin, and Ruth Siddall. Pigment Compendium: A Dictionary and Optical Microscopy of Historical Pigments. Amsterdam: Elsevier, Butterworth-Heinemann, 2008.</dct:bibliographicCitation>
            <dct:bibliographicCitation>Winter, John, and Elisabeth West FitzHugh. ‘Pigments Based on Carbon’. In Artists’ Pigments. A Handbook of Their History and Characteristics, edited by Barbara H. Berrie, 4:1–37. Washington: National Gallery of Art, 2007.</dct:bibliographicCitation> 
            <dct:bibliographicCitation>ColourLex https://colourlex.com/project/bone-black/</dct:bibliographicCitation>
            <dct:bibliographicCitation>Spectra ivory black by A. Cosentino, Cultural Heritage Science Open Source (CHSOS): https://chsopensource.org/ivory-black-k-12000/</dct:bibliographicCitation>
            <dct:bibliographicCitation>Spectra bone black by A. Cosentino, Cultural Heritage Science Open Source (CHSOS): https://chsopensource.org/bone-black-k-47100/</dct:bibliographicCitation>
        </skos:definition>        
        <skos:example>https://upload.wikimedia.org/wikipedia/commons/1/1d/%C5%BDivo%C4%8Di%C5%A1n%C3%A9_uhl%C3%AD_%28Carbocit%29.jpg</skos:example>
        <skos:related rdf:resource="http://gams.uni-graz.at/thesaurus/carbon"/>
        <skos:related rdf:resource="http://gams.uni-graz.at/thesaurus/calcium"/>
        <skos:related rdf:resource="http://gams.uni-graz.at/thesaurus/phosphorus"/>
        <skos:broader rdf:resource="http://gams.uni-graz.at/thesaurus/carbon-based-black"/>
    </skos:Concept>    
    <skos:Concept rdf:about="http://gams.uni-graz.at/thesaurus/antimony-black">
        <skos:inScheme rdf:resource="http://gams.uni-graz.at/thesaurus/mss-materials"/>
        <skos:prefLabel xml:lang="de">Antimon Schwarz</skos:prefLabel>
        <skos:prefLabel xml:lang="en">Antimony black</skos:prefLabel>
        <skos:definition xml:lang="en">Antimony black is produced by ground stibnite, a dark grey sulphide of antimony (Sb2S3). Antimony black has been identified in a group of Italian manuscripts and easel paintings dating to c. 1500 (Panayotova 2020).</skos:definition>
        <skos:definition rdf:parseType="Resource">
            <rdf:value>References</rdf:value>
            <dct:bibliographicCitation>Panayotova, Stella. ‘Painting Materials and Techniques in Western Illuminated  Manuscripts c. 600 -c. 1600’. In The Art and Science of Illuminated Manuscripts: A Handbook, edited by Stella Panayotova, 127–70. Turnhout: Brepols, 2020.</dct:bibliographicCitation>
        </skos:definition>
        <skos:related rdf:resource="http://gams.uni-graz.at/thesaurus/antimony"/>
        <skos:related rdf:resource="http://gams.uni-graz.at/thesaurus/sulfur"/>
        <skos:broader rdf:resource="http://gams.uni-graz.at/thesaurus/black-colorants"/>
    </skos:Concept>
    <skos:Concept rdf:about="http://gams.uni-graz.at/thesaurus/bismuth-black">
        <skos:inScheme rdf:resource="http://gams.uni-graz.at/thesaurus/mss-materials"/>
        <skos:prefLabel xml:lang="de">Bismut Schwarz</skos:prefLabel>
        <skos:prefLabel xml:lang="en">Bismuth black</skos:prefLabel>
        <skos:definition xml:lang="en">Bismut is a metallic element found in Europe (Erzgibirge in Saxony, Piedmont in Italy, Sierra Morena in Spain) and South America. Its grey-black colour was said to imitate silver either on its own or as amalgams together with tin.
            Black pigment using the metallic bismuth has been identified in a several fifteenth-century illuminated manuscripts illuminated by the French miniature painter Jean Bourdichon. The Master of the Antiphoner Q (active c. 1440-1470 in the Veneto and Lombardy) used bismuth black as an ink to draw thin silvery-black branches of foliage (Panayotova 2020).</skos:definition>
        <skos:definition rdf:parseType="Resource">
            <rdf:value>References</rdf:value>
            <dct:bibliographicCitation>Eastaugh, Nicholas, Valentine Walsh, Tracey Chaplin, and Ruth Siddall. Pigment Compendium: A Dictionary and Optical Microscopy of Historical Pigments. Amsterdam: Elsevier, Butterworth-Heinemann, 2008.</dct:bibliographicCitation>
            <dct:bibliographicCitation>Panayotova, Stella. ‘Painting Materials and Techniques in Western Illuminated  Manuscripts c. 600 -c. 1600’. In The Art and Science of Illuminated Manuscripts: A Handbook, edited by Stella Panayotova, 127–70. Turnhout: Brepols, 2020.</dct:bibliographicCitation>
        </skos:definition>
        <skos:related rdf:resource="http://gams.uni-graz.at/thesaurus/bismuth"/>
        <skos:broader rdf:resource="http://gams.uni-graz.at/thesaurus/black-colorants"/>
    </skos:Concept>
    <skos:Concept rdf:about="http://gams.uni-graz.at/thesaurus/pyrolusite-black">
        <skos:inScheme rdf:resource="http://gams.uni-graz.at/thesaurus/mss-materials"/>
        <skos:prefLabel xml:lang="de">Pyrolusit Schwarz</skos:prefLabel>
        <skos:prefLabel xml:lang="en">Pyrolusite black</skos:prefLabel>
        <skos:definition xml:lang="en">A black pigment produced from pyrolusite, a manganese(IV) oxide mineral with the composition MnO2. In Europe there are deposits in France (Ariege), Germany (Elgersburg), Greece (Laurion), Austria (Styria), England (Cornwall) and Italy (Tuscany). Pyrolusite was detected in prehistoric cave paintings in Spain, in Egyptian painted relief as well as on Bulgarian icons of the Middle Ages and Renaissance (Eastaugh et al. 2008). In European book illumination the pigment has been found in an initial in a late fifteenth-century Italian manuscript (Panayotova 2020).</skos:definition>
        <skos:definition rdf:parseType="Resource">
            <rdf:value>References</rdf:value>
            <dct:bibliographicCitation>Eastaugh, Nicholas, Valentine Walsh, Tracey Chaplin, and Ruth Siddall. Pigment Compendium: A Dictionary and Optical Microscopy of Historical Pigments. Amsterdam: Elsevier, Butterworth-Heinemann, 2008.</dct:bibliographicCitation>
            <dct:bibliographicCitation>Panayotova, Stella. ‘Painting Materials and Techniques in Western Illuminated  Manuscripts c. 600 -c. 1600’. In The Art and Science of Illuminated Manuscripts: A Handbook, edited by Stella Panayotova, 127–70. Turnhout: Brepols, 2020.</dct:bibliographicCitation>
        </skos:definition>
        <skos:related rdf:resource="http://gams.uni-graz.at/thesaurus/oxygen"/>
        <skos:related rdf:resource="http://gams.uni-graz.at/thesaurus/manganese"/>
        <skos:broader rdf:resource="http://gams.uni-graz.at/thesaurus/black-colorants"/>
    </skos:Concept>
<!--    ####### METAL PIGMENTS ######-->
    <skos:Concept rdf:about="http://gams.uni-graz.at/thesaurus/metal-pigments">
        <skos:inScheme rdf:resource="http://gams.uni-graz.at/thesaurus/mss-materials"/>
        <skos:prefLabel xml:lang="de">Metallische Pigmente</skos:prefLabel>
        <skos:prefLabel xml:lang="en">Metal pigments</skos:prefLabel>
        <skos:definition xml:lang="en">Medieval artists used also metals as pigments either in their elemental form (Aluminium, Antimony, Bismuth, Gold, Nickel, Silver) or as alloy. They were applied either as thinly beaten leaves or as finely ground powder. 
        For the powdered antimony (called also iron black) and bismuth see the respective sections in black colourants. 
        </skos:definition>
        <skos:example></skos:example>
        <skos:broader rdf:resource="http://gams.uni-graz.at/thesaurus/colorants"/>
    </skos:Concept>
<!--    ###### GOLD ########-->
    <skos:Concept rdf:about="http://gams.uni-graz.at/thesaurus/gold-colourant">
        <skos:inScheme rdf:resource="http://gams.uni-graz.at/thesaurus/mss-materials"/>
        <skos:prefLabel xml:lang="de">Gold</skos:prefLabel>
        <skos:prefLabel xml:lang="en">Gold</skos:prefLabel>
        <skos:definition xml:lang="en">There are three methods for applying gold on manuscript pages. The first is to use shell gold, while the other two methods involve gold leaf (thinly beaten solid sheets) applied over glue or guesso.</skos:definition>
        <skos:example>https://ids.lib.harvard.edu/ids/iiif/11732825/full/full/0/native.jpg</skos:example>
        <skos:related rdf:resource="http://gams.uni-graz.at/thesaurus/gold"/>
        <skos:broader rdf:resource="http://gams.uni-graz.at/thesaurus/metal-pigments"/>
    </skos:Concept>    
    <skos:Concept rdf:about="http://gams.uni-graz.at/thesaurus/shell-gold">
        <skos:inScheme rdf:resource="http://gams.uni-graz.at/thesaurus/mss-materials"/>
        <skos:prefLabel xml:lang="de">Muschelgold</skos:prefLabel>
        <skos:prefLabel xml:lang="en">Shell gold</skos:prefLabel>
        <skos:definition xml:lang="en">A powdered gold mixed with a binding agent (usually glair or gum arabic) to create a gold ink, which was applied with pen or brush. The method was used particularly in detailed work and in chrysography (writing in gold). Unlike leaf gold, it was added after the colour.
        The process of grinding gold was difficult since pure or nearly pure gold is rather soft. In order to produce a coarse powder one could add additional substances (honey or salt), which would be washed later on. Another method was to make an alloy by adding copper or mercury; grinding the hardened substance and at the end using an acid to dissolve the copper particles or use heat to separate mercury from gold (Thompson).</skos:definition>
        <skos:definition rdf:parseType="Resource">
            <rdf:value>References</rdf:value>
            <dct:bibliographicCitation>Thompson, Daniel Varney. The Materials and Techniques of Medieval Painting. Edited by Bernard Berenson. New York: Dover Publications, 1956.
            </dct:bibliographicCitation>
            <dct:bibliographicCitation>http://web.ceu.hu/medstud/manual/MMM/gilding.html</dct:bibliographicCitation>
        </skos:definition>
        <skos:example>https://gallica.bnf.fr/iiif/ark:/12148/btv1b6000718s/f51/full/full/0/native.jpg</skos:example>
        <skos:related rdf:resource="http://gams.uni-graz.at/thesaurus/gold"/>
        <skos:related rdf:resource="http://w3id.org/lob/concept/1594"/>
        <skos:broader rdf:resource="http://gams.uni-graz.at/thesaurus/gold-colourant"/>
    </skos:Concept>
    <skos:Concept rdf:about="http://gams.uni-graz.at/thesaurus/gold-leaf">
        <skos:inScheme rdf:resource="http://gams.uni-graz.at/thesaurus/mss-materials"/>
        <skos:prefLabel xml:lang="de">Blattgold</skos:prefLabel>
        <skos:prefLabel xml:lang="en">Gold leaf</skos:prefLabel>
        <skos:definition xml:lang="en">A thinly beaten or rolled sheet of gold applied over a ground layer of gypsum and a red clay</skos:definition>
        <skos:related rdf:resource="http://gams.uni-graz.at/thesaurus/gold"/>
        <skos:related rdf:resource="http://w3id.org/lob/concept/1370"/>
        <skos:broader rdf:resource="http://gams.uni-graz.at/thesaurus/gold-colourant"/>
        <skos:example>https://upload.wikimedia.org/wikipedia/commons/e/eb/Blattgold%2C_2010_%2801%29.jpg</skos:example>
    </skos:Concept>
<!--    ##########Silver #######-->
    <skos:Concept rdf:about="http://gams.uni-graz.at/thesaurus/silver-colourant">
        <skos:inScheme rdf:resource="http://gams.uni-graz.at/thesaurus/mss-materials"/>
        <skos:prefLabel xml:lang="de">Silber</skos:prefLabel>
        <skos:prefLabel xml:lang="en">Silver</skos:prefLabel>
        <skos:definition>Silver could be applied directly on the parchment, over a gypsum and/or calcium carbonate ground or over paint layers. In layering with other pigments, silver could be the final or the background layer. In situ non-invasive techniques are not effective in acquiring information regarding the silver paints stratigraphy; a new method was proposed using in situ examination (microscope) and analytical methods (μ-EDXRF and μ-Raman) on microsamples (Araújo et al. 2018).</skos:definition>
        <skos:example></skos:example>
        <skos:definition rdf:parseType="Resource">
            <rdf:value>References</rdf:value>
            <dct:bibliographicCitation>Araújo, Rita, Paula Nabais, Isabel Pombo Cardoso, Conceição Casanova, Ana Lemos, and Maria J. Melo. ‘Silver Paints in Medieval Manuscripts: A First Molecular Survey into Their Degradation’. Heritage Science 6, no. 1 (2018): 1–13. https://doi.org/10.1186/s40494-018-0172-7.</dct:bibliographicCitation>    
        </skos:definition>
        <skos:related rdf:resource="http://gams.uni-graz.at/thesaurus/silver"/>
        <skos:broader rdf:resource="http://gams.uni-graz.at/thesaurus/metal-pigments"/>
    </skos:Concept>
    <skos:Concept rdf:about="http://gams.uni-graz.at/thesaurus/silver-leaf">
        <skos:inScheme rdf:resource="http://gams.uni-graz.at/thesaurus/mss-materials"/>
        <skos:prefLabel xml:lang="de">Blattsilber</skos:prefLabel>
        <skos:prefLabel xml:lang="en">Silver leaf</skos:prefLabel>
        <skos:definition xml:lang="en"></skos:definition>
        <skos:example></skos:example>
        <skos:related rdf:resource="http://gams.uni-graz.at/thesaurus/silver"/>
        <skos:related rdf:resource="http://w3id.org/lob/concept/1597"/>
        <skos:broader rdf:resource="http://gams.uni-graz.at/thesaurus/silver-colourant"/>
    </skos:Concept>
    <skos:Concept rdf:about="http://gams.uni-graz.at/thesaurus/shell-silver">
        <skos:inScheme rdf:resource="http://gams.uni-graz.at/thesaurus/mss-materials"/>
        <skos:prefLabel xml:lang="de">Muschelsilber</skos:prefLabel>
        <skos:prefLabel xml:lang="en">Shell silver</skos:prefLabel>
        <skos:definition xml:lang="en"></skos:definition>
        <skos:example></skos:example>
        <skos:related rdf:resource="http://gams.uni-graz.at/thesaurus/silver"/>
        <skos:related rdf:resource="http://w3id.org/lob/concept/3017"/>       
        <skos:broader rdf:resource="http://gams.uni-graz.at/thesaurus/silver-colourant"/>
    </skos:Concept>
    <skos:Concept rdf:about="http://gams.uni-graz.at/thesaurus/tin-colourant">
        <skos:inScheme rdf:resource="http://gams.uni-graz.at/thesaurus/mss-materials"/>
        <skos:prefLabel xml:lang="de">Zinn</skos:prefLabel>
        <skos:prefLabel xml:lang="en">Tin</skos:prefLabel>
        <skos:definition xml:lang="en">Tin was used as a common, less expensive substitute for silver leaf and shell silver. Apart from its cheaper prise, tin was often preferred because it tends to oxidize and tarnish much slower than silver (Clemens and Graham 2007). One could further paint it with organic yellow (as for instance saffron) and imitate gold (Theophilius book I, ch. 30).</skos:definition>
        <skos:example></skos:example>
        <skos:definition rdf:parseType="Resource">
            <rdf:value>References</rdf:value>
            <dct:bibliographicCitation>Theophilus, Presbyter. On Divers Arts: The Foremost Medieval Treatise on Painting, Glassmaking and Metalwork. Translated by John G. Hawthorne. New York: Dover, 1979.</dct:bibliographicCitation>
            <dct:bibliographicCitation>Clemens, Raymond, and Timothy Graham. Introduction to Manuscript Studies. Ithaca, NY: Cornell University Press, 2007.</dct:bibliographicCitation>    
        </skos:definition>
        <skos:related rdf:resource="http://gams.uni-graz.at/thesaurus/tin"/>
        <skos:broader rdf:resource="http://gams.uni-graz.at/thesaurus/metal-pigments"/>
    </skos:Concept>    
    
<!--    ############ ALLOY ##########-->
    <skos:Concept rdf:about="http://gams.uni-graz.at/thesaurus/alloy-colorants">
        <skos:inScheme rdf:resource="http://gams.uni-graz.at/thesaurus/mss-materials"/>
        <skos:prefLabel xml:lang="de">Farbmittel mit Legierung</skos:prefLabel>
        <skos:prefLabel xml:lang="en">Alloy colorants</skos:prefLabel>
        <skos:broader rdf:resource="http://gams.uni-graz.at/thesaurus/metal-pigments"/>
    </skos:Concept>
    <skos:Concept rdf:about="http://gams.uni-graz.at/thesaurus/copper-alloy">
        <skos:inScheme rdf:resource="http://gams.uni-graz.at/thesaurus/mss-materials"/>
        <skos:prefLabel xml:lang="de">Kupferlegierung</skos:prefLabel>
        <skos:prefLabel xml:lang="en">Copper alloy</skos:prefLabel>
        <skos:definition xml:lang="en">Alloy containing copper (Cu) as the principle element.</skos:definition>
        <skos:example>https://upload.wikimedia.org/wikipedia/commons/c/c0/Copper_pigment.JPG</skos:example>
        <skos:related rdf:resource="http://w3id.org/lob/concept/2408"/> 
        <skos:related rdf:resource="http://vocab.getty.edu/aat/300010942"/>
        <skos:related rdf:resource="http://gams.uni-graz.at/thesaurus/copper"/>
        <skos:broader rdf:resource="http://gams.uni-graz.at/thesaurus/alloy-colorants"/>
    </skos:Concept>
    <skos:Concept rdf:about="http://gams.uni-graz.at/thesaurus/brass">
        <skos:inScheme rdf:resource="http://gams.uni-graz.at/thesaurus/mss-materials"/>
        <skos:prefLabel xml:lang="de">Messing</skos:prefLabel>
        <skos:altLabel xml:lang="de">Messingpigment</skos:altLabel>
        <skos:prefLabel xml:lang="en">Brass</skos:prefLabel>
        <skos:definition xml:lang="en">Alloy containing copper (Cu) and zinc (Zn).</skos:definition>
        <skos:example>https://upload.wikimedia.org/wikipedia/commons/2/2b/Gold_bronze_pigment.JPG</skos:example>
        <skos:related rdf:resource="http://gams.uni-graz.at/thesaurus/copper"/> 
        <skos:related rdf:resource="http://gams.uni-graz.at/thesaurus/zinc"/>
        <skos:related rdf:resource="http://w3id.org/lob/concept/2412"/>
        <skos:related rdf:resource="http://vocab.getty.edu/aat/300010946"/>
        <skos:broader rdf:resource="http://gams.uni-graz.at/thesaurus/alloy-colorants"/>
    </skos:Concept>
    <skos:Concept rdf:about="http://gams.uni-graz.at/thesaurus/bronze">
        <skos:inScheme rdf:resource="http://gams.uni-graz.at/thesaurus/mss-materials"/>
        <skos:prefLabel xml:lang="de">Bronze</skos:prefLabel>
        <skos:prefLabel xml:lang="en">Bronze</skos:prefLabel>
        <skos:definition xml:lang="en">Bronze contains copper (Cu) and other additives such as tin (Sn), silicon, aluminum, manganese, phosphorus, or various other elements. One could hence differentiaate between aluminium bronze (aluminium), speculum metal (tin), etc. </skos:definition>
        <skos:related rdf:resource="http://gams.uni-graz.at/thesaurus/copper"/> 
        <skos:related rdf:resource="http://w3id.org/lob/concept/2410"/>
        <skos:related rdf:resource="http://vocab.getty.edu/page/aat/300010957"/>
        <skos:broader rdf:resource="http://gams.uni-graz.at/thesaurus/alloy-colorants"/>
    </skos:Concept>
    <skos:Concept rdf:about="http://gams.uni-graz.at/thesaurus/alloy-au-ag">
        <skos:inScheme rdf:resource="http://gams.uni-graz.at/thesaurus/mss-materials"/>
        <skos:prefLabel xml:lang="de">Goldlegierung mit Silber</skos:prefLabel>
        <skos:prefLabel xml:lang="en">Alloy of gold and silver</skos:prefLabel> 
        <skos:definition xml:lang="en">Alloy containing gold (Au) and silver (Ag).</skos:definition>
        <skos:related rdf:resource="http://gams.uni-graz.at/thesaurus/silver"/>
        <skos:related rdf:resource="http://gams.uni-graz.at/thesaurus/gold"/>
        <skos:broader rdf:resource="http://gams.uni-graz.at/thesaurus/alloy-colorants"/>
    </skos:Concept>
    <skos:Concept rdf:about="http://gams.uni-graz.at/thesaurus/alloy-au-ag-cu">
        <skos:inScheme rdf:resource="http://gams.uni-graz.at/thesaurus/mss-materials"/>
        <skos:prefLabel xml:lang="de">Goldlegierung mit Silber und Kupfer</skos:prefLabel>
        <skos:prefLabel xml:lang="en">Alloy of gold, silver and copper</skos:prefLabel> 
        <skos:definition xml:lang="en">Alloy containing gold (Au), silver (Ag) and copper (Cu).</skos:definition>
        <skos:related rdf:resource="http://gams.uni-graz.at/thesaurus/silver"/>
        <skos:related rdf:resource="http://gams.uni-graz.at/thesaurus/gold"/>
        <skos:related rdf:resource="http://gams.uni-graz.at/thesaurus/copper"/>
        <skos:broader rdf:resource="http://gams.uni-graz.at/thesaurus/alloy-colorants"/>
    </skos:Concept>
    <skos:Concept rdf:about="http://gams.uni-graz.at/thesaurus/alloy-au-cu">
        <skos:inScheme rdf:resource="http://gams.uni-graz.at/thesaurus/mss-materials"/>
        <skos:prefLabel xml:lang="de">Goldlegierung mit Kupfer</skos:prefLabel>
        <skos:prefLabel xml:lang="en">Alloy of gold and copper</skos:prefLabel> 
        <skos:definition xml:lang="en">Alloy containing gold (Au) and copper (Cu).</skos:definition>
        <skos:related rdf:resource="http://gams.uni-graz.at/thesaurus/gold"/>
        <skos:related rdf:resource="http://gams.uni-graz.at/thesaurus/copper"/>
        <skos:broader rdf:resource="http://gams.uni-graz.at/thesaurus/alloy-colorants"/>
    </skos:Concept>
    
</rdf:RDF>