<rdf:RDF xmlns:dc="http://purl.org/dc/elements/1.1/" xmlns:fedora="info:fedora/" xmlns:rdf="http://www.w3.org/1999/02/22-rdf-syntax-ns#" xmlns:rdfs="http://www.w3.org/2000/01/rdf-schema#" xmlns:skos="http://www.w3.org/2004/02/skos/core#" xmlns:void="http://rdfs.org/ns/void#" xmlns:dct="http://purl.org/dc/terms#">
    
    <void:Dataset rdf:about="http://gams.uni-graz.at/">
        <dc:title>Vocabulary for conservation measures in mediaeval manuscripts - SKOS</dc:title>
        <dc:identifier></dc:identifier>
        <fedora:isMemberOf rdf:resource="info:fedora/context:ontology"/>
        <dc:creator>Ivana Dobcheva (rdf encoding)</dc:creator>
        <dc:creator>Patricia Engel</dc:creator>       
    </void:Dataset>
    <skos:ConceptScheme rdf:about="http://gams.uni-graz.at/thesaurus/mss-conservation">
        <dc:title>Conservation of Medieval Manuscripts</dc:title>
        <skos:hasTopConcept rdf:resource="http://gams.uni-graz.at/thesaurus/conservation"/>
        <skos:note xml:lang="en">Terms used for the description of conservation of manuscripts.</skos:note>
    </skos:ConceptScheme>
    <skos:Concept rdf:about="http://gams.uni-graz.at/thesaurus/conservation">
        <skos:inScheme rdf:resource="http://gams.uni-graz.at/thesaurus/mss-conservation"/>
        <skos:prefLabel xml:lang="de">Restauration</skos:prefLabel>
        <skos:prefLabel xml:lang="en">Conservation</skos:prefLabel>
    </skos:Concept>
    <!--    ########### Damages #############-->
    <skos:Concept rdf:about="http://gams.uni-graz.at/thesaurus/damages">
        <skos:inScheme rdf:resource="http://gams.uni-graz.at/thesaurus/mss-conservation"/>
        <skos:prefLabel xml:lang="de">Schäden</skos:prefLabel>
        <skos:prefLabel xml:lang="en">Material alteration and deterioration</skos:prefLabel>
        <skos:definition xml:lang="en">Taxonomy for damages in manuscripts and works of graphic art made of parchment and paper.
            Damage is a generic term referring to any alteration of the material possibly influencing the readability of the content. In this document we use the division into intentional (e.g. cuttings) and unintentional (e.g. mould) damages, which are further divided according to the agents of deterioration (e.g. pest infestations).</skos:definition>
        <skos:definition rdf:parseType="Resource">
            <rdf:value>References</rdf:value> 
            <dct:bibliographicCitation>Damaged Books. London: British Library (https://www.bl.uk/britishlibrary/~/media/bl/global/conservation/pdf-guides/damaged-books-preservation-guide.pdf).</dct:bibliographicCitation>
            <dct:bibliographicCitation>Archives Damage Atlas 
                https://www.metamorfoze.nl/sites/default/files/documents/schadeatlas-2010%20engels.pdf</dct:bibliographicCitation>
            <dct:bibliographicCitation>Roberts, Matt T. and Don Etherington. Bookbinding and the Conservation of Books. A Dictionary of Descriptive Terminology. Washington: Library of Congress, 1982. (online: https://cool.culturalheritage.org/don/don.html).</dct:bibliographicCitation>
            <dct:bibliographicCitation>Book and Paper Group Wiki. 2022. Book and Paper Group Wiki. American Institute for Conservation (AIC). Accessed April 17, 2023. https://www.conservation-wiki.com/wiki/Book_and_Paper_Group_Wiki</dct:bibliographicCitation>
        </skos:definition>
        <skos:broader rdf:resource="http://gams.uni-graz.at/thesaurus/conservation"/>
    </skos:Concept>
    
    <!--    ########### Intentional Damages // Deletions #############-->
    <skos:Concept rdf:about="http://gams.uni-graz.at/thesaurus/intentionalDamage">
        <skos:inScheme rdf:resource="http://gams.uni-graz.at/thesaurus/mss-conservation"/>
        <skos:prefLabel xml:lang="en">Intentional damage</skos:prefLabel>
        <skos:prefLabel xml:lang="de">Absichtliche Schäden</skos:prefLabel>
        <skos:definition xml:lang="en">An intentional damage on the whole or part of the manuscript.</skos:definition>
        <skos:broader rdf:resource="http://gams.uni-graz.at/thesaurus/damages"/>
    </skos:Concept>
    <skos:Concept rdf:about="http://gams.uni-graz.at/thesaurus/fragmentation">
        <skos:inScheme rdf:resource="http://gams.uni-graz.at/thesaurus/mss-conservation"/>
        <skos:prefLabel xml:lang="de">Fragment</skos:prefLabel>
        <skos:prefLabel xml:lang="en">Fragment</skos:prefLabel>
        <skos:definition xml:lang="en">Intentional braking the structure of the original book.</skos:definition>
        <skos:broader rdf:resource="http://gams.uni-graz.at/thesaurus/intentionalDamage"/>
    </skos:Concept>
    <skos:Concept rdf:about="http://gams.uni-graz.at/thesaurus/brokenBook">
        <skos:inScheme rdf:resource="http://gams.uni-graz.at/thesaurus/mss-conservation"/>
        <skos:prefLabel xml:lang="de">Disiecta membra</skos:prefLabel>
        <skos:prefLabel xml:lang="en">Broken book</skos:prefLabel>
        <skos:definition xml:lang="en">Intentional braking the structure of the original book in detached and dispersed leaves.</skos:definition>
        <skos:broader rdf:resource="http://gams.uni-graz.at/thesaurus/fragmentation"/>
    </skos:Concept>
    <skos:Concept rdf:about="http://gams.uni-graz.at/thesaurus/cutting">
        <skos:inScheme rdf:resource="http://gams.uni-graz.at/thesaurus/mss-conservation"/>
        <skos:prefLabel xml:lang="de">Schnitt</skos:prefLabel>
        <skos:prefLabel xml:lang="en">Cutting</skos:prefLabel>
        <skos:definition xml:lang="en">Parts usually including illumination cut out from the original leaf.</skos:definition>
        <skos:broader rdf:resource="http://gams.uni-graz.at/thesaurus/fragmentation"/>
    </skos:Concept>
    <skos:Concept rdf:about="http://gams.uni-graz.at/thesaurus/binding-waste">
        <skos:inScheme rdf:resource="http://gams.uni-graz.at/thesaurus/mss-conservation"/>
        <skos:prefLabel xml:lang="de">Makulatur</skos:prefLabel>
        <skos:prefLabel xml:lang="en">Binding waste</skos:prefLabel>
<!--        #############!-->
        <skos:definition xml:lang="en"></skos:definition>
        <skos:broader rdf:resource="http://gams.uni-graz.at/thesaurus/fragmentation"/>
    </skos:Concept>
<!--    ###################### DELETIONS ######################-->
    <skos:Concept rdf:about="http://gams.uni-graz.at/thesaurus/deletions">
        <skos:inScheme rdf:resource="http://gams.uni-graz.at/thesaurus/mss-conservation"/>
        <skos:prefLabel xml:lang="de">Tilgungen</skos:prefLabel>
        <skos:prefLabel xml:lang="en">Deletions</skos:prefLabel>
        <skos:definition xml:lang="en">List of methods for deleting text in mediaeval manuscripts. Divided in groups based on the tools and techniques applied.</skos:definition>
        <skos:broader rdf:resource="http://gams.uni-graz.at/thesaurus/intentionalDamage"/>
    </skos:Concept>
    <skos:Concept rdf:about="http://gams.uni-graz.at/thesaurus/dryDeletions">
        <skos:inScheme rdf:resource="http://gams.uni-graz.at/thesaurus/mss-conservation"/>
        <skos:prefLabel xml:lang="en">Dry methods</skos:prefLabel>  
        <skos:prefLabel xml:lang="de">Tilgungen mit trockenen Mitteln</skos:prefLabel>
        <skos:defintion xml:lang="en">The more common method of dry deleting is the abrasion of the inks plus the uppermost layer of the parchment. This can be done with a knife, a piece of pumice, sepiolite, deletion bread or a sand stone. A second technique is by dusting off writing material with feathers (Engel 2021).</skos:defintion>
        <skos:definition rdf:parseType="Resource">
            <rdf:value>References</rdf:value>
            <dct:bibliographicCitation>Engel, P. "Deletions in Manuscripts and Conservators´ Decision-Making Depicted in SKOS". Conservation Update 2(2021): 25-49. DOI: 10.48341/rva1-5g91</dct:bibliographicCitation>
        </skos:definition>
        <skos:broader rdf:resource="http://gams.uni-graz.at/thesaurus/deletions"/>
    </skos:Concept>
    <skos:Concept rdf:about="http://gams.uni-graz.at/thesaurus/duringWritingDeletions">
        <skos:inScheme rdf:resource="http://gams.uni-graz.at/thesaurus/mss-conservation"/>
        <skos:prefLabel xml:lang="en">Deletions during writing</skos:prefLabel>    
        <skos:prefLabel xml:lang="de">Tilgungen während des Schreibens</skos:prefLabel>
        <skos:definition xml:lang="en">By mistake during the writing of the text scribes would first delete the incorrect letters or words (in most cases using a penknife), and then overwrite the area immediately. </skos:definition>
        <skos:definition rdf:parseType="Resource">
            <rdf:value>References</rdf:value>
            <dct:bibliographicCitation>Engel, P. "Deletions in Manuscripts and Conservators´ Decision-Making Depicted in SKOS". Conservation Update 2(2021): 25-49. DOI: 10.48341/rva1-5g91</dct:bibliographicCitation>
        </skos:definition>
        <skos:broader rdf:resource="http://gams.uni-graz.at/thesaurus/dryDeletions"/>
    </skos:Concept>
    <skos:Concept rdf:about="http://gams.uni-graz.at/thesaurus/penknife">
        <skos:inScheme rdf:resource="http://gams.uni-graz.at/thesaurus/mss-conservation"/>
        <skos:prefLabel xml:lang="en">Penknife</skos:prefLabel>   
        <skos:altLabel xml:lang="en">Knife</skos:altLabel>
        <skos:prefLabel xml:lang="de">Radiermesser</skos:prefLabel>
        <skos:deinition xml:lang="en">Penknives can be used to delete text in all inks on papyrus, parchment and paper. Traces left: thinner and rougher areas. Detection: lighter area (detected using transmitted light), darker area (detected using raking light); locally, smeared inks; the ink written over the area is in most cases blurring (this may also be the case with other dry deleting methods, however if an entire page is cleaned it is often re-polished after this, which is actually not the case when a penknife was used).</skos:deinition>
        <skos:definition rdf:parseType="Resource">
            <rdf:value>References</rdf:value>
            <dct:bibliographicCitation>Engel, P. "Deletions in Manuscripts and Conservators´ Decision-Making Depicted in SKOS". Conservation Update 2(2021): 25-49. DOI: 10.48341/rva1-5g91</dct:bibliographicCitation>
        </skos:definition>
        <skos:relatedMatch rdf:resource="http://codicologia.irht.cnrs.fr/term-1554"/>
        <skos:broader rdf:resource="http://gams.uni-graz.at/thesaurus/duringWritingDeletions"/>
    </skos:Concept>    
   
    <skos:Concept rdf:about="http://gams.uni-graz.at/thesaurus/dryDeletionsAfter">
        <skos:inScheme rdf:resource="http://gams.uni-graz.at/thesaurus/mss-conservation"/>
        <skos:prefLabel xml:lang="en">Dry methods after writing</skos:prefLabel>   
        <skos:prefLabel xml:lang="de">Tilgungen nach dem Schreiben</skos:prefLabel>
        <skos:broader rdf:resource="http://gams.uni-graz.at/thesaurus/dryDeletions"/>
    </skos:Concept>
    <skos:Concept rdf:about="http://gams.uni-graz.at/thesaurus/deletionPumice">
        <skos:inScheme rdf:resource="http://gams.uni-graz.at/thesaurus/mss-conservation"/>
        <skos:prefLabel xml:lang="en">Pumice</skos:prefLabel>   
        <skos:altLabel xml:lang="en">Pumice stone</skos:altLabel>
        <skos:prefLabel xml:lang="de">Bimsstein</skos:prefLabel>
        <skos:definition xml:lang="en">Pumice is a volcanic rockglass in which the encapsulated gas was released immediately, which accounts for its porous structure. It was used to erase text written in all inks on papyrus and parchment. Traces left: parallel scratches visible under magnification and in raking light as darker area.</skos:definition>
        <skos:definition rdf:parseType="Resource">
            <rdf:value>References</rdf:value>
            <dct:bibliographicCitation>Engel, P. "Deletions in Manuscripts and Conservators´ Decision-Making Depicted in SKOS". Conservation Update 2(2021): 25-49. DOI: 10.48341/rva1-5g91</dct:bibliographicCitation>
        </skos:definition>
        <skos:relatedMatch rdf:resource="http://codicologia.irht.cnrs.fr/term-1558"/>
        <skos:broader rdf:resource="http://gams.uni-graz.at/thesaurus/dryDeletionsAfter"/>
    </skos:Concept>
    <skos:Concept rdf:about="http://gams.uni-graz.at/thesaurus/deletionCuttlebone">
        <skos:inScheme rdf:resource="http://gams.uni-graz.at/thesaurus/mss-conservation"/>
        <skos:prefLabel xml:lang="en">Cuttlebone</skos:prefLabel>
        <skos:altLabel xml:lang="en">Cuttlefish bone</skos:altLabel>
        <skos:prefLabel xml:lang="de">Schulp</skos:prefLabel>
        <skos:altLabel xml:lang="de">Os sepium</skos:altLabel>
        <skos:definition xml:lang="en">Cuttlebone is the inner skeleton of a sepia fish (sepia officinalis), a light white porous piece consisting mainly of aragonite (calcium carbonate).</skos:definition>
        <skos:definition rdf:parseType="Resource">
            <rdf:value>References</rdf:value>
            <dct:bibliographicCitation>Engel, P. "Deletions in Manuscripts and Conservators´ Decision-Making Depicted in SKOS". Conservation Update 2(2021): 25-49. DOI: 10.48341/rva1-5g91</dct:bibliographicCitation>
        </skos:definition>
        <skos:broader rdf:resource="http://gams.uni-graz.at/thesaurus/dryDeletionsAfter"/>        
    </skos:Concept>
    <skos:Concept rdf:about="http://gams.uni-graz.at/thesaurus/deletionSepiolite">
        <skos:inScheme rdf:resource="http://gams.uni-graz.at/thesaurus/mss-conservation"/>
        <skos:prefLabel xml:lang="en">Sepiolite</skos:prefLabel>
        <skos:altLabel xml:lang="en">Meerschaum</skos:altLabel>
        <skos:prefLabel xml:lang="de">Sepiolith</skos:prefLabel>
        <skos:altLabel xml:lang="de">Meerschaum</skos:altLabel>
        <skos:definition xml:lang="en">Sepiolite is a soft and porous white clay mineral (a complex magnesium silicate).</skos:definition>        
        <skos:broader rdf:resource="http://gams.uni-graz.at/thesaurus/dryDeletionsAfter"/>        
    </skos:Concept>
    <skos:Concept rdf:about="http://gams.uni-graz.at/thesaurus/deletionBread">
        <skos:inScheme rdf:resource="http://gams.uni-graz.at/thesaurus/mss-conservation"/>
        <skos:prefLabel xml:lang="en">Bread</skos:prefLabel>
        <skos:prefLabel xml:lang="de">Schleifbrot</skos:prefLabel>
        <skos:broader rdf:resource="http://gams.uni-graz.at/thesaurus/dryDeletionsAfter"/>
        <skos:definition xml:lang="en">Bread (Schleifbrot) is a mixture of flour, chalk, egg white and glass (sometimes yeast was added too and the substance was baked). This chalky “bread” was used in geographic areas far from sea coasts, where pumice and sepiolite were not readily available. It was used to erase text written in all inks on papyrus and parchment.</skos:definition>
        <skos:definition rdf:parseType="Resource">
            <rdf:value>References</rdf:value>
            <dct:bibliographicCitation>Engel, P. "Deletions in Manuscripts and Conservators´ Decision-Making Depicted in SKOS". Conservation Update 2(2021): 25-49. DOI: 10.48341/rva1-5g91</dct:bibliographicCitation>
        </skos:definition>
    </skos:Concept>
    <skos:Concept rdf:about="http://gams.uni-graz.at/thesaurus/deletionSandstone">
        <skos:inScheme rdf:resource="http://gams.uni-graz.at/thesaurus/mss-conservation"/>
        <skos:prefLabel xml:lang="en">Sandstone</skos:prefLabel>
        <skos:prefLabel xml:lang="de">Sandstein</skos:prefLabel>
        <skos:definition xml:lang="en">Sandstone is a natural fine-structured stone which was also readily available in areas far from sea coasts. It was made into sticks and used for deletion of text. It was used to erase text written in all inks on papyrus and parchment. Its use is detectable by transmitted light (lighter area) and raking light (darker/rougher area).</skos:definition>
        <skos:definition rdf:parseType="Resource">
            <rdf:value>References</rdf:value>
            <dct:bibliographicCitation>Engel, P. "Deletions in Manuscripts and Conservators´ Decision-Making Depicted in SKOS". Conservation Update 2(2021): 25-49. DOI: 10.48341/rva1-5g91</dct:bibliographicCitation>
        </skos:definition>
        <skos:broader rdf:resource="http://gams.uni-graz.at/thesaurus/dryDeletionsAfter"/>
    </skos:Concept>
    <skos:Concept rdf:about="http://gams.uni-graz.at/thesaurus/deletionErasurePowder">
        <skos:inScheme rdf:resource="http://gams.uni-graz.at/thesaurus/mss-conservation"/>
        <skos:prefLabel xml:lang="en">Erasure powder</skos:prefLabel>
        <skos:prefLabel xml:lang="de">Tilgungspulver</skos:prefLabel>
        <skos:definition xml:lang="en">Erasure powder is a comparatively late recipe for deleting texts; the powder made of dried powdered hare skin was used in combination with pumice as a tool for rubbing the powder into the letter required to be deleted – the leather fibres penetrated both the pumice and the surface of the writing material (Engel 2021).</skos:definition>
        <skos:definition rdf:parseType="Resource">
            <rdf:value>References</rdf:value>
            <dct:bibliographicCitation>Engel, P. "Deletions in Manuscripts and Conservators´ Decision-Making Depicted in SKOS". Conservation Update 2(2021): 25-49. DOI: 10.48341/rva1-5g91</dct:bibliographicCitation>
        </skos:definition>
        <skos:broader rdf:resource="http://gams.uni-graz.at/thesaurus/dryDeletionsAfter"/>        
    </skos:Concept>
    <skos:Concept rdf:about="http://gams.uni-graz.at/thesaurus/deletionFeathers">
        <skos:inScheme rdf:resource="http://gams.uni-graz.at/thesaurus/mss-conservation"/>
        <skos:prefLabel xml:lang="en">Feathers</skos:prefLabel>
        <skos:prefLabel xml:lang="de">Feder</skos:prefLabel>
        <skos:definition xml:lang="en">Feathers might be used to dust off coal and other pigments applied without binding agents, and so to avoid harming the parchment surface (Engel 2021).</skos:definition>
        <skos:broader rdf:resource="http://gams.uni-graz.at/thesaurus/dryDeletionsAfter"/>   
        <skos:definition rdf:parseType="Resource">
            <rdf:value>References</rdf:value>
            <dct:bibliographicCitation>Engel, P. "Deletions in Manuscripts and Conservators´ Decision-Making Depicted in SKOS". Conservation Update 2(2021): 25-49. DOI: 10.48341/rva1-5g91</dct:bibliographicCitation>
        </skos:definition>
    </skos:Concept>
    
    <skos:Concept rdf:about="http://gams.uni-graz.at/thesaurus/coverDeletion">
        <skos:inScheme rdf:resource="http://gams.uni-graz.at/thesaurus/mss-conservation"/>
        <skos:prefLabel xml:lang="en">Covering methods</skos:prefLabel> 
        <skos:prefLabel xml:lang="de">Überdecken</skos:prefLabel>
        <skos:definition xml:lang="en">The third main category of deleting methods is to cover the a part of the written surface either with paint or with additional material. The written instructions are not known, but there is ample evidence of this practice in manuscripts.</skos:definition>
        <skos:definition rdf:parseType="Resource">
            <rdf:value>References</rdf:value>
            <dct:bibliographicCitation>Engel, P. "Deletions in Manuscripts and Conservators´ Decision-Making Depicted in SKOS". Conservation Update 2(2021): 25-49. DOI: 10.48341/rva1-5g91</dct:bibliographicCitation>
        </skos:definition>
        <skos:broader rdf:resource="http://gams.uni-graz.at/thesaurus/deletions"/>
    </skos:Concept>
    <skos:Concept rdf:about="http://gams.uni-graz.at/thesaurus/overpaint">
        <skos:inScheme rdf:resource="http://gams.uni-graz.at/thesaurus/mss-conservation"/>
        <skos:prefLabel xml:lang="en">Overpainting</skos:prefLabel> 
        <skos:prefLabel xml:lang="de">Übermalen</skos:prefLabel>
        <skos:broader rdf:resource="http://gams.uni-graz.at/thesaurus/coverDeletion"/>
    </skos:Concept>
    <skos:Concept rdf:about="http://gams.uni-graz.at/thesaurus/overpaste">
        <skos:inScheme rdf:resource="http://gams.uni-graz.at/thesaurus/mss-conservation"/>
        <skos:prefLabel xml:lang="en">Pasting over</skos:prefLabel> 
        <skos:prefLabel xml:lang="de">Überkleben</skos:prefLabel>
        <skos:broader rdf:resource="http://gams.uni-graz.at/thesaurus/coverDeletion"/>
    </skos:Concept>
    <skos:Concept rdf:about="http://gams.uni-graz.at/thesaurus/oversew">
        <skos:inScheme rdf:resource="http://gams.uni-graz.at/thesaurus/mss-conservation"/>
        <skos:prefLabel xml:lang="en">Sewing over</skos:prefLabel> 
        <skos:prefLabel xml:lang="de">Übernähen</skos:prefLabel>
        <skos:broader rdf:resource="http://gams.uni-graz.at/thesaurus/coverDeletion"/>
    </skos:Concept>
    
    <skos:Concept rdf:about="http://gams.uni-graz.at/thesaurus/liftingDeletions">
        <skos:inScheme rdf:resource="http://gams.uni-graz.at/thesaurus/mss-conservation"/>
        <skos:prefLabel xml:lang="en">Lifting off</skos:prefLabel> 
        <skos:prefLabel xml:lang="de">Abheben</skos:prefLabel>
        <skos:definition xml:lang="en">Lifting off is a deleting technique relevant for charcoal. Cennini recommends fresh bread for this purpose. We might assume that this was a widely used method. However, in manuscripts charcoal was actually only used for first sketches for illuminations (Engel 2021).</skos:definition>
        <skos:definition rdf:parseType="Resource">
            <rdf:value>References</rdf:value>
            <dct:bibliographicCitation>Engel, P. "Deletions in Manuscripts and Conservators´ Decision-Making Depicted in SKOS". Conservation Update 2(2021): 25-49. DOI: 10.48341/rva1-5g91</dct:bibliographicCitation>
        </skos:definition>
        <skos:broader rdf:resource="http://gams.uni-graz.at/thesaurus/deletions"/>
    </skos:Concept>
    
    <skos:Concept rdf:about="http://gams.uni-graz.at/thesaurus/cuttingDeletions">
        <skos:inScheme rdf:resource="http://gams.uni-graz.at/thesaurus/mss-conservation"/>
        <skos:prefLabel xml:lang="en">Cutting out</skos:prefLabel>   
        <skos:prefLabel xml:lang="de">Herausschneiden</skos:prefLabel>
        <skos:broader rdf:resource="http://gams.uni-graz.at/thesaurus/deletions"/>
    </skos:Concept>
    
    <skos:Concept rdf:about="http://gams.uni-graz.at/thesaurus/liquidDeletions">
        <skos:inScheme rdf:resource="http://gams.uni-graz.at/thesaurus/mss-conservation"/>
        <skos:prefLabel xml:lang="en">Liquid methods</skos:prefLabel>
        <skos:prefLabel xml:lang="de">Tilgungen mit Flüssigkeiten</skos:prefLabel>
        <skos:note xml:lang="en">Liquids work in two ways: they either wash off the inks or modify them in such a way that inks become invisible/less visible (for example by pH changes). A third possible way of using liquid deletion agents is to swell the surface of the parchment and then scratch it off (Engel 2021).</skos:note>
        <skos:definition rdf:parseType="Resource">
            <rdf:value>References</rdf:value>
            <dct:bibliographicCitation>Engel, P. "Deletions in Manuscripts and Conservators´ Decision-Making Depicted in SKOS". Conservation Update 2(2021): 25-49. DOI: 10.48341/rva1-5g91</dct:bibliographicCitation>
        </skos:definition>
        <skos:broader rdf:resource="http://gams.uni-graz.at/thesaurus/deletions"/>
    </skos:Concept>
    <skos:Concept rdf:about="http://gams.uni-graz.at/thesaurus/deletionWater">
        <skos:inScheme rdf:resource="http://gams.uni-graz.at/thesaurus/mss-conservation"/>
        <skos:prefLabel xml:lang="en">Water</skos:prefLabel>
        <skos:prefLabel xml:lang="de">Wasser</skos:prefLabel>
        <skos:definition xml:lang="en">Depending on the amount of water used and the way of application we find roughened areas.</skos:definition>
        <skos:definition rdf:parseType="Resource">
            <rdf:value>References</rdf:value>
            <dct:bibliographicCitation>Engel, P. "Deletions in Manuscripts and Conservators´ Decision-Making Depicted in SKOS". Conservation Update 2(2021): 25-49. DOI: 10.48341/rva1-5g91</dct:bibliographicCitation>
        </skos:definition>
        <skos:broader rdf:resource="http://gams.uni-graz.at/thesaurus/liquidDeletions"/>        
    </skos:Concept>
    <skos:Concept rdf:about="http://gams.uni-graz.at/thesaurus/deletionWine">
        <skos:inScheme rdf:resource="http://gams.uni-graz.at/thesaurus/mss-conservation"/>
        <skos:prefLabel xml:lang="en">Wine</skos:prefLabel>
        <skos:prefLabel xml:lang="de">Wein</skos:prefLabel>
        <skos:definition rdf:parseType="Resource">
            <rdf:value>References</rdf:value>
            <dct:bibliographicCitation>Engel, P. "Deletions in Manuscripts and Conservators´ Decision-Making Depicted in SKOS". Conservation Update 2(2021): 25-49. DOI: 10.48341/rva1-5g91</dct:bibliographicCitation>
        </skos:definition>
        <skos:broader rdf:resource="http://gams.uni-graz.at/thesaurus/liquidDeletions"/>        
    </skos:Concept>
    <skos:Concept rdf:about="http://gams.uni-graz.at/thesaurus/deletionMilk">
        <skos:inScheme rdf:resource="http://gams.uni-graz.at/thesaurus/mss-conservation"/>
        <skos:prefLabel xml:lang="en">Milk</skos:prefLabel>
        <skos:prefLabel xml:lang="de">Milch</skos:prefLabel>
        <skos:definition xml:lang="en">Methods of detection: Grayish line flour in the structure; smell of milk. Soot ink completely deleted on smooth and rough parchment. Iron gall ink vanishes on a smooth surface; on a rough surface remains detectable under the microscope; in transmitted light traces detectable.</skos:definition>
        <skos:definition rdf:parseType="Resource">
            <rdf:value>References</rdf:value>
            <dct:bibliographicCitation>Engel, P. "Deletions in Manuscripts and Conservators´ Decision-Making Depicted in SKOS". Conservation Update 2(2021): 25-49. DOI: 10.48341/rva1-5g91</dct:bibliographicCitation>
        </skos:definition>
        <skos:broader rdf:resource="http://gams.uni-graz.at/thesaurus/liquidDeletions"/> 
    </skos:Concept>
    
    <skos:Concept rdf:about="http://gams.uni-graz.at/thesaurus/deletionMixture">
        <skos:inScheme rdf:resource="http://gams.uni-graz.at/thesaurus/mss-conservation"/>
        <skos:prefLabel xml:lang="en">Mixture</skos:prefLabel>
        <skos:prefLabel xml:lang="de">Mischung</skos:prefLabel>
        <skos:definition xml:lang="en">All recipes for mixtures of substances to result in a liquid or, in most cases a pasty mass for deleting text originate from the 15th century or later. They rely on physico-chemical degradation of the ink, washing off, swelling of parchment and, in some cases, additional scratching off the surface (Engel 2021).</skos:definition>
        <skos:definition rdf:parseType="Resource">
            <rdf:value>References</rdf:value>
            <dct:bibliographicCitation>Engel, P. "Deletions in Manuscripts and Conservators´ Decision-Making Depicted in SKOS". Conservation Update 2(2021): 25-49. DOI: 10.48341/rva1-5g91</dct:bibliographicCitation>
        </skos:definition>
        <skos:broader rdf:resource="http://gams.uni-graz.at/thesaurus/liquidDeletions"/>        
    </skos:Concept>
    <skos:Concept rdf:about="http://gams.uni-graz.at/thesaurus/deletionMixture1">
        <skos:inScheme rdf:resource="http://gams.uni-graz.at/thesaurus/mss-conservation"/>
        <skos:prefLabel xml:lang="en">Mixture: lime, vitriol, alum</skos:prefLabel>
        <skos:prefLabel xml:lang="de">Mischung: Kalk, Vitriol, Alaun</skos:prefLabel>
        <skos:broader rdf:resource="http://gams.uni-graz.at/thesaurus/deletionMixture"/> 
        <skos:definition xml:lang="en">According to a medieval recipe the mixture was spread over the parchment and later rubbed. The ink becomes much lighter, actually yellowish as a first step. Parchment is also yellowish after the application of this recipe. On a smooth parchment the ink may be deleted, on rough parchment a stain is left. In the area where the mixture was applied one might detect various sorts of vitriol (other than from the ink) and alum (Engel 2021).</skos:definition>
        <skos:definition rdf:parseType="Resource">
            <rdf:value>References</rdf:value>
            <dct:bibliographicCitation>Engel, P. "Deletions in Manuscripts and Conservators´ Decision-Making Depicted in SKOS". Conservation Update 2(2021): 25-49. DOI: 10.48341/rva1-5g91</dct:bibliographicCitation>
        </skos:definition>
    </skos:Concept>
    <skos:Concept rdf:about="http://gams.uni-graz.at/thesaurus/deletionMixture2">
        <skos:inScheme rdf:resource="http://gams.uni-graz.at/thesaurus/mss-conservation"/>
        <skos:prefLabel xml:lang="en">Mixture: vitriol and potassium or sodium nitrate</skos:prefLabel>
        <skos:prefLabel xml:lang="de">Mischung: Vitriol, Kalium oder Natriumnitrat</skos:prefLabel>
        <skos:definition xml:lang="en">The method comes from a 15th-century recipe. The deletion is detectable by the yellow stain on paper caused by the Nitration (Engel 2021).</skos:definition>
        <skos:definition rdf:parseType="Resource">
            <rdf:value>References</rdf:value>
            <dct:bibliographicCitation>Engel, P. "Deletions in Manuscripts and Conservators´ Decision-Making Depicted in SKOS". Conservation Update 2(2021): 25-49. DOI: 10.48341/rva1-5g91</dct:bibliographicCitation>
        </skos:definition>
        <skos:broader rdf:resource="http://gams.uni-graz.at/thesaurus/deletionMixture"/> 
    </skos:Concept>
    <skos:Concept rdf:about="http://gams.uni-graz.at/thesaurus/deletionMixture3">
        <skos:inScheme rdf:resource="http://gams.uni-graz.at/thesaurus/mss-conservation"/>
        <skos:prefLabel xml:lang="en">Mixture: potassium or sodium nitrate and iron sulfate and water</skos:prefLabel>
        <skos:prefLabel xml:lang="de">Mischung: Kalium oder Natriumnitrat, Eisensulfat und Wasser</skos:prefLabel>
        <skos:definition xml:lang="en">The method comes from a 15th-century recipe. The deletion is detectable by the yellow stain on paper caused by the Nitration (Engel 2021).</skos:definition>
        <skos:definition rdf:parseType="Resource">
            <rdf:value>References</rdf:value>
            <dct:bibliographicCitation>Engel, P. "Deletions in Manuscripts and Conservators´ Decision-Making Depicted in SKOS". Conservation Update 2(2021): 25-49. DOI: 10.48341/rva1-5g91</dct:bibliographicCitation>
        </skos:definition>
        <skos:broader rdf:resource="http://gams.uni-graz.at/thesaurus/deletionMixture"/> 
    </skos:Concept>    
    <skos:Concept rdf:about="http://gams.uni-graz.at/thesaurus/deletionMixture4">
        <skos:inScheme rdf:resource="http://gams.uni-graz.at/thesaurus/mss-conservation"/>
        <skos:prefLabel xml:lang="en">Mixture: alum, orange juice</skos:prefLabel>
        <skos:prefLabel xml:lang="de">Mischung: Alaun, Orangensaft</skos:prefLabel>
        <skos:definition xml:lang="en">The method is described in a 15th-century recipe. Iron gall ink becomes much lighter on paper, other writing material, such as stylus, abrasives and soot ink can be deleted completely. Surface texture of paper or parchment stays unchanged. The fresher the inks are the easier they can be deleted using this recipe.</skos:definition>
        <skos:definition rdf:parseType="Resource">
            <rdf:value>References</rdf:value>
            <dct:bibliographicCitation>Engel, P. "Deletions in Manuscripts and Conservators´ Decision-Making Depicted in SKOS". Conservation Update 2(2021): 25-49. DOI: 10.48341/rva1-5g91</dct:bibliographicCitation>
        </skos:definition>
        <skos:broader rdf:resource="http://gams.uni-graz.at/thesaurus/deletionMixture"/> 
    </skos:Concept>
    <skos:Concept rdf:about="http://gams.uni-graz.at/thesaurus/deletionMixture5">
        <skos:inScheme rdf:resource="http://gams.uni-graz.at/thesaurus/mss-conservation"/>
        <skos:prefLabel xml:lang="en">Mixture: Orange juice, chalk and water</skos:prefLabel>
        <skos:prefLabel xml:lang="de">Mischung: Orangensaft, Kreide und Wasser</skos:prefLabel>
        <skos:definition xml:lang="en">The method is described in a 15th-century recipe. The surface should be rubbed with a sponge soaked in orange juice. Then one applies chalk either as powder or in water solution on the relevant area or as a powder. Traces left by the method include chalk, locally different then in unchanged areas. The ink becomes light brown after application of orange juice.</skos:definition>
        <skos:definition rdf:parseType="Resource">
            <rdf:value>References</rdf:value>
            <dct:bibliographicCitation>Engel, P. "Deletions in Manuscripts and Conservators´ Decision-Making Depicted in SKOS". Conservation Update 2(2021): 25-49. DOI: 10.48341/rva1-5g91</dct:bibliographicCitation>
        </skos:definition>
        <skos:broader rdf:resource="http://gams.uni-graz.at/thesaurus/deletionMixture"/> 
    </skos:Concept>
    <skos:Concept rdf:about="http://gams.uni-graz.at/thesaurus/deletionMixture6">
        <skos:inScheme rdf:resource="http://gams.uni-graz.at/thesaurus/mss-conservation"/>
        <skos:prefLabel xml:lang="en">Mixture: rosin and horse dung</skos:prefLabel>
        <skos:prefLabel xml:lang="de">Mischung: Harz, Pferdeäpfel</skos:prefLabel>
        <skos:definition rdf:parseType="Resource">
            <rdf:value>References</rdf:value>
            <dct:bibliographicCitation>Engel, P. "Deletions in Manuscripts and Conservators´ Decision-Making Depicted in SKOS". Conservation Update 2(2021): 25-49. DOI: 10.48341/rva1-5g91</dct:bibliographicCitation>
        </skos:definition>
        <skos:broader rdf:resource="http://gams.uni-graz.at/thesaurus/deletionMixture"/>         
    </skos:Concept>
    <skos:Concept rdf:about="http://gams.uni-graz.at/thesaurus/deletionMixture7">
        <skos:inScheme rdf:resource="http://gams.uni-graz.at/thesaurus/mss-conservation"/>
        <skos:prefLabel xml:lang="en">Mixture: alum and salmiac</skos:prefLabel>
        <skos:prefLabel xml:lang="de">Mischung: Alaun, Salmiak</skos:prefLabel>
        <skos:definition rdf:parseType="Resource">
            <rdf:value>References</rdf:value>
            <dct:bibliographicCitation>Engel, P. "Deletions in Manuscripts and Conservators´ Decision-Making Depicted in SKOS". Conservation Update 2(2021): 25-49. DOI: 10.48341/rva1-5g91</dct:bibliographicCitation>
        </skos:definition>
        <skos:broader rdf:resource="http://gams.uni-graz.at/thesaurus/deletionMixture"/>         
    </skos:Concept>
    <skos:Concept rdf:about="http://gams.uni-graz.at/thesaurus/deletionMixture8">
        <skos:inScheme rdf:resource="http://gams.uni-graz.at/thesaurus/mss-conservation"/>
        <skos:prefLabel xml:lang="en">Mixture: powdered hare meat and lime</skos:prefLabel>
        <skos:prefLabel xml:lang="de">Mischung: Hasenfleisch (pulverisiert), Kalk</skos:prefLabel>
        <skos:definition rdf:parseType="Resource">
            <rdf:value>References</rdf:value>
            <dct:bibliographicCitation>Engel, P. "Deletions in Manuscripts and Conservators´ Decision-Making Depicted in SKOS". Conservation Update 2(2021): 25-49. DOI: 10.48341/rva1-5g91</dct:bibliographicCitation>
        </skos:definition>
        <skos:broader rdf:resource="http://gams.uni-graz.at/thesaurus/deletionMixture"/>         
    </skos:Concept>
    <skos:Concept rdf:about="http://gams.uni-graz.at/thesaurus/deletionMixture9">
        <skos:inScheme rdf:resource="http://gams.uni-graz.at/thesaurus/mss-conservation"/>
        <skos:prefLabel xml:lang="en">Mixture: alum, ash, egg shells</skos:prefLabel>
        <skos:prefLabel xml:lang="de">Mischung: Alaun, Asche, Eierschale</skos:prefLabel>
        <skos:definition rdf:parseType="Resource">
            <rdf:value>References</rdf:value>
            <dct:bibliographicCitation>Engel, P. "Deletions in Manuscripts and Conservators´ Decision-Making Depicted in SKOS". Conservation Update 2(2021): 25-49. DOI: 10.48341/rva1-5g91</dct:bibliographicCitation>
        </skos:definition>
        <skos:broader rdf:resource="http://gams.uni-graz.at/thesaurus/deletionMixture"/>         
    </skos:Concept>
    <skos:Concept rdf:about="http://gams.uni-graz.at/thesaurus/deletionMixture10">
        <skos:inScheme rdf:resource="http://gams.uni-graz.at/thesaurus/mss-conservation"/>
        <skos:prefLabel xml:lang="en">Mixture: Hare flesh fried and salted, wine</skos:prefLabel>
        <skos:prefLabel xml:lang="de">Mischung: Hasenfleisch gebraten und gesalzen, Wein</skos:prefLabel>
        <skos:definition rdf:parseType="Resource">
            <rdf:value>References</rdf:value>
            <dct:bibliographicCitation>Engel, P. "Deletions in Manuscripts and Conservators´ Decision-Making Depicted in SKOS". Conservation Update 2(2021): 25-49. DOI: 10.48341/rva1-5g91</dct:bibliographicCitation>
        </skos:definition>
        <skos:broader rdf:resource="http://gams.uni-graz.at/thesaurus/deletionMixture"/>         
    </skos:Concept>
    <skos:Concept rdf:about="http://gams.uni-graz.at/thesaurus/deletionMixture11">
        <skos:inScheme rdf:resource="http://gams.uni-graz.at/thesaurus/mss-conservation"/>
        <skos:prefLabel xml:lang="en">Mixture: bone marrow, oil</skos:prefLabel>
        <skos:prefLabel xml:lang="de">Mischung: Knochenmark, Öl</skos:prefLabel>
        <skos:definition rdf:parseType="Resource">
            <rdf:value>References</rdf:value>
            <dct:bibliographicCitation>Engel, P. "Deletions in Manuscripts and Conservators´ Decision-Making Depicted in SKOS". Conservation Update 2(2021): 25-49. DOI: 10.48341/rva1-5g91</dct:bibliographicCitation>
        </skos:definition>
        <skos:broader rdf:resource="http://gams.uni-graz.at/thesaurus/deletionMixture"/>         
    </skos:Concept>
    <skos:Concept rdf:about="http://gams.uni-graz.at/thesaurus/deletionMixture12">
        <skos:inScheme rdf:resource="http://gams.uni-graz.at/thesaurus/mss-conservation"/>
        <skos:prefLabel xml:lang="en">Mixture: Malus sylvestris (low pH) juice, and a rough cloth</skos:prefLabel>
        <skos:prefLabel xml:lang="de">Mischung: Saft aus Malus sylvestris</skos:prefLabel>
        <skos:definition rdf:parseType="Resource">
            <rdf:value>References</rdf:value>
            <dct:bibliographicCitation>Engel, P. "Deletions in Manuscripts and Conservators´ Decision-Making Depicted in SKOS". Conservation Update 2(2021): 25-49. DOI: 10.48341/rva1-5g91</dct:bibliographicCitation>
        </skos:definition>
        <skos:broader rdf:resource="http://gams.uni-graz.at/thesaurus/deletionMixture"/>        
    </skos:Concept>
    <skos:Concept rdf:about="http://gams.uni-graz.at/thesaurus/deletionMixture13">
        <skos:inScheme rdf:resource="http://gams.uni-graz.at/thesaurus/mss-conservation"/>
        <skos:prefLabel xml:lang="en">Mixture: Wine yeast (saccharomyces cerevisiae), ashes, water</skos:prefLabel>
        <skos:prefLabel xml:lang="de">Mischung: Weinhefe (saccharomyces cerevisiae), Asche, Wasser</skos:prefLabel>
        <skos:definition rdf:parseType="Resource">
            <rdf:value>References</rdf:value>
            <dct:bibliographicCitation>Engel, P. "Deletions in Manuscripts and Conservators´ Decision-Making Depicted in SKOS". Conservation Update 2(2021): 25-49. DOI: 10.48341/rva1-5g91</dct:bibliographicCitation>
        </skos:definition>
        <skos:broader rdf:resource="http://gams.uni-graz.at/thesaurus/deletionMixture"/>         
    </skos:Concept>
    <skos:Concept rdf:about="http://gams.uni-graz.at/thesaurus/deletionMixture14">
        <skos:inScheme rdf:resource="http://gams.uni-graz.at/thesaurus/mss-conservation"/>
        <skos:prefLabel xml:lang="en">Mixture: lime, flour, water, egg shells</skos:prefLabel>
        <skos:prefLabel xml:lang="de">Mischung: Kalk, Mehl, Wasser, Eierschale</skos:prefLabel>
        <skos:definition rdf:parseType="Resource">
            <rdf:value>References</rdf:value>
            <dct:bibliographicCitation>Engel, P. "Deletions in Manuscripts and Conservators´ Decision-Making Depicted in SKOS". Conservation Update 2(2021): 25-49. DOI: 10.48341/rva1-5g91</dct:bibliographicCitation>
        </skos:definition>
        <skos:broader rdf:resource="http://gams.uni-graz.at/thesaurus/deletionMixture"/>         
    </skos:Concept>    
    <!--    ########### Unintentional Damages #############-->
    <skos:Concept rdf:about="http://gams.uni-graz.at/thesaurus/unintentionalDamage">
        <skos:inScheme rdf:resource="http://gams.uni-graz.at/thesaurus/conservation"/>
        <skos:prefLabel xml:lang="en">Unintentional damage</skos:prefLabel>
        <skos:altLabel xml:lang="en">Unintentional alteration</skos:altLabel>
        <skos:prefLabel xml:lang="de">Unabsichtliche Schäden</skos:prefLabel>
        <skos:definition xml:lang="en">An unintentional damage on the whole or part of the manuscript.</skos:definition>
        <skos:broader rdf:resource="http://gams.uni-graz.at/thesaurus/damages"/>
    </skos:Concept>
    <skos:Concept rdf:about="http://gams.uni-graz.at/thesaurus/other-agents">
        <skos:inScheme rdf:resource="http://gams.uni-graz.at/thesaurus/conservation"/>
        <skos:prefLabel xml:lang="en">Other agents</skos:prefLabel>
        <skos:prefLabel xml:lang="de">Andere Schadenverursacher</skos:prefLabel>
        <skos:definition xml:lang="en"/>
        <skos:broader rdf:resource="http://gams.uni-graz.at/thesaurus/unintentionalDamage"/>
    </skos:Concept>
    <skos:Concept rdf:about="http://gams.uni-graz.at/thesaurus/surfaceDirt">
        <skos:inScheme rdf:resource="http://gams.uni-graz.at/thesaurus/conservation"/>
        <skos:prefLabel xml:lang="en">Surface dirt</skos:prefLabel>
        <skos:prefLabel xml:lang="de">Verschmutzung</skos:prefLabel>
        <skos:definition xml:lang="en">Any dirt on the surface of the pages or binding. It may be imbedded or superficial.</skos:definition>
        <skos:broader rdf:resource="http://gams.uni-graz.at/thesaurus/other-agents"/>
    </skos:Concept>        
    <skos:Concept rdf:about="http://gams.uni-graz.at/thesaurus/stains">
        <skos:inScheme rdf:resource="http://gams.uni-graz.at/thesaurus/conservation"/>
        <skos:prefLabel xml:lang="en">Stains</skos:prefLabel>
        <skos:prefLabel xml:lang="de">Flecken</skos:prefLabel>
        <skos:definition xml:lang="en">Stains are areas, which show a colour or surface gloss which is different from that of the surrounding area.            
            Virtually any substance may cause a stain. Stains are often caused by drinks (coffee, tea, or wine), ink splashed onto the page or candle material (wax and other components). If the stain was caused by a liquid, it shows the characteristic splashes.            
            Stains however can also be produced by the excrement of insects, bird, bats and rodents, by iron movement from one page to the other in case of ink- or copper corrosion or silver leaf in precious manuscripts; they can be caused by insects or spiders squeezed in a fold or from plants pressed in books. Greasy stains may come from food and often stains are caused by renovation work in the room where the book is kept, from scholars who tried to read a deleted text and applied mixes of substances to bring out the text or by conservators, who used the wrong material.            
            Sometimes stains occur only over time – for example, when transparent surface sizing is used on paper and turns yellow only with ageing. Such stains should not be treated, as these are an immediate part of the paper.
            A particular kind of fleck-like spots on paper is characteristic to foxing – a chemical damage inflicting paper.</skos:definition>
        <skos:definition rdf:parseType="Resource">
            <rdf:value>References</rdf:value>            
            <dct:bibliographicCitation>Archives Damage Atlas, pp. 42-45 (accessed 13.04.2023)
                https://www.metamorfoze.nl/sites/default/files/documents/schadeatlas-2010%20engels.pdf</dct:bibliographicCitation>
        </skos:definition>
        <skos:broader rdf:resource="http://gams.uni-graz.at/thesaurus/other-agents"/>
    </skos:Concept>
    
   
    
    <skos:Concept rdf:about="http://gams.uni-graz.at/thesaurus/waterDamage">
        <skos:inScheme rdf:resource="http://gams.uni-graz.at/thesaurus/conservation"/>
        <skos:prefLabel xml:lang="en">Water damage</skos:prefLabel>
        <skos:prefLabel xml:lang="de">Wasserschaden</skos:prefLabel>
        <skos:definition xml:lang="en">Water damage are caused either by floods or the extinguishing water in case of fire. These include stains and discolourations, felting, mould, stuck sheets and warping of the text block or whole book due to excessive moisture.</skos:definition>
        <skos:definition rdf:parseType="Resource">
            <rdf:value>References</rdf:value>
            <dct:bibliographicCitation>Archives Damage Atlas, pp. 117-139 (accessed 13.04.2023)
                https://www.metamorfoze.nl/sites/default/files/documents/schadeatlas-2010%20engels.pdf</dct:bibliographicCitation>
            <dct:bibliographicCitation>Salvaging library and archive collections. British Library conservation guide (accessed 13.04.2023). https://www.bl.uk/britishlibrary/~/media/bl/global/conservation/pdf-guides/salvaging-library-and-archive-collections-preservation-guide.pdf</dct:bibliographicCitation>            
        </skos:definition>        
        <skos:broader rdf:resource="http://gams.uni-graz.at/thesaurus/unintentionalDamage"/>
    </skos:Concept>
    <skos:Concept rdf:about="http://gams.uni-graz.at/thesaurus/schwemmrand">
        <skos:inScheme rdf:resource="http://gams.uni-graz.at/thesaurus/conservation"/>
        <skos:prefLabel xml:lang="en">Tide lines</skos:prefLabel>
        <skos:prefLabel xml:lang="de">Schwemmränder</skos:prefLabel>
        <skos:definition xml:lang="en">An alluvial edge occurs when a liquid (water or other) meets an absorbent material and washes coloured particles to the boundary between the liquid-soaked and dry material, where they condense to form a visible edge. These particles can either originate from the liquid itself or be dissolved from the material by the liquid.</skos:definition>
        <skos:broader rdf:resource="http://gams.uni-graz.at/thesaurus/waterDamage"/>
    </skos:Concept>
    <skos:Concept rdf:about="http://gams.uni-graz.at/thesaurus/mould">
        <skos:inScheme rdf:resource="http://gams.uni-graz.at/thesaurus/conservation"/>
        <skos:prefLabel xml:lang="en">Mould</skos:prefLabel>
        <skos:prefLabel xml:lang="de">Schimmel</skos:prefLabel>
        <skos:definition xml:lang="en">Mould is a type of fungus. In favourable conditions its spores can quickly germinate and cause severe damage: from small spots and discolourations to decomposition of parts of the paper.</skos:definition>
        <skos:definition rdf:parseType="Resource">
            <rdf:value>References</rdf:value>
            <dct:bibliographicCitation>Archives Damage Atlas, pp. 128-133 (accessed 13.04.2023)
                https://www.metamorfoze.nl/sites/default/files/documents/schadeatlas-2010%20engels.pdf</dct:bibliographicCitation>
            <dct:bibliographicCitation>Mould outbreaks in library and archive collections (PDF format). British Library conservation guide (accessed 13.04.2023). https://www.bl.uk/britishlibrary/~/media/bl/global/conservation/pdf-guides/mould-outbreaks-in-libraries-preservation-guide.pdf</dct:bibliographicCitation>
        </skos:definition>
        <skos:broader rdf:resource="http://gams.uni-graz.at/thesaurus/waterDamage"/>
    </skos:Concept>
    <skos:Concept rdf:about="http://gams.uni-graz.at/thesaurus/softeningBindingAgent">
        <skos:inScheme rdf:resource="http://gams.uni-graz.at/thesaurus/conservation"/>
        <skos:prefLabel xml:lang="en">Softening of binding agents</skos:prefLabel>
        <skos:prefLabel xml:lang="de">Anquellen von Bindemitteln</skos:prefLabel>
        <skos:definition xml:lang="en"/>
        <skos:broader rdf:resource="http://gams.uni-graz.at/thesaurus/waterDamage"/>
    </skos:Concept>
    <skos:Concept rdf:about="http://gams.uni-graz.at/thesaurus/mechanical">
        <skos:inScheme rdf:resource="http://gams.uni-graz.at/thesaurus/conservation"/>
        <skos:prefLabel xml:lang="en">Mechanical damage</skos:prefLabel>
        <skos:prefLabel xml:lang="de">Mechanische Schäden</skos:prefLabel>
        <skos:definition xml:lang="en">Mechanical damages are usually man-made caused by wear, transport or mishandling the material. They may include kinks, folds and cracks of the leaves, which may further lead to tears, fractures or even detached leaves or fragments thereof.</skos:definition>
        <skos:definition rdf:parseType="Resource">
            <rdf:value>References</rdf:value>
            <dct:bibliographicCitation>Archives Damage Atlas, pp. 81-99 (accessed 13.04.2023)
                https://www.metamorfoze.nl/sites/default/files/documents/schadeatlas-2010%20engels.pdf</dct:bibliographicCitation>
        </skos:definition>        
        <skos:broader rdf:resource="http://gams.uni-graz.at/thesaurus/unintentionalDamage"/>
    </skos:Concept>
    <skos:Concept rdf:about="http://gams.uni-graz.at/thesaurus/crackedBoards">
        <skos:inScheme rdf:resource="http://gams.uni-graz.at/thesaurus/conservation"/>
        <skos:prefLabel xml:lang="en">Cracked boards</skos:prefLabel>
        <skos:prefLbel xml:lang="de">Riss oder Spalt an den Holzdeckeln</skos:prefLbel>
        <skos:definition xml:lang="en">Cracks or splits of the binding boards.</skos:definition>
        <skos:broader rdf:resource="http://gams.uni-graz.at/thesaurus/mechanical"/>
    </skos:Concept>
    <skos:Concept rdf:about="http://gams.uni-graz.at/thesaurus/abbrasion">
        <skos:inScheme rdf:resource="http://gams.uni-graz.at/thesaurus/conservation"/>
        <skos:prefLabel xml:lang="en"></skos:prefLabel>
        <skos:prefLbel xml:lang="de">Abreiben</skos:prefLbel>
        <skos:altLbel xml:lang="de">Abbrasion</skos:altLbel>
        <skos:definition xml:lang="en">Cracks or splits of the binding boards.</skos:definition>
        <skos:broader rdf:resource="http://gams.uni-graz.at/thesaurus/mechanical"/>
    </skos:Concept>
    <skos:Concept rdf:about="http://gams.uni-graz.at/thesaurus/fold">
        <skos:inScheme rdf:resource="http://gams.uni-graz.at/thesaurus/conservation"/>
        <skos:prefLabel xml:lang="en">Fold</skos:prefLabel>
        <skos:altLbel xml:lang="en">Crease</skos:altLbel>
        <skos:altLbel xml:lang="en">Wrinkle</skos:altLbel>
        <skos:prefLabel xml:lang="de">Falte</skos:prefLabel>
        <skos:altLbel xml:lang="de">Knick</skos:altLbel>
        <skos:definition xml:lang="en">Deformation of leaves which weaken its structure and can further lead to tears.</skos:definition>
        <skos:broader rdf:resource="http://gams.uni-graz.at/thesaurus/mechanical"/>
    </skos:Concept>
    <skos:Concept rdf:about="http://gams.uni-graz.at/thesaurus/cut">
        <skos:inScheme rdf:resource="http://gams.uni-graz.at/thesaurus/conservation"/>
        <skos:prefLabel xml:lang="en">Cut</skos:prefLabel>
        <skos:prefLbel xml:lang="de">Schnitt</skos:prefLbel>
        <skos:definition xml:lang="en">Cuts made by a knife or a pair of scissors usually have sharp edges, which distinguish them from tears.</skos:definition>
        <skos:broader rdf:resource="http://gams.uni-graz.at/thesaurus/mechanical"/>
    </skos:Concept>
    <skos:Concept rdf:about="http://gams.uni-graz.at/thesaurus/hole">
        <skos:inScheme rdf:resource="http://gams.uni-graz.at/thesaurus/conservation"/>
        <skos:prefLabel xml:lang="en">Hole</skos:prefLabel>
        <skos:prefLbel xml:lang="de">Loch</skos:prefLbel>
        <skos:definition xml:lang="en">Some holes were made deliberately in the procedure of making a manuscript, such as piercings for the lines of the text, the margins, but also for ticketing to hold together the quires in the right order before bookbinding as a help for the bookbinders. The preparation for the sewing includes also tiny slits or piercings in the gutter to accommodate the sewing thread.
        For holes made by insects and rodents see the respective entries under 'Pest infestation'.</skos:definition>
        <skos:broader rdf:resource="http://gams.uni-graz.at/thesaurus/mechanical"/>
    </skos:Concept>
    <skos:Concept rdf:about="http://gams.uni-graz.at/thesaurus/loss">
        <skos:inScheme rdf:resource="http://gams.uni-graz.at/thesaurus/conservation"/>
        <skos:prefLabel xml:lang="en">Loss</skos:prefLabel>
        <skos:prefLbel xml:lang="de">Fehlstelle</skos:prefLbel>
        <skos:definition xml:lang="en">Loss is a broader term, which may be applied to any detached or missing parts of the book block or binding.</skos:definition>
        <skos:definition rdf:parseType="Resource">
            <rdf:value>References</rdf:value>
            <dct:bibliographicCitation>Book and Paper Group Wiki. 2022. Book and Paper Group Wiki. American Institute for Conservation (AIC). Accessed April 17, 2023. https://www.conservation-wiki.com/wiki/Book_and_Paper_Group_Wiki</dct:bibliographicCitation>
            <dct:bibliographicCitation>Adam Agnes and Wolfgang Kreuzer. Die Fehlstellenergänzung von Pergament am Einband und am Schriftträger. Forschungsblog (accessed 13.04.2023) https://www.onb.ac.at/news-einzelansicht/die-fehlstellenergaenzung-von-pergament-am-einband-und-am-schrifttraeger</dct:bibliographicCitation>
        </skos:definition>
        <skos:broader rdf:resource="http://gams.uni-graz.at/thesaurus/mechanical"/>
    </skos:Concept>  
    <skos:Concept rdf:about="http://gams.uni-graz.at/thesaurus/lacuna">
        <skos:inScheme rdf:resource="http://gams.uni-graz.at/thesaurus/conservation"/>
        <skos:prefLabel xml:lang="en">Lacuna</skos:prefLabel>
        <skos:altLbel xml:lang="en">Lacuna</skos:altLbel>
        <skos:prefLbel xml:lang="de">Fehlstelle</skos:prefLbel>
        <skos:definition xml:lang="en">Lacuna is an area of the writing support which is physically detached or missing, be it by having been cut out by people or eaten by rodents or caused by aggressive substances.</skos:definition>
        <skos:broader rdf:resource="http://gams.uni-graz.at/thesaurus/loss"/>
    </skos:Concept>
    
    <skos:Concept rdf:about="http://gams.uni-graz.at/thesaurus/tornLeaves">
        <skos:inScheme rdf:resource="http://gams.uni-graz.at/thesaurus/conservation"/>
        <skos:prefLabel xml:lang="en">Torn out leaves</skos:prefLabel>
        <skos:prefLabel xml:lang="de">Herausgerissene Blätter</skos:prefLabel>
        <skos:definition xml:lang="en">Leaves which are torn out from the book block and missing.</skos:definition>
        <skos:broader rdf:resource="http://gams.uni-graz.at/thesaurus/loss"/>
    </skos:Concept>
    <skos:Concept rdf:about="http://gams.uni-graz.at/thesaurus/tear">
        <skos:inScheme rdf:resource="http://gams.uni-graz.at/thesaurus/conservation"/>
        <skos:prefLabel xml:lang="en">Tear</skos:prefLabel>
        <skos:prefLabel xml:lang="de">Riss</skos:prefLabel>
        <skos:altLabel xml:lang="de">Beschädigung durch Zerreißen</skos:altLabel>
        <skos:definition xml:lang="en">Tears may be observed particularly on the leaves' edges (tears along the edges or else known as frayed edges). In most cases these are due to careless use, often in combination with improper storage.</skos:definition>
        <skos:definition rdf:parseType="Resource">
            <rdf:value>References</rdf:value>
            <dct:bibliographicCitation>Archives Damage Atlas, pp. 81-99 (accessed 13.04.2023)
                https://www.metamorfoze.nl/sites/default/files/documents/schadeatlas-2010%20engels.pdf</dct:bibliographicCitation>            
        </skos:definition>
        <skos:broader rdf:resource="http://gams.uni-graz.at/thesaurus/mechanical"/>
    </skos:Concept>
        
    <skos:Concept rdf:about="http://gams.uni-graz.at/thesaurus/chemicalDamage">
        <skos:inScheme rdf:resource="http://gams.uni-graz.at/thesaurus/conservation"/>
        <skos:prefLabel xml:lang="en">Chemical damage</skos:prefLabel>
        <skos:prefLabel xml:lang="de">Chemische Schäden</skos:prefLabel>
        <skos:definition xml:lang="en">Alteration and deterioration of the material caused either by its intrinsic chemical composition (e.g. chemical composition of ink in the case of ink corrosion) or by external accidents (e.g. fire damage) and factors (e.g. gelatinisation).</skos:definition>
        <skos:broader rdf:resource="http://gams.uni-graz.at/thesaurus/unintentionalDamage"/>
    </skos:Concept>   
    <skos:Concept rdf:about="http://gams.uni-graz.at/thesaurus/fireDamage">
        <skos:inScheme rdf:resource="http://gams.uni-graz.at/thesaurus/conservation"/>
        <skos:prefLabel xml:lang="en">Carbonisation</skos:prefLabel>
        <skos:altLabel xml:lang="en">Fire damage</skos:altLabel>
        <skos:prefLabel xml:lang="de">Brandschaden</skos:prefLabel>
        <skos:definition xml:lang="en">The Archive Damage Atlas classifies fire damage as chemical one, because burning is essentially oxidation (a reaction with oxygen). Possible damages caused by fire, gas, smoke and indirect heat: charred areas; fragile and brittle leaves; illegible writing; leaves burnt along their edges; smudge. In the event of fire books often suffer furthermore damages through the impact of water and extinguishing agents.</skos:definition>
        <skos:definition rdf:parseType="Resource">
            <rdf:value>References</rdf:value>
            <dct:bibliographicCitation>Archives Damage Atlas, pp. 36-41 (accessed 13.04.2023)
                https://www.metamorfoze.nl/sites/default/files/documents/schadeatlas-2010%20engels.pdf</dct:bibliographicCitation>
            <dct:bibliographicCitation>Salvaging library and archive collections. British Library conservation guide (accessed 13.04.2023). https://www.bl.uk/britishlibrary/~/media/bl/global/conservation/pdf-guides/salvaging-library-and-archive-collections-preservation-guide.pdf</dct:bibliographicCitation>            
            <dct:bibliographicCitation>Völkel Laura et al. Assessing Fire-Damage in Historical Papers and Alleviating Damage with Soft Cellulose Nanofibers".  In Nano-Micro Small 18 (2022). https://doi.org/10.1002/smll.202105420</dct:bibliographicCitation>
            <dct:bibliographicCitation>Pottier Fabien et al. "Recovering illegible writings in fire-damaged medieval manuscripts through data treatment of UV-fluorescence photography". Journal of Cultural Heritage 36(2019): 183-190. https://hal.science/hal-03027994</dct:bibliographicCitation>
        </skos:definition>        
        <skos:broader rdf:resource="http://gams.uni-graz.at/thesaurus/chemicalDamage"/>
    </skos:Concept>
    <skos:Concept rdf:about="http://gams.uni-graz.at/thesaurus/gelatinization">
        <skos:inScheme rdf:resource="http://gams.uni-graz.at/thesaurus/conservation"/>
        <skos:prefLabel xml:lang="en">Gelatinization</skos:prefLabel>
        <skos:altLabel xml:lang="en">Gelatinisation</skos:altLabel>
        <skos:prefLabel xml:lang="de">Pergamentgelatinierung</skos:prefLabel>
        <skos:definition xml:lang="en">Occurs on parchment and is caused by elevated humidity and temperature. The appearance is a yellow glossy glass-like and hard parchment.</skos:definition>
        <skos:broader rdf:resource="http://gams.uni-graz.at/thesaurus/chemicalDamage"/>
    </skos:Concept>
    <skos:Concept rdf:about="http://gams.uni-graz.at/thesaurus/paperDegradation">
        <skos:inScheme rdf:resource="http://gams.uni-graz.at/thesaurus/conservation"/>
        <skos:prefLabel xml:lang="en">Acidic paper decay</skos:prefLabel>
        <skos:altLabel xml:lang="en">Paper degradation</skos:altLabel>
        <skos:prefLabel xml:lang="de">Saurer Papierabbau</skos:prefLabel>
        <skos:definition xml:lang="en">Unlike parchment, paper is frequently prone to degradation, due in part to alkaline agents such as lime and chalk that are used in the manufacturing process.</skos:definition>
        <skos:broader rdf:resource="http://gams.uni-graz.at/thesaurus/chemicalDamage"/>
    </skos:Concept> 
    <skos:Concept rdf:about="http://gams.uni-graz.at/thesaurus/metalCorrosion">
        <skos:inScheme rdf:resource="http://gams.uni-graz.at/thesaurus/conservation"/>
        <skos:prefLabel xml:lang="en">Metal corrosion</skos:prefLabel>
        <skos:prefLabel xml:lang="de">Korrosion</skos:prefLabel>
        <skos:definition xml:lang="en">The deterioration of metal by chemical or electrochemical reaction resulting from exposure to weathering, moisture, chemicals, or other agents.</skos:definition>
        <skos:related rdf:resource="http://vocab.getty.edu/page/aat/300054107"/>
        <skos:definition rdf:parseType="Resource">
            <rdf:value>References</rdf:value>
            <dct:bibliographicCitation>Corrosion. AIC Wiki (accessed 16.05.2023) https://www.conservation-wiki.com/wiki/Corrosion</dct:bibliographicCitation>
        </skos:definition>
        <skos:broader rdf:resource="http://gams.uni-graz.at/thesaurus/chemicalDamage"/>
    </skos:Concept>
    <skos:Concept rdf:about="http://gams.uni-graz.at/thesaurus/tapeResidue">
        <skos:inScheme rdf:resource="http://gams.uni-graz.at/thesaurus/conservation"/>
        <skos:prefLabel xml:lang="en">Tape and sticker residue</skos:prefLabel>
        <skos:altLabel xml:lang="en">Tape and stcker decay</skos:altLabel>
        <skos:prefLabel xml:lang="de">Abbau von Klebebendern</skos:prefLabel>
        <skos:definition xml:lang="en">Damages caused by the use of tape and stickers may include: discolouration of the tape and the writing surface on which it is applied; a browned layer of glue on the surface; a glue residue causing pages to stick together.</skos:definition>
        <skos:definition rdf:parseType="Resource">
            <rdf:value>References</rdf:value>
            <dct:bibliographicCitation>Archives Damage Atlas, pp. 58-63 (accessed 13.04.2023)
                https://www.metamorfoze.nl/sites/default/files/documents/schadeatlas-2010%20engels.pdf</dct:bibliographicCitation>
            
        </skos:definition>
        <skos:broader rdf:resource="http://gams.uni-graz.at/thesaurus/chemicalDamage"/>
    </skos:Concept>
    <skos:Concept rdf:about="http://gams.uni-graz.at/thesaurus/leatherDecay">
        <skos:inScheme rdf:resource="http://gams.uni-graz.at/thesaurus/conservation"/>
        <skos:prefLabel xml:lang="en">Leather decay</skos:prefLabel>
        <skos:prefLabel xml:lang="de">Ledderabbau</skos:prefLabel>
        <skos:definition xml:lang="en">Damage on the leather surface of bookbindings, caused usually by the tanning process of leather. The leather may be brittle; fibres or whole pieces of leather can easily come loose.</skos:definition>
        <skos:definition rdf:parseType="Resource">
            <rdf:value>References</rdf:value>
            <dct:bibliographicCitation>Archives Damage Atlas, p. 28 (accessed 16.05.2023)
                https://www.metamorfoze.nl/sites/default/files/documents/schadeatlas-2010%20engels.pdf</dct:bibliographicCitation>
            
        </skos:definition>
        <skos:broader rdf:resource="http://gams.uni-graz.at/thesaurus/chemicalDamage"/>
    </skos:Concept>
    <skos:Concept rdf:about="http://gams.uni-graz.at/thesaurus/warping">
        <skos:inScheme rdf:resource="http://gams.uni-graz.at/thesaurus/conservation"/>
        <skos:prefLabel xml:lang="en">Warping</skos:prefLabel>
        <skos:altLbel xml:lang="en">Distortion</skos:altLbel>
        <skos:prefLabel xml:lang="de">Verwerfungen</skos:prefLabel>
        <skos:definition xml:lang="en">Planar distortion of the surface by which the material (book cover, quires or single leaves) bends and distorts its original flat form.</skos:definition>
        <skos:definition rdf:parseType="Resource">
            <rdf:value>References</rdf:value>
            <dct:bibliographicCitation>Archives Damage Atlas, p. 12 (accessed 16.05.2023)
                https://www.metamorfoze.nl/sites/default/files/documents/schadeatlas-2010%20engels.pdf</dct:bibliographicCitation>
            
        </skos:definition>
        <skos:related rdf:resource="http://vocab.getty.edu/page/aat/300155059"/>
        <skos:broader rdf:resource="http://gams.uni-graz.at/thesaurus/chemicalDamage"/>
    </skos:Concept>
    <skos:Concept rdf:about="http://gams.uni-graz.at/thesaurus/deteriorationInkPigment">
        <skos:inScheme rdf:resource="http://gams.uni-graz.at/thesaurus/conservation"/>
        <skos:prefLabel xml:lang="en">Deterioration of inks, colourants, and varnish</skos:prefLabel>
        <skos:prefLabel xml:lang="de">Abbau von Tinten, Farbmitteln und Überzug</skos:prefLabel>
        <skos:definition xml:lang="en"></skos:definition>        
        <skos:broader rdf:resource="http://gams.uni-graz.at/thesaurus/chemicalDamage"/>
    </skos:Concept>
    <skos:Concept rdf:about="http://gams.uni-graz.at/thesaurus/discolouration">
        <skos:inScheme rdf:resource="http://gams.uni-graz.at/thesaurus/conservation"/>
        <skos:prefLabel xml:lang="en">Discolouration</skos:prefLabel>
        <skos:altLbel xml:lang="en">Fading</skos:altLbel>
        <skos:prefLabel xml:lang="de">Ausbleichen</skos:prefLabel>
        <skos:altLbel xml:lang="de">Verbräunen</skos:altLbel>
        <skos:altLbel xml:lang="de">Verfärbung</skos:altLbel>
        <skos:definition xml:lang="en">Colour change can be caused by internal reaction of substances or by light impact. Any dye (including some inks) can fade to lighter or even invisible colour. Green pigments change to brown over time and red and while lead pigments change to black.</skos:definition>
        <skos:definition rdf:parseType="Resource">
            <rdf:value>References</rdf:value>   
            <dct:bibliographicCitation>AIC Wiki (accessed 16.05.2023)
                https://www.conservation-wiki.com/wiki/Fading</dct:bibliographicCitation>            
        </skos:definition>
        <skos:related rdf:resource="http://vocab.getty.edu/page/aat/300053045"/>
        <skos:broader rdf:resource="http://gams.uni-graz.at/thesaurus/deteriorationInkPigment"/>
    </skos:Concept>
    <skos:Concept rdf:about="http://gams.uni-graz.at/thesaurus/inkCorrosion">
        <skos:inScheme rdf:resource="http://gams.uni-graz.at/thesaurus/conservation"/>
        <skos:prefLabel xml:lang="en">Ink corrosion</skos:prefLabel>
        <skos:prefLabel xml:lang="de">Tintenfraß</skos:prefLabel>
        <skos:definition xml:lang="en">Ink corrosion involves a presence of iron gall ink, often brown text and the corroded area, if it creates a lacuna, is brown on the verso and brittle. The appearance of ink corrosion at its various stages has been well described by Reissland.</skos:definition>
        <skos:definition rdf:parseType="Resource">
            <rdf:value>References</rdf:value>   
            <dct:bibliographicCitation>Archives Damage Atlas, pp. 46-51 (accessed 13.04.2023)
                https://www.metamorfoze.nl/sites/default/files/documents/schadeatlas-2010%20engels.pdf</dct:bibliographicCitation>
            <dct:bibliographicCitation>Reissland, Birgit. "Ink Corrosion. Aqueous and Non-Aqueous Treatment of Paper Objects – State of the Art" , vol. 20, no. 3-4, 1999, pp. 167-180. https://doi-org.uaccess.univie.ac.at/10.1515/rest.1999.20.3-4.167</dct:bibliographicCitation>
        </skos:definition>
        <skos:broader rdf:resource="http://gams.uni-graz.at/thesaurus/deteriorationInkPigment"/>
    </skos:Concept>
    <skos:Concept rdf:about="http://gams.uni-graz.at/thesaurus/copperCorrosion">
        <skos:inScheme rdf:resource="http://gams.uni-graz.at/thesaurus/conservation"/>
        <skos:prefLabel xml:lang="en">Copper corrosion</skos:prefLabel>
        <skos:prefLabel xml:lang="de">Kupferfraß</skos:prefLabel>
        <skos:definition xml:lang="en">In case of copper corrosion green-painted sections on paper or parchment bleed through to the reverse side and turn brown. The lacuna has sharp edges and the area is actually broken out. The stability of the writing material (especially that of paper) decreases sharply, so that the leaves may break under low stress, e.g. when turning the pages.</skos:definition>
        <skos:definition rdf:parseType="Resource">
            <rdf:value>References</rdf:value>   
            <dct:bibliographicCitation>Archives Damage Atlas, pp. 52-57 (accessed 13.04.2023)
                https://www.metamorfoze.nl/sites/default/files/documents/schadeatlas-2010%20engels.pdf</dct:bibliographicCitation>
        </skos:definition>
        <skos:broader rdf:resource="http://gams.uni-graz.at/thesaurus/deteriorationInkPigment"/>
    </skos:Concept>
    <skos:Concept rdf:about="http://gams.uni-graz.at/thesaurus/crackle">
        <skos:inScheme rdf:resource="http://gams.uni-graz.at/thesaurus/conservation"/>
        <skos:prefLabel xml:lang="en">Crackle</skos:prefLabel>
        <skos:altLabel xml:lang="en">Craquelure</skos:altLabel>
        <skos:prefLabel xml:lang="de">Craquelé</skos:prefLabel>
        <skos:altLabel xml:lang="de">Krakelee</skos:altLabel>
        <skos:definition xml:lang="en">A network of fine fracture lines in a coating layer, such as a ground, paint layer, varnish, or glaze.</skos:definition>
        <skos:definition rdf:parseType="Resource">
            <rdf:value>References</rdf:value>   
            <dct:bibliographicCitation>AIC Wiki (accessed 1.05.2023) https://www.conservation-wiki.com/wiki/Crackle</dct:bibliographicCitation>
        </skos:definition> 
        <skos:related rdf:resource="http://vocab.getty.edu/page/aat/300228345"/>
        <skos:broader rdf:resource="http://gams.uni-graz.at/thesaurus/deteriorationInkPigment"/>
    </skos:Concept>
    <skos:Concept rdf:about="http://gams.uni-graz.at/thesaurus/tarnish">
        <skos:inScheme rdf:resource="http://gams.uni-graz.at/thesaurus/conservation"/>
        <skos:prefLabel xml:lang="en">Tarnish</skos:prefLabel>
        <skos:prefLabel xml:lang="de">Beschlag</skos:prefLabel>
        <skos:altLabel xml:lang="de">Anlaufen</skos:altLabel>
        <skos:definition xml:lang="en">A discoloration or dulling of a metal surface due to a chemical reaction.</skos:definition>
        <skos:definition rdf:parseType="Resource">
            <rdf:value>References</rdf:value>   
            <dct:bibliographicCitation>Tarnish. AIC Wiki (accessed 1.05.2023) https://www.conservation-wiki.com/wiki/Tarnish</dct:bibliographicCitation>
        </skos:definition> 
        <skos:related rdf:resource="http://vocab.getty.edu/page/aat/300219955"/>
        <skos:broader rdf:resource="http://gams.uni-graz.at/thesaurus/deteriorationInkPigment"/>
    </skos:Concept>
    <skos:Concept rdf:about="http://gams.uni-graz.at/thesaurus/flaking">
        <skos:inScheme rdf:resource="http://gams.uni-graz.at/thesaurus/conservation"/>
        <skos:prefLabel xml:lang="en">Flaking</skos:prefLabel>
        <skos:altLabel xml:lang="en">Powdering</skos:altLabel>
        <skos:altLabel xml:lang="en">Chalking</skos:altLabel>
        <skos:altLabel xml:lang="en">Cleavage</skos:altLabel>
        <skos:prefLabel xml:lang="de">Abplatzung</skos:prefLabel>
        <skos:altLabel xml:lang="de">Abplatzen</skos:altLabel>
        <skos:definition xml:lang="en">Flaking off of areas of metal leaf or pigment/dye–binder composites are caused either by priming or binder quality, bad handling or a fluctuation of temperature and humidity.</skos:definition>
        <skos:definition rdf:parseType="Resource">
            <rdf:value>References</rdf:value>   
            <dct:bibliographicCitation>Flaking. AIC Wiki (accessed 16.05.2023) https://www.conservation-wiki.com/wiki/Flaking</dct:bibliographicCitation>
        </skos:definition> 
        <skos:related rdf:resource="http://vocab.getty.edu/page/aat/300054129"/>
        <skos:broader rdf:resource="http://gams.uni-graz.at/thesaurus/deteriorationInkPigment"/>
    </skos:Concept>    
    <skos:Concept rdf:about="http://gams.uni-graz.at/thesaurus/cupping">
        <skos:inScheme rdf:resource="http://gams.uni-graz.at/thesaurus/conservation"/>
        <skos:prefLabel xml:lang="en">Cupping</skos:prefLabel>
        <skos:prefLabel xml:lang="de">Schusselbildung</skos:prefLabel>
        <skos:definition xml:lang="en">Formation of a concavity or cuplike hollow in a paint layer.</skos:definition>
        <skos:definition rdf:parseType="Resource">
            <rdf:value>References</rdf:value>   
            <dct:bibliographicCitation>Cupping. AIC Wiki (accessed 16.05.2023)https://www.conservation-wiki.com/wiki/Cupping</dct:bibliographicCitation>
        </skos:definition> 
        <skos:related rdf:resource="http://vocab.getty.edu/page/aat/300220569"/>
        <skos:broader rdf:resource="http://gams.uni-graz.at/thesaurus/flaking"/>
    </skos:Concept>
    <skos:Concept rdf:about="http://gams.uni-graz.at/thesaurus/peeling-off">
        <skos:inScheme rdf:resource="http://gams.uni-graz.at/thesaurus/conservation"/>
        <skos:prefLabel xml:lang="en">Peeling off</skos:prefLabel>
        <skos:prefLabel xml:lang="de">Abschälen</skos:prefLabel>
        <skos:definition xml:lang="en"></skos:definition>
        <skos:definition rdf:parseType="Resource">
            <rdf:value>References</rdf:value>   
            <dct:bibliographicCitation></dct:bibliographicCitation>
        </skos:definition> 
        <skos:related rdf:resource="http://vocab.getty.edu/page/aat/300054127"/>
        <skos:broader rdf:resource="http://gams.uni-graz.at/thesaurus/flaking"/>
    </skos:Concept>
    <skos:Concept rdf:about="http://gams.uni-graz.at/thesaurus/pest">
        <skos:inScheme rdf:resource="http://gams.uni-graz.at/thesaurus/conservation"/>
        <skos:prefLabel xml:lang="en">Damages caused by pest infestation</skos:prefLabel>
        <skos:prefLabel xml:lang="de">Schädlingsbefall</skos:prefLabel>
        <skos:definition xml:lang="en">Pests, such as insects and mice, can cause enormous damage to book and archival materials. Based on the pattern, size and edges of the holes a trained conservator can differentiate between damages caused by rodents (rats and mice) or insects.</skos:definition>
        <skos:definition rdf:parseType="Resource">
            <rdf:value>References</rdf:value> 
            <dct:bibliographicCitation>Archives Damage Atlas, pp. 101-115 (accessed 13.04.2023)
                https://www.metamorfoze.nl/sites/default/files/documents/schadeatlas-2010%20engels.pdf</dct:bibliographicCitation>
            <dct:bibliographicCitation>Managing Pests in Paper-Based Collections. British Library conservation guide (accessed 13.04.2023). https://www.bl.uk/britishlibrary/~/media/bl/global/conservation/pdf-guides/managing-pests-in-paper-based-collections-guide.pdf</dct:bibliographicCitation>
            <dct:bibliographicCitation>Pests. AIC Wiki (accessed 16.05.2023) https://www.conservation-wiki.com/wiki/Pests</dct:bibliographicCitation>
        </skos:definition> 
        <skos:broader rdf:resource="http://gams.uni-graz.at/thesaurus/unintentionalDamage"/>
    </skos:Concept>
    <skos:Concept rdf:about="http://gams.uni-graz.at/thesaurus/rodents">
        <skos:inScheme rdf:resource="http://gams.uni-graz.at/thesaurus/conservation"/>
        <skos:prefLabel xml:lang="en">Damages by rodents</skos:prefLabel>
        <skos:prefLabel xml:lang="de">Nagerschäden</skos:prefLabel>
        <skos:definition xml:lang="en">Rats and mice gnaw parts of books to keep their teeth sharp or use shredded paper to make nests. The holes they produce are usually larger. Additionally, mouse urine and droppings can stain the surface and present a disease hazard (cf. British library guide). </skos:definition>
        <skos:definition rdf:parseType="Resource">
            <rdf:value>References</rdf:value> 
            <dct:bibliographicCitation>Archives Damage Atlas, pp. 114-115 (accessed 13.04.2023)
                https://www.metamorfoze.nl/sites/default/files/documents/schadeatlas-2010%20engels.pdf</dct:bibliographicCitation>
            <dct:bibliographicCitation>Managing Pests in Paper-Based Collections. British Library conservation guide (accessed 13.04.2023). https://www.bl.uk/britishlibrary/~/media/bl/global/conservation/pdf-guides/managing-pests-in-paper-based-collections-guide.pdf</dct:bibliographicCitation>
        </skos:definition>
        <skos:broader rdf:resource="http://gams.uni-graz.at/thesaurus/pest"/>
    </skos:Concept>
    <skos:Concept rdf:about="http://gams.uni-graz.at/thesaurus/insects">
        <skos:inScheme rdf:resource="http://gams.uni-graz.at/thesaurus/conservation"/>
        <skos:prefLabel xml:lang="en">Damages by insects</skos:prefLabel>
        <skos:prefLabel xml:lang="de">Insektenschäden</skos:prefLabel>
        <skos:definition xml:lang="en">Various types of insects may attack either the writing surface (paper, wood, parchment etc.) or any additional material applied on it (binding agent, mould, organic debris etc.).</skos:definition>
        <skos:definition rdf:parseType="Resource">
            <rdf:value>References</rdf:value> 
            <dct:bibliographicCitation>Archives Damage Atlas, pp. 102-113 (accessed 13.04.2023)
                https://www.metamorfoze.nl/sites/default/files/documents/schadeatlas-2010%20engels.pdf</dct:bibliographicCitation>
            <dct:bibliographicCitation>Managing Pests in Paper-Based Collections. British Library conservation guide (accessed 13.04.2023). https://www.bl.uk/britishlibrary/~/media/bl/global/conservation/pdf-guides/managing-pests-in-paper-based-collections-guide.pdf</dct:bibliographicCitation>
        </skos:definition>
        <skos:broader rdf:resource="http://gams.uni-graz.at/thesaurus/pest"/>
    </skos:Concept>
    <skos:Concept rdf:about="http://gams.uni-graz.at/thesaurus/previousRepairs">
        <skos:inScheme rdf:resource="http://gams.uni-graz.at/thesaurus/conservation"/>
        <skos:prefLabel xml:lang="en">Previous repairs</skos:prefLabel>
        <skos:altLabel xml:lang="en">Previous conservation treatments</skos:altLabel>
        <skos:prefLabel xml:lang="de">Schaden durch alte Reparaturen</skos:prefLabel>
        <skos:altLabel xml:lang="de">Frühere konservatorische Maßnahme</skos:altLabel>
        <skos:definition xml:lang="en">Implied are all previous measures intended to secure the conservation of the book. Previous repairs may have been carries out already during or immediately after the production of the manuscript (e.g. repairing holes in the parchment by stitching or gluing additional parchment pieces). In modern times one used materials which in time damaged the document (e.g. tape to glue together fragments or chemical solutions to enhance faded writing).</skos:definition>
        <skos:definition rdf:parseType="Resource">
            <rdf:value>References</rdf:value>             
            <dct:bibliographicCitation>Archives Damage Atlas, pp. 58-63 and 75-79 (accessed 13.04.2023)
                https://www.metamorfoze.nl/sites/default/files/documents/schadeatlas-2010%20engels.pdf</dct:bibliographicCitation>
        </skos:definition>
        <skos:broader rdf:resource="http://gams.uni-graz.at/thesaurus/intentionalDamage"/>
    </skos:Concept>
    
</rdf:RDF>